# baseURI: http://loop3d.org/GSO/ontology/2020/1/hydrology/ontology
# imports: http://loop3d.org/GSO/ontology/2020/1/common/ontology

@prefix : <http://loop3d.org/GSO/ontology/2020/1/hydrology/> .
@prefix dct: <http://purl.org/dc/terms/> .
@prefix gsoc: <http://loop3d.org/GSO/ontology/2020/1/common/> .
@prefix gsoh: <http://loop3d.org/GSO/ontology/2020/1/hydrology/> .
@prefix owl: <http://www.w3.org/2002/07/owl#> .
@prefix rdf: <http://www.w3.org/1999/02/22-rdf-syntax-ns#> .
@prefix rdfs: <http://www.w3.org/2000/01/rdf-schema#> .
@prefix skos: <http://www.w3.org/2004/02/skos/core#> .
@prefix xsd: <http://www.w3.org/2001/XMLSchema#> .

gsoh:Hydrologic_Event
  rdf:type owl:Class ;
  rdfs:label "Hydrologic Event"@en ;
  rdfs:subClassOf gsoc:Event ;
.
gsoh:Hydrologic_Process
  rdf:type owl:Class ;
  rdfs:comment "Process that has a water entity as an output.  Water entities include things such as rivers, lakes, ocean, clouds, aquifers as well as various qualities like river stage, mean sea level."@en ;
  rdfs:label "Hydrologic Process"@en ;
  rdfs:subClassOf gsoc:Process ;
.
gsoh:Sea_Level_Fluctuation
  rdf:type owl:Class ;
  rdfs:comment "process of alteration of global sea levels due to changes in either the volume of water in the world's oceans or net changes in the volume of the oceanic basins."@en ;
  rdfs:label "Sea Level Fluctuation"@en ;
  rdfs:subClassOf gsoh:Hydrologic_Process ;
.
gsoh:boyan_brodaric
  rdf:type owl:NamedIndividual ;
  rdfs:comment "affiliation:  Natural Resources Canada, Geological Survey of Canada" ;
  rdfs:comment "e-mail: mailto:boyan.brodaric@canada.ca " ;
  rdfs:comment "orcid: https://orcid.org/0000-0002-7987-3810" ;
  rdfs:label "Dr. Boyan Brodaric" ;
.
gsoh:ontology
  rdf:type owl:Ontology ;
  dct:created "2021-03-26"^^xsd:date ;
  dct:creator gsoh:boyan_brodaric ;
  dct:creator gsoh:stephen_richard ;
  dct:license <https://creativecommons.org/licenses/by/4.0/legalcode> ;
  dct:modified "2021-03-26"^^xsd:date ;
  dct:publisher "ARC Loop3D project;  https://loop3d.org/" ;
  dct:publisher "Geological Survey of Canada, Natural Resources Canada, Government of Canada" ;
  dct:rights "Copyright (c) 2021 Government of Canada" ;
  rdfs:comment "Hydrology ontology"@en ;
  rdfs:label "Geoscience Ontology, Hydrology "@en ;
  owl:imports gsoc:ontology ;
  skos:definition "Hydrogeology module in Geoscience Ontology"@en ;
  skos:prefLabel "Geoscience Ontology, Geoscience Ontology, "@en ;
.
gsoh:stephen_richard
  rdf:type owl:NamedIndividual ;
  rdfs:comment "e-mail: mailto:smrTucson@gmail.com " ;
  rdfs:comment "orcid: https://orcid.org/0000-0001-6041-5302" ;
  rdfs:label "Dr. Stephen M. Richard" ;
.
