# baseURI: http://loop3d.org/GSO/ontology/2020/1/geologicsetting/ontology
# imports: http://loop3d.org/GSO/ontology/2020/1/common/ontology
# imports: http://loop3d.org/GSO/ontology/2020/1/geologicprocess/ontology
# imports: http://loop3d.org/GSO/ontology/2020/1/geology/ontology
# imports: http://loop3d.org/GSO/ontology/2020/1/rockobject/ontology

@prefix : <http://loop3d.org/GSO/ontology/2020/1/geologicsetting/> .
@prefix gsen: <http://loop3d.org/GSO/ontology/2020/1/geologicsetting/> .
@prefix gsoc: <http://loop3d.org/GSO/ontology/2020/1/common/> .
@prefix gsog: <http://loop3d.org/GSO/ontology/2020/1/geology/> .
@prefix gspr: <http://loop3d.org/GSO/ontology/2020/1/geologicprocess/> .
@prefix gsro: <http://loop3d.org/GSO/ontology/2020/1/rockobject/> .
@prefix owl: <http://www.w3.org/2002/07/owl#> .
@prefix rdf: <http://www.w3.org/1999/02/22-rdf-syntax-ns#> .
@prefix rdfs: <http://www.w3.org/2000/01/rdf-schema#> .
@prefix xsd: <http://www.w3.org/2001/XMLSchema#> .

gsen:Abandoned_Channel_Setting
  rdf:type owl:Class ;
  rdfs:comment "A drainage channel along which runoff no longer occurs, as on an alluvial fan"@en ;
  rdfs:comment "dct:source--  Neuendorf et al., 2005"@en ;
  rdfs:label "abandoned river channel setting"@en ;
  rdfs:subClassOf gsen:River_Plain_System_Setting ;
  rdfs:subClassOf [
      rdf:type owl:Restriction ;
      owl:onProperty gsoc:isStaticPartOf ;
      owl:someValuesFrom gsen:River_Plain_System_Setting ;
    ] ;
.
gsen:Above_Carbonate_Compensation_Depth_Setting
  rdf:type owl:Class ;
  rdfs:comment "Marine environment in which carbonate sediment does not dissolve before reaching the sea floor and can accumulate."@en ;
  rdfs:comment "dct:source--  this vocabulary"@en ;
  rdfs:label "above carbonate compensation depth setting"@en ;
  rdfs:subClassOf gsen:Marine_Setting ;
.
gsen:Abyssal_Setting
  rdf:type owl:Class ;
  rdfs:comment "The ocean environment at water depths between 3500 and 6000 metres"@en ;
  rdfs:comment "dct:source--  Neuendorf et al., 2005"@en ;
  rdfs:label "abyssal setting"@en ;
  rdfs:subClassOf gsen:Marine_Setting ;
.
gsen:Active_Continental_Margin_Setting
  rdf:type owl:Class ;
  rdfs:comment "Plate margin setting on continental crust."@en ;
  rdfs:comment "dct:source--  This vocabulary"@en ;
  rdfs:label "active continental margin setting"@en ;
  rdfs:subClassOf gsen:Plate_Margin_Setting ;
.
gsen:Active_Spreading_Center_Setting
  rdf:type owl:Class ;
  rdfs:comment "Divergent plate margin at which new oceanic crust is being formed"@en ;
  rdfs:comment "dct:source--  this vocabulary"@en ;
  rdfs:label "active spreading center setting"@en ;
  rdfs:subClassOf gsen:Plate_Margin_Setting ;
  rdfs:subClassOf gsen:Plate_Spreading_Center_Setting ;
.
gsen:Aeolian_Process_Setting
  rdf:type owl:Class ;
  rdfs:comment "Sedimentary setting in which wind is the dominant process producing, transporting, and depositing sediment. Typically has low-relief plain or piedmont slope physiography."@en ;
  rdfs:comment "dct:source--  this vocabulary"@en ;
  rdfs:label "aeolian process setting"@en ;
  rdfs:subClassOf gsen:Subaerial_Setting ;
  rdfs:subClassOf gsen:Terrestrial_Setting ;
.
gsen:Algal_Flat_Setting
  rdf:type owl:Class ;
  rdfs:comment "Modern algal flats are found on rock or mud in areas flooded only by the highest tides and are often subject to high evaporation rates. Algal flats survive only when an area is salty enough to eliminate snails and other herbivorous animals that eat algae, yet is not so salty that the algae cannot survive. The most common species of algae found on algal flats are blue-green algae of the genera Scytonema and Schizothrix. These algae can tolerate the daily extremes in temperature and oxygen that typify conditions on the flats. Other plants sometimes found on algal flats include one-celled green algae, flagellates, diatoms, bacteria, and isolated scrubby red and black mangroves, as well as patches of saltwort. Animals include false cerith, cerion snails, fiddler crabs, and great land crabs. Flats with well developed algal mats are restricted for the most part to the Keys, with Sugarloaf and Crane Keys offering prime examples of algal flat habitat. (Audubon, 1991)"@en ;
  rdfs:comment "dct:source--  http://www.audubonofflorida.org/main/wetlands/chp3.htm, Reading, 1978"@en ;
  rdfs:label "algal flat setting"@en ;
  rdfs:subClassOf gsen:Low_Energy_Shoreline_Setting ;
.
gsen:Alluvial_Fan_Setting
  rdf:type owl:Class ;
  rdfs:comment "A low, outspread, relatively flat to gently sloping mass of loose rock material, shaped like an open fan or a segment of a cone, deposited by a stream (esp. in a semiarid region) at the place where it issues from a narrow mountain valley upon a plain or broad valley, or where a tributary stream is near or at its junction with the main stream, or wherever a constriction in a valley abruptly ceases or the gradient of the stream suddenly decreases, it is steepest near the mouth of the valley where its apex points upstream, and it slopes gently and convexly outward with gradually decreasing gradient"@en ;
  rdfs:comment "dct:source--  Neuendorf et al., 2005"@en ;
  rdfs:label "alluvial fan setting"@en ;
  rdfs:subClassOf gsen:Piedmont_Slope_System_Setting ;
  rdfs:subClassOf [
      rdf:type owl:Restriction ;
      owl:onProperty gsoc:isStaticPartOf ;
      owl:someValuesFrom gsen:Piedmont_Slope_System_Setting ;
    ] ;
.
gsen:Alluvial_Plain_Setting
  rdf:type owl:Class ;
  rdfs:comment "An assemblage landforms produced by alluvial and fluvial processes (braided streams, terraces, etc.) that form low gradient, regional ramps along the flanks of mountains and extend great distances from their sources (e.g.high Plains of North America). (NRCS GLOSSARY OF LANDFORM AND GEOLOGIC TERMS). A level or gently sloping tract or a slightly undulating land surface produced by extensive deposition of alluvium... Synonym-- wash plain,...river plain, aggraded valley plain,... (Jackson, 1997, p. 17). May include one or more River plain systems."@en ;
  rdfs:comment "dct:source--  North American Geologic-map Data Model Science Language Technical Team, 2004, Sedimentary materials:science language for their classification, description, and interpretation in digital geologic-map databases, Version 1.0 (12/18/2004): U.S. Geological Survey Open-File Report 2004-1451 appendix C, 595 p., accessed at http://pubs.usgs.gov/of/2004/1451/sltt/appendixC/,"@en ;
  rdfs:label "alluvial plain setting"@en ;
  rdfs:subClassOf gsen:Piedmont_Slope_System_Setting ;
  rdfs:subClassOf [
      rdf:type owl:Restriction ;
      owl:onProperty gsoc:isStaticPartOf ;
      owl:someValuesFrom gsen:Piedmont_Slope_System_Setting ;
    ] ;
.
gsen:Anoxic_Setting
  rdf:type owl:Class ;
  rdfs:comment "Setting depleted in oxygen, typically subaqueous."@en ;
  rdfs:comment "dct:source--  this vocabulary"@en ;
  rdfs:label "anoxic setting"@en ;
  rdfs:subClassOf gsen:Planet_Surface_Setting ;
.
gsen:Arid_Or_Semi_Arid_Environment_Setting
  rdf:type owl:Class ;
  rdfs:comment "Setting characterized by mean annual precipitation of 10 inches (25 cm) or less. (Jackson, 1997, p. 172). Equivalent to SLTT 'Desert setting', but use 'Arid' to emphasize climatic nature of setting definition."@en ;
  rdfs:comment "dct:source--  North American Geologic-map Data Model Science Language Technical Team, 2004, Sedimentary materials:science language for their classification, description, and interpretation in digital geologic-map databases, Version 1.0 (12/18/2004): U.S. Geological Survey Open-File Report 2004-1451 appendix C, 595 p., accessed at http://pubs.usgs.gov/of/2004/1451/sltt/appendixC/,"@en ;
  rdfs:label "arid or semi arid environment setting"@en ;
  rdfs:subClassOf gsen:Planet_Surface_Setting ;
.
gsen:Back_Arc_Setting
  rdf:type owl:Class ;
  rdfs:comment "Tectonic setting adjacent to a volcanic arc formed above a subduction zone. The back arc setting is on the opposite side of the volcanic arc from the trench at which oceanic crust is consumed in a subduction zone. Back arc setting includes terrane that is affected by plate margin and arc-related processes."@en ;
  rdfs:comment "dct:source--  this vocabulary"@en ;
  rdfs:label "back arc setting"@en ;
  rdfs:subClassOf gsen:Tectonic_Setting ;
.
gsen:Backreef_Setting
  rdf:type owl:Class ;
  gsoc:isPartOf gsen:Biological_Reef_Setting ;
  rdfs:comment "The landward side of a reef. The term is often used adjectivally to refer to deposits within the restricted lagoon behind a barrier reef, such as the back-reef facies of lagoonal deposits. In some places, as on a platform-edge reef tract, back reef refers to the side of the reef away from the open sea, even though no land may be nearby"@en ;
  rdfs:comment "dct:source--  Neuendorf et al., 2005"@en ;
  rdfs:label "backreef setting"@en ;
  rdfs:subClassOf gsen:Biological_Reef_Setting ;
.
gsen:Barrier_Beach_Setting
  rdf:type owl:Class ;
  rdfs:comment "A narrow, elongate sand or gravel ridge rising slightly above the high-tide level and extending generally parallel with the shore, but separated from it by a lagoon (Shepard, 1954, p.1904), estuary, or marsh, it is extended by longshore transport and is rarely more than several kilometers long."@en ;
  rdfs:comment "dct:source--  Neuendorf et al., 2005"@en ;
  rdfs:label "barrier beach setting"@en ;
  rdfs:subClassOf gsen:Barrier_Island_Coastline_Setting ;
  rdfs:subClassOf gsen:Beach_Setting ;
  rdfs:subClassOf [
      rdf:type owl:Restriction ;
      owl:onProperty gsoc:isStaticPartOf ;
      owl:someValuesFrom gsen:Barrier_Island_Coastline_Setting ;
    ] ;
.
gsen:Barrier_Island_Coastline_Setting
  rdf:type owl:Class ;
  rdfs:comment "dct:source--  this vocabulary"@en ;
  rdfs:comment "setting meant to include all the various geographic elements typically associated with a barrier island coastline, including the barrier islands, and geomorphic/geographic elements that are linked by processes associated with the presence of the island (e.g. wash over fans, inlet channel, back barrier lagoon)."@en ;
  rdfs:label "barrier island coastline setting"@en ;
  rdfs:subClassOf gsen:Shoreline_Setting ;
.
gsen:Barrier_Lagoon_Setting
  rdf:type owl:Class ;
  rdfs:comment "A lagoon that is roughly parallel to the coast and is separated from the open ocean by a strip of land or by a barrier reef. Tidal influence is typically restricted and the lagoon is commonly hypersaline."@en ;
  rdfs:comment "dct:source--  Neuendorf et al., 2005"@en ;
  rdfs:label "barrier lagoon setting"@en ;
  rdfs:subClassOf gsen:Barrier_Island_Coastline_Setting ;
  rdfs:subClassOf gsen:Lagoonal_Setting ;
  rdfs:subClassOf [
      rdf:type owl:Restriction ;
      owl:onProperty gsoc:isStaticPartOf ;
      owl:someValuesFrom gsen:Barrier_Island_Coastline_Setting ;
    ] ;
.
gsen:Basin_Bog_Setting
  rdf:type owl:Class ;
  rdfs:comment "An ombrotrophic or ombrogene peat/bog whose nutrient supply is exclusively from rain water (including snow and atmospheric fallout) therefore making nutrients extremely oligotrophic"@en ;
  rdfs:comment "dct:source--  1-GE WP3; Neuendorf et al.(2005), p. 451"@en ;
  rdfs:label "basin bog setting"@en ;
  rdfs:subClassOf gsen:Bog_Setting ;
.
gsen:Basin_Plain_Setting
  rdf:type owl:Class ;
  rdfs:comment "Near flat areas of ocean floor, slope less than 1:1000, generally receive only distal turbidite and pelagic sediments."@en ;
  rdfs:comment "dct:source--  Bates & Jackson, 1987, Heezen & Laughton, 1963, Reading, 1978, p. 390"@en ;
  rdfs:label "basin plain setting"@en ;
  rdfs:subClassOf gsen:Marine_Setting ;
  rdfs:subClassOf [
      rdf:type owl:Restriction ;
      owl:onProperty gsoc:isStaticPartOf ;
      owl:someValuesFrom gsen:Marine_Setting ;
    ] ;
.
gsen:Bathyal_Setting
  rdf:type owl:Class ;
  rdfs:comment "The ocean environment at water depths between 200 and 3500 metres"@en ;
  rdfs:comment "dct:source--  Neuendorf et al., 2005"@en ;
  rdfs:label "bathyal setting"@en ;
  rdfs:subClassOf gsen:Marine_Setting ;
.
gsen:Beach_Setting
  rdf:type owl:Class ;
  rdfs:comment "The unconsolidated material at the shoreline that covers a gently sloping zone, typically with a concave profile, extending landward from the low-water line to the place where there is a definite change in material or physiographic form (such as a cliff), or to the line of permanent vegetation (usually the effective limit of the highest storm waves), at the shore of a body of water, formed and washed by waves or tides, usually covered by sand or gravel, and lacking a bare rocky surface."@en ;
  rdfs:comment "dct:source--  Neuendorf et al., 2005"@en ;
  rdfs:label "beach setting"@en ;
  rdfs:subClassOf gsen:Shoreline_Setting ;
.
gsen:Below_Carbonate_Compensation_Depth_Setting
  rdf:type owl:Class ;
  rdfs:comment "Marine environment in which water is deep enough that carbonate sediment goes into solution before it can accumulate on the sea floor."@en ;
  rdfs:comment "dct:source--  this vocabulary"@en ;
  rdfs:label "below carbonate compensation depth setting"@en ;
  rdfs:subClassOf gsen:Marine_Setting ;
.
gsen:Biological_Reef_Setting
  rdf:type owl:Class ;
  rdfs:comment "A ridgelike or moundlike structure, layered or massive, built by sedentary calcareous organisms, esp. corals, and consisting mostly of their remains, it is wave-resistant and stands topographically above the surrounding contemporaneously deposited sediment."@en ;
  rdfs:comment "dct:source--  Neuendorf et al., 2005"@en ;
  rdfs:label "biological reef setting"@en ;
  rdfs:subClassOf gsen:Marine_Setting ;
  rdfs:subClassOf [
      rdf:type owl:Restriction ;
      owl:onProperty gsoc:hasStaticPart ;
      owl:someValuesFrom gsen:Backreef_Setting ;
    ] ;
  rdfs:subClassOf [
      rdf:type owl:Restriction ;
      owl:onProperty gsoc:hasStaticPart ;
      owl:someValuesFrom gsen:Forereef_Setting ;
    ] ;
  rdfs:subClassOf [
      rdf:type owl:Restriction ;
      owl:onProperty gsoc:hasStaticPart ;
      owl:someValuesFrom gsen:Reef_Flat_Setting ;
    ] ;
  rdfs:subClassOf [
      rdf:type owl:Restriction ;
      owl:onProperty gsoc:isStaticPartOf ;
      owl:someValuesFrom gsen:Marine_Setting ;
    ] ;
.
gsen:Blanket_Bog_Setting
  rdf:type owl:Class ;
  rdfs:comment "Topogeneous bog/peat whose moisture content is largely dependent on surface water. It is relatively rich in plant nutrients, nitrogen, and mineral matter, is mildly acidic to nearly neutral, and contains little or no cellulose, forms in topographic depressions with essential stagnat or non-moving minerotrophic water supply"@en ;
  rdfs:comment "dct:source--  1-GE WP3; Neuendorf et al.(2005), p. 675"@en ;
  rdfs:label "blanket bog"@en ;
  rdfs:subClassOf gsen:Bog_Setting ;
.
gsen:Bog_Setting
  rdf:type owl:Class ;
  rdfs:comment "Waterlogged, spongy ground, consisting primarily of mosses, containing acidic, decaying vegetation that may develop into peat."@en ;
  rdfs:comment "dct:source--  Jackson, 1997, North American Geologic-map Data Model Science Language Technical Team, 2004, Sedimentary materials:science language for their classification, description, and interpretation in digital geologic-map databases, Version 1.0 (12/18/2004): U.S. Geological Survey Open-File Report 2004-1451 appendix C, 595 p., accessed at http://pubs.usgs.gov/of/2004/1451/sltt/appendixC/,"@en ;
  rdfs:label "bog setting"@en ;
  rdfs:subClassOf gsen:Terrestrial_Setting ;
  rdfs:subClassOf gsen:Wetland_Setting ;
.
gsen:Braided_Channel_Setting
  rdf:type owl:Class ;
  rdfs:comment "A stream that divides into or follows an interlacing or tangled network of several small branching and reuniting shallow channels separated from each other by ephemeral branch islands or channel bars, resembling in plan the strands of a complex braid. Such a stream is generally believed to indicate an inability to carry all of its load, such as an overloaded and aggrading stream flowing in a wide channel on a floodplain"@en ;
  rdfs:comment "dct:source--  Neuendorf et al., 2005"@en ;
  rdfs:label "braided river channel setting"@en ;
  rdfs:subClassOf gsen:River_Channel_Setting ;
.
gsen:Carbonate_Dominated_Shoreline_Setting
  rdf:type owl:Class ;
  rdfs:comment "A shoreline setting in which terrigenous input is minor compared to local carbonate sediment production. Constructional biogenic activity is an important element in geomorphic development."@en ;
  rdfs:comment "dct:source--  this vocabulary"@en ;
  rdfs:label "carbonate dominated shoreline setting"@en ;
  rdfs:subClassOf gsen:Shoreline_Setting ;
.
gsen:Cave_Setting
  rdf:type owl:Class ;
  rdfs:comment "A natural underground open space, it generally has a connection to the surface, is large enough for a person to enter, and extends into darkness. The most common type of cave is formed in limestone by dissolution."@en ;
  rdfs:comment "dct:source--  Neuendorf et al., 2005"@en ;
  rdfs:label "cave setting"@en ;
  rdfs:subClassOf gsen:Planet_Surface_Setting ;
.
gsen:Coastal_Dune_Field_Setting
  rdf:type owl:Class ;
  rdfs:comment "A dune field on low-lying land recently abandoned or built up by the sea, the dunes may ascend a cliff and travel inland."@en ;
  rdfs:comment "dct:source--  Neuendorf et al., 2005"@en ;
  rdfs:label "coastal dune field setting"@en ;
  rdfs:subClassOf gsen:Dune_Field_Setting ;
.
gsen:Coastal_Plain_Setting
  rdf:type owl:Class ;
  rdfs:comment "A low relief plain bordering a water body extending inland to the nearest elevated land, sloping very gently towards the water body. Distinguished from alluvial plain by presence of relict shoreline-related deposits or morphology."@en ;
  rdfs:comment "dct:source--  based on Neuendorf et al, 2005, p. 125"@en ;
  rdfs:label "coastal plain setting"@en ;
  rdfs:subClassOf gsen:Shoreline_Setting ;
  rdfs:subClassOf gsen:Subaerial_Setting ;
.
gsen:Collisional_Setting
  rdf:type owl:Class ;
  rdfs:comment "Tectonic setting in which two continental crustal plates impact and are sutured together after intervening oceanic crust is entirely consumed at a subduction zone separating the plates. Such collision typically involves major mountain forming events, exemplified by the modern Alpine and Himalayan mountain chains."@en ;
  rdfs:comment "dct:source--  this vocabulary"@en ;
  rdfs:label "collisional setting"@en ;
  rdfs:subClassOf gsen:Tectonic_Setting ;
.
gsen:Contact_Metamorphic_Setting
  rdf:type owl:Class ;
  rdfs:comment "Metamorphism of country rock at the contact of an igneous body.  Because metamorphism inherently requires elevated temperature or pressure, it is necessarily an Earth interior setting"@en ;
  rdfs:comment "dct:source--  NADM metamorphic rock vocabulary SLTTm1.0, 2004"@en ;
  rdfs:label "contact metamorphic setting"@en ;
  rdfs:subClassOf gsen:Planet_Interior_Setting ;
  rdfs:subClassOf [
      rdf:type owl:Restriction ;
      owl:onProperty gsoc:isStaticPartOf ;
      owl:someValuesFrom gsen:Planet_Interior_Setting ;
    ] ;
.
gsen:Continental_Borderland_Setting
  rdf:type owl:Class ;
  rdfs:comment "An area of the continental margin between the shoreline and the continental slope that is topographically more complex than the continental shelf. It is characterized by ridges and basins, some of which are below the depth of the continental shelf. An example is the southern California continental borderland,.... (Jackson, 1997, p. 138).."@en ;
  rdfs:comment "dct:source--  North American Geologic-map Data Model Science Language Technical Team, 2004, Sedimentary materials:science language for their classification, description, and interpretation in digital geologic-map databases, Version 1.0 (12/18/2004): U.S. Geological Survey Open-File Report 2004-1451 appendix C, 595 p., accessed at http://pubs.usgs.gov/of/2004/1451/sltt/appendixC/"@en ;
  rdfs:label "continental borderland setting"@en ;
  rdfs:subClassOf gsen:Marine_Setting ;
  rdfs:subClassOf [
      rdf:type owl:Restriction ;
      owl:onProperty gsoc:isStaticPartOf ;
      owl:someValuesFrom gsen:Marine_Setting ;
    ] ;
.
gsen:Continental_Crust_Setting
  rdf:type owl:Class ;
  rdfs:comment "That type of the Earth's crust which underlies the continents and the continental shelves, it is equivalent to the sial and continental sima and ranges in thickness from about 25 km to more than 70 km under mountain ranges, averaging ~40 km. The density of the continental crust averages ~2.8 g/cm3 and is ~2.7 g.cm3 in the upper layer. The velocities of compressional seismic waves through it average ~6.5 km/s and are less than ~7.0 km/sec."@en ;
  rdfs:comment "dct:source--  Neuendorf et al., 2005"@en ;
  rdfs:label "continental crustal setting"@en ;
  rdfs:subClassOf gsen:Crustal_Setting ;
.
gsen:Continental_Rift_Setting
  rdf:type owl:Class ;
  rdfs:comment "Extended terrane in a zone of continental breakup, may include incipient oceanic crust. Examples include Red Sea, East Africa Rift, Salton Trough"@en ;
  rdfs:comment "dct:source--  this vocabulary"@en ;
  rdfs:label "continental rift setting"@en ;
  rdfs:subClassOf gsen:Extended_Terrane_Setting ;
.
gsen:Continental_Shelf_Setting
  rdf:type owl:Class ;
  rdfs:comment "That part of the ocean floor that is between the shoreline and the continental slope (or, when there is no noticeable continental slope, a depth of 200 m). It is characterized by its gentle slope of 0.1 degree (Jackson, 1997, p. 138). Continental shelves have a classic shoreline-shelf-slope profile termed 'clinoform'."@en ;
  rdfs:comment "dct:source--  North American Geologic-map Data Model Science Language Technical Team, 2004, Sedimentary materials:science language for their classification, description, and interpretation in digital geologic-map databases, Version 1.0 (12/18/2004): U.S. Geological Survey Open-File Report 2004-1451 appendix C, 595 p., accessed at http://pubs.usgs.gov/of/2004/1451/sltt/appendixC/"@en ;
  rdfs:label "continental shelf setting"@en ;
  rdfs:subClassOf gsen:Marine_Setting ;
  rdfs:subClassOf [
      rdf:type owl:Restriction ;
      owl:onProperty gsoc:isStaticPartOf ;
      owl:someValuesFrom gsen:Marine_Setting ;
    ] ;
.
gsen:Crustal_Setting
  rdf:type owl:Class ;
  rdfs:comment "The outermost layer or shell of the Earth, defined according to various criteria, including seismic velocity, density and composition, that part of the Earth above the Mohorovicic discontinuity, made up of the sial and the sima."@en ;
  rdfs:comment "dct:source--  Neuendorf et al., 2005"@en ;
  rdfs:label "crustal setting"@en ;
  rdfs:subClassOf gsen:Planet_Interior_Setting ;
  rdfs:subClassOf [
      rdf:type owl:Restriction ;
      owl:onClass gsro:Crust ;
      owl:onProperty gsoc:hasStaticPart ;
      owl:qualifiedCardinality "1"^^xsd:nonNegativeInteger ;
    ] ;
  rdfs:subClassOf [
      rdf:type owl:Restriction ;
      owl:onProperty gsoc:isStaticPartOf ;
      owl:someValuesFrom gsen:Planet_Interior_Setting ;
    ] ;
.
gsen:Cutoff_Meander_Setting
  rdf:type owl:Class ;
  rdfs:comment "The abandoned, bow- or horseshoe-shaped channel of a former meander, left when the stream formed a cutoff across a narrow meander neck. Note that these are typically lakes, thus also lacustrine."@en ;
  rdfs:comment "dct:source--  Neuendorf et al., 2005"@en ;
  rdfs:label "cutoff meander setting"@en ;
  rdfs:subClassOf gsen:River_Plain_System_Setting ;
  rdfs:subClassOf [
      rdf:type owl:Restriction ;
      owl:onProperty gsoc:isStaticPartOf ;
      owl:someValuesFrom gsen:River_Plain_System_Setting ;
    ] ;
.
gsen:Deep_Sea_Trench_Setting
  rdf:type owl:Class ;
  rdfs:comment "Deep ocean basin with steep (average 10 degrees) slope toward land, more gentle slope (average 5 degrees) towards the sea, and abundant seismic activity on landward side of trench. Does not denote water depth, but may be very deep."@en ;
  rdfs:comment "dct:source--  Reading 1978"@en ;
  rdfs:label "deep sea trench setting"@en ;
  rdfs:subClassOf gsen:Marine_Setting ;
  rdfs:subClassOf [
      rdf:type owl:Restriction ;
      owl:onProperty gsoc:isStaticPartOf ;
      owl:someValuesFrom gsen:Marine_Setting ;
    ] ;
.
gsen:Delta_Front_Setting
  rdf:type owl:Class ;
  rdfs:comment "A narrow zone where deposition in deltas is most active, consisting of a continuous sheet of sand, and occurring within the effective depth of wave erosion (10 m or less). It is the zone separating the prodelta from the delta plain, and it may or may not be steep\\"@en ;
  rdfs:comment "dct:source--  Neuendorf et al., 2005"@en ;
  rdfs:label "delta front setting"@en ;
  rdfs:subClassOf gsen:Delta_System_Setting ;
  rdfs:subClassOf [
      rdf:type owl:Restriction ;
      owl:onProperty gsoc:isStaticPartOf ;
      owl:someValuesFrom gsen:Delta_System_Setting ;
    ] ;
.
gsen:Delta_Plain_Setting
  rdf:type owl:Class ;
  rdfs:comment "The level or nearly level surface composing the landward part of a large or compound delta, strictly, an alluvial plain characterized by repeated channel bifurcation and divergence, multiple distributary channels, and interdistributary flood basins"@en ;
  rdfs:comment "dct:source--  Neuendorf et al., 2005"@en ;
  rdfs:label "delta plain setting"@en ;
  rdfs:subClassOf gsen:Delta_System_Setting ;
  rdfs:subClassOf [
      rdf:type owl:Restriction ;
      owl:onProperty gsoc:isStaticPartOf ;
      owl:someValuesFrom gsen:Delta_System_Setting ;
    ] ;
.
gsen:Delta_System_Setting
  rdf:type owl:Class ;
  rdfs:comment "Environments at the mouth of a river or stream that enters a standing body of water (ocean or lake). The delta forms a triangular or fan-shaped plain of considerable area. Subaerial parts of the delta are crossed by many distributaries of the main river, and commonly extend beyond the general trend of the coast. Subaqueous parts of the delta merge with the adjacent basin floor, and are progressively influenced by non-fluvial processes. Deltas result from the accumulation of sediment supplied by the river in such quantities that it is not removed by tides, waves, and currents. Adapted from the Glossary of Geology definition for delta (Jackson, 1997, p. 167)."@en ;
  rdfs:comment "dct:source--  North American Geologic-map Data Model Science Language Technical Team, 2004, Sedimentary materials:science language for their classification, description, and interpretation in digital geologic-map databases, Version 1.0 (12/18/2004): U.S. Geological Survey Open-File Report 2004-1451 appendix C, 595 p., accessed at http://pubs.usgs.gov/of/2004/1451/sltt/appendixC/"@en ;
  rdfs:label "deltaic system setting"@en ;
  rdfs:subClassOf gsen:Shoreline_Setting ;
.
gsen:Distributary_Channel_Setting
  rdf:type owl:Class ;
  rdfs:comment "A divergent stream flowing away from the main stream and not returning to it, as in a delta or on an alluvial plain"@en ;
  rdfs:comment "dct:source--  Neuendorf et al., 2005"@en ;
  rdfs:label "delta distributary channel setting"@en ;
  rdfs:subClassOf gsen:Delta_System_Setting ;
  rdfs:subClassOf [
      rdf:type owl:Restriction ;
      owl:onProperty gsoc:isStaticPartOf ;
      owl:someValuesFrom gsen:Delta_System_Setting ;
    ] ;
.
gsen:Distributary_Mouth_Setting
  rdf:type owl:Class ;
  rdfs:comment "The mouth of a delta distributary channel where fluvial discharge moves from confined to unconfined flow conditions"@en ;
  rdfs:comment "dct:source--  Neuendorf et al., 2005"@en ;
  rdfs:label "delta distributary mouth setting"@en ;
  rdfs:subClassOf gsen:Delta_System_Setting ;
  rdfs:subClassOf [
      rdf:type owl:Restriction ;
      owl:onProperty gsoc:isStaticPartOf ;
      owl:someValuesFrom gsen:Delta_System_Setting ;
    ] ;
.
gsen:Dune_Field_Setting
  rdf:type owl:Class ;
  rdfs:comment "Extensive deposits on sand in an area where the supply is abundant. As a characteristic, individual dunes somewhat resemble barchans but are highly irregular in shape and crowded, erg areas of the Sahara are an example."@en ;
  rdfs:comment "dct:source--  Neuendorf et al., 2005"@en ;
  rdfs:label "dunefield setting"@en ;
  rdfs:subClassOf gsen:Aeolian_Process_Setting ;
.
gsen:Englacial_Setting
  rdf:type owl:Class ;
  rdfs:comment "Contained, embedded, or carried within the body of a glacier or ice sheet, said of meltwater streams, till, drift, moraine"@en ;
  rdfs:comment "dct:source--  Neuendorf et al., 2005"@en ;
  rdfs:label "englacial setting"@en ;
  rdfs:subClassOf gsen:Glacier_Related_Setting ;
  rdfs:subClassOf [
      rdf:type owl:Restriction ;
      owl:onProperty gsoc:isStaticPartOf ;
      owl:someValuesFrom gsen:Glacier_Related_Setting ;
    ] ;
.
gsen:Epicontinental_Marine_Setting
  rdf:type owl:Class ;
  rdfs:comment "Marine setting situated within the interior of the continent, rather than at the edge of a continent."@en ;
  rdfs:comment "dct:source--  North American Geologic-map Data Model Science Language Technical Team, 2004, Sedimentary materials:science language for their classification, description, and interpretation in digital geologic-map databases, Version 1.0 (12/18/2004): U.S. Geological Survey Open-File Report 2004-1451 appendix C, 595 p., accessed at http://pubs.usgs.gov/of/2004/1451/sltt/appendixC/"@en ;
  rdfs:label "epicontinental marine setting"@en ;
  rdfs:subClassOf gsen:Marine_Setting ;
.
gsen:Estuarine_Delta_Setting
  rdf:type owl:Class ;
  rdfs:comment "A delta that has filled, or is in the process of filling, an estuary"@en ;
  rdfs:comment "dct:source--  Neuendorf et al., 2005"@en ;
  rdfs:label "estuarine delta setting"@en ;
  rdfs:subClassOf gsen:Delta_System_Setting ;
  rdfs:subClassOf gsen:Estuary_Setting ;
  rdfs:subClassOf [
      rdf:type owl:Restriction ;
      owl:onProperty gsoc:isStaticPartOf ;
      owl:someValuesFrom gsen:Estuary_Setting ;
    ] ;
.
gsen:Estuarine_Lagoon_Setting
  rdf:type owl:Class ;
  rdfs:comment "A lagoon produced by the temporary sealing of a river estuary by a storm barrier. Such lagoons are usually seasonal and exist until the river breaches the barrier, they occur in regions of low or spasmodic rainfall"@en ;
  rdfs:comment "dct:source--  Neuendorf et al., 2005"@en ;
  rdfs:label "estuarine lagoon setting"@en ;
  rdfs:subClassOf gsen:Estuary_Setting ;
  rdfs:subClassOf gsen:Lagoonal_Setting ;
  rdfs:subClassOf [
      rdf:type owl:Restriction ;
      owl:onProperty gsoc:isStaticPartOf ;
      owl:someValuesFrom gsen:Estuary_Setting ;
    ] ;
.
gsen:Estuary_Setting
  rdf:type owl:Class ;
  rdfs:comment "Environments at the seaward end or the widened funnel-shaped tidal mouth of a river valley where fresh water comes into contact with seawater and where tidal effects are evident (adapted from Glossary of Geology, Jackson, 1997, p. 217)."@en ;
  rdfs:comment "dct:source--  North American Geologic-map Data Model Science Language Technical Team, 2004, Sedimentary materials:science language for their classification, description, and interpretation in digital geologic-map databases, Version 1.0 (12/18/2004): U.S. Geological Survey Open-File Report 2004-1451 appendix C, 595 p., accessed at http://pubs.usgs.gov/of/2004/1451/sltt/appendixC/"@en ;
  rdfs:label "estuary setting"@en ;
  rdfs:subClassOf gsen:Shoreline_Setting ;
.
gsen:Extended_Terrane_Setting
  rdf:type owl:Class ;
  rdfs:comment "Tectonic setting characterized by extension of the upper crust manifested by formation of rift valleys or basin and range physiography, with arrays of low to high angle normal faults. Modern examples include the North Sea, East Africa, and the Basin and Range of the North American Cordillera. Typically applied in continental crustal settings."@en ;
  rdfs:comment "dct:source--  This vocabulary"@en ;
  rdfs:label "extended terrane setting"@en ;
  rdfs:subClassOf gsen:Tectonic_Setting ;
.
gsen:Extra_Terrestrial_Setting
  rdf:type owl:Class ;
  rdfs:comment "Material originated outside of the Earth or its atmosphere."@en ;
  rdfs:comment "dct:source--  Neuendorf et al 2005,"@en ;
  rdfs:label "extra terrestrial setting"@en ;
  rdfs:subClassOf gsoc:Setting ;
  rdfs:subClassOf [
      rdf:type owl:Class ;
      owl:complementOf [
          rdf:type owl:Restriction ;
          owl:onProperty gsoc:containedBy ;
          owl:someValuesFrom [
              rdf:type owl:Class ;
              owl:oneOf (
                  gsoc:Earth
                ) ;
            ] ;
        ] ;
    ] ;
  owl:disjointWith [
      rdf:type owl:Restriction ;
      owl:onProperty gsoc:containedBy ;
      owl:someValuesFrom [
          rdf:type owl:Class ;
          owl:oneOf (
              gsoc:Earth
            ) ;
        ] ;
    ] ;
  owl:equivalentClass [
      rdf:type owl:Class ;
      owl:intersectionOf (
          gsoc:Setting
          [
            rdf:type owl:Class ;
            owl:complementOf [
                rdf:type owl:Restriction ;
                owl:onProperty gsoc:containedBy ;
                owl:someValuesFrom [
                    rdf:type owl:Class ;
                    owl:oneOf (
                        gsoc:Earth
                      ) ;
                  ] ;
              ] ;
          ]
        ) ;
    ] ;
.
gsen:Fast_Spreading_Center_Setting
  rdf:type owl:Class ;
  rdfs:comment "Spreading center at which the opening rate is greater than 100 mm per year."@en ;
  rdfs:comment "dct:source--  Macdonald 1982"@en ;
  rdfs:label "fast spreading center setting"@en ;
  rdfs:subClassOf gsen:Active_Spreading_Center_Setting ;
.
gsen:Floodplain_Setting
  rdf:type owl:Class ;
  rdfs:comment "The surface or strip of relatively smooth land adjacent to a river channel, constructed by the present river in its existing regimen and covered with water when the river overflows its banks. It is built of alluvium carried by the river during floods and deposited in the sluggish water beyond the influence of the swiftest current. A river has one floodplain and may have one or more terraces representing abandoned floodplains"@en ;
  rdfs:comment "dct:source--  Neuendorf et al., 2005"@en ;
  rdfs:label "floodplain setting"@en ;
  rdfs:subClassOf gsen:River_Plain_System_Setting ;
  rdfs:subClassOf [
      rdf:type owl:Restriction ;
      owl:onProperty gsoc:isStaticPartOf ;
      owl:someValuesFrom gsen:River_Plain_System_Setting ;
    ] ;
.
gsen:Forearc_Setting
  rdf:type owl:Class ;
  rdfs:comment "Tectonic setting between a subduction-related trench and a volcanic arc"@en ;
  rdfs:comment "dct:source--  1-GE WP3, Neuendorf et al.(2005), p. 249"@en ;
  rdfs:label "forearc setting"@en ;
  rdfs:subClassOf gsen:Plate_Margin_Setting ;
.
gsen:Foreland_Setting
  rdf:type owl:Class ;
  rdfs:comment "The exterior area of an orogenic belt where deformation occurs without significant metamorphism. Generally the foreland is closer to the continental interior than other portions of the orogenic belt are."@en ;
  rdfs:comment "dct:source--  1-GE WP3, Neuendorf et al.(2005), p. 250"@en ;
  rdfs:label "foreland setting"@en ;
  rdfs:subClassOf gsen:Tectonic_Setting ;
.
gsen:Forereef_Setting
  rdf:type owl:Class ;
  rdfs:comment "The seaward side of a reef, the slope covered with deposits of coarse reef talus"@en ;
  rdfs:comment "dct:source--  Neuendorf et al., 2005"@en ;
  rdfs:label "forereef setting"@en ;
  rdfs:subClassOf gsen:Biological_Reef_Setting ;
.
gsen:Gibber_Plain_Setting
  rdf:type owl:Class ;
  rdfs:comment "A desert plain strewn with wind-abraded pebbles, or gibbers, a gravelly desert."@en ;
  rdfs:comment "dct:source--  Neuendorf et al., 2005"@en ;
  rdfs:label "gibber plain setting"@en ;
  rdfs:subClassOf gsen:Arid_Or_Semi_Arid_Environment_Setting ;
  rdfs:subClassOf gsen:Subaerial_Setting ;
  rdfs:subClassOf gsen:Terrestrial_Setting ;
.
gsen:Glacial_Outwash_Plain_Setting
  rdf:type owl:Class ;
  rdfs:comment "Areas adjacent to glacial front dominated by sediment and water supplied by glacial melting."@en ;
  rdfs:comment "dct:source--  North American Geologic-map Data Model Science Language Technical Team, 2004, Sedimentary materials:science language for their classification, description, and interpretation in digital geologic-map databases, Version 1.0 (12/18/2004): U.S. Geological Survey Open-File Report 2004-1451 appendix C, 595 p., accessed at http://pubs.usgs.gov/of/2004/1451/sltt/appendixC/"@en ;
  rdfs:label "glacial outwash plain setting"@en ;
  rdfs:subClassOf gsen:Glacier_Related_Setting ;
  rdfs:subClassOf gsen:Terrestrial_Setting ;
  rdfs:subClassOf [
      rdf:type owl:Restriction ;
      owl:onProperty gsoc:isStaticPartOf ;
      owl:someValuesFrom gsen:Glacier_Related_Setting ;
    ] ;
.
gsen:Glacier_Lateral_Setting
  rdf:type owl:Class ;
  rdfs:comment "Settings adjacent to edges of confined glacier."@en ;
  rdfs:comment "dct:source--  this vocabulary"@en ;
  rdfs:label "glacier lateral setting"@en ;
  rdfs:subClassOf gsen:Glacier_Related_Setting ;
  rdfs:subClassOf [
      rdf:type owl:Restriction ;
      owl:onProperty gsoc:isStaticPartOf ;
      owl:someValuesFrom gsen:Glacier_Related_Setting ;
    ] ;
.
gsen:Glacier_Related_Setting
  rdf:type owl:Class ;
  rdfs:comment "Earth surface setting with geography defined by spatial relationship to glaciers (e.g. on top of a glacier, next to a glacier, in front of a glacier...). Processes related to moving ice dominate sediment transport and deposition and landform development. Includes subaqueous, shoreline, and terrestrial settings that are impacted by the presence of glaciers. Considered a geographically defined setting in that a glacier is a geographic feature."@en ;
  rdfs:comment "dct:source--  this vocabulary"@en ;
  rdfs:label "glacier related setting"@en ;
  rdfs:subClassOf gsen:Polar_Climatic_Setting ;
.
gsen:Glacier_Terminus_Setting
  rdf:type owl:Class ;
  rdfs:comment "Region of sediment deposition due to melting of glacier ice. ablation and flow till setting."@en ;
  rdfs:comment "dct:source--  NADM SLTTs, 2004"@en ;
  rdfs:label "glacier terminus setting"@en ;
  rdfs:subClassOf gsen:Proglacial_Setting ;
.
gsen:Hadal_Setting
  rdf:type owl:Class ;
  rdfs:comment "The deepest oceanic environment, i.e., over 6000 m in depth. Always in deep sea trench."@en ;
  rdfs:comment "dct:source--  Neuendorf et al., 2005"@en ;
  rdfs:label "hadal setting"@en ;
  rdfs:subClassOf gsen:Marine_Setting ;
.
gsen:High_Pressure_Low_Temperature_Earth_Interior_Setting
  rdf:type owl:Class ;
  rdfs:comment "High pressure environment characterized by geothermal gradient significantly lower than standard continental geotherm, enviornment in which blueschist facies metamorphic rocks form. Typically associated with subduction zones."@en ;
  rdfs:comment "dct:source--  this vocabulary"@en ;
  rdfs:label "high pressure low temperature earth interior setting"@en ;
  rdfs:subClassOf gsen:Planet_Interior_Setting ;
  rdfs:subClassOf [
      rdf:type owl:Restriction ;
      owl:onProperty gsoc:isStaticPartOf ;
      owl:someValuesFrom gsen:Planet_Interior_Setting ;
    ] ;
.
gsen:Hillslope_Setting
  rdf:type owl:Class ;
  rdfs:comment "Earth surface setting characterized by surface slope angles high enough that gravity alone becomes a significant factor in geomorphic development, as well as base-of-slope areas influenced by hillslope processes. Hillslope activities include creep, sliding, slumping, falling, and other downslope movements caused by slope collapse induced by gravitational influence on earth materials. May be subaerial or subaqueous."@en ;
  rdfs:comment "dct:source--  North American Geologic-map Data Model Science Language Technical Team, 2004, Sedimentary materials:science language for their classification, description, and interpretation in digital geologic-map databases, Version 1.0 (12/18/2004): U.S. Geological Survey Open-File Report 2004-1451 appendix C, 595 p., accessed at http://pubs.usgs.gov/of/2004/1451/sltt/appendixC/, Hawley, J.W., and Parsons, R.B. 1980. Glossary of selected geomorphic and geologic terms. Mimeo. USDA Soil Conservation Service, West National Technical Center, Portland, OR. 30 p."@en ;
  rdfs:label "hillslope setting"@en ;
  rdfs:subClassOf gsen:Planet_Surface_Setting ;
.
gsen:Hinterland_Setting
  rdf:type owl:Class ;
  rdfs:comment "Tectonic setting in the internal part of an orogenic belt, characterized by plastic deformation of rocks accompanied by significant metamorphism, typically involving crystalline basement rocks. Typically denotes the most structurally thickened part of an orogenic belt, between a magmatic arc or collision zone and a more 'external' foreland setting."@en ;
  rdfs:comment "dct:source--  this vocabulary"@en ;
  rdfs:label "hinterland tectonic setting"@en ;
  rdfs:subClassOf gsen:Tectonic_Setting ;
.
gsen:Hot_Spot_Setting
  rdf:type owl:Class ;
  rdfs:comment "Setting in a zone of high heat flow from the mantle. Typically identified in intraplate settings, but hot spot may also interact with active plate margins (Iceland...). Includes surface manifestations like volcanic center, but also includes crust and mantle manifestations as well."@en ;
  rdfs:comment "dct:source--  this vocabulary"@en ;
  rdfs:label "hot spot setting"@en ;
  rdfs:subClassOf gsen:Tectonic_Setting ;
.
gsen:Humid_Temperate_Climatic_Setting
  rdf:type owl:Class ;
  rdfs:comment "Setting with seasonal climate having hot to cold or humid to arid seasons."@en ;
  rdfs:comment "dct:source--  Cleland, D.T., Avers, P.E., McNab, W.H., Jensen, M.E., Bailey, R.G., King, T., Russell, W.E. 1997. National Hierarchical Framework of Ecological Units, in Boyce, M. S., Haney, A., ed., Ecosystem Management Applications for Sustainable Forest and WildlifeResources: Yale University Press, New Haven, CT. pp. 181-200."@en ;
  rdfs:label "humid temperate climatic setting"@en ;
  rdfs:subClassOf gsen:Planet_Surface_Setting ;
  rdfs:subClassOf [
      rdf:type owl:Restriction ;
      owl:onProperty gsoc:isStaticPartOf ;
      owl:someValuesFrom gsen:Planet_Surface_Setting ;
    ] ;
.
gsen:Humid_Tropical_Climatic_Setting
  rdf:type owl:Class ;
  rdfs:comment "Setting with hot humid climate influenced by equatorial air masses, no winter season."@en ;
  rdfs:comment "dct:source--  Cleland, D.T., Avers, P.E., McNab, W.H., Jensen, M.E., Bailey, R.G., King, T., Russell, W.E. 1997. National Hierarchical Framework of Ecological Units, in Boyce, M. S., Haney, A., ed., Ecosystem Management Applications for Sustainable Forest and WildlifeResources: Yale University Press, New Haven, CT. pp. 181-200."@en ;
  rdfs:label "humid tropical climatic setting"@en ;
  rdfs:subClassOf gsen:Planet_Surface_Setting ;
  rdfs:subClassOf [
      rdf:type owl:Restriction ;
      owl:onProperty gsoc:isStaticPartOf ;
      owl:someValuesFrom gsen:Planet_Surface_Setting ;
    ] ;
.
gsen:Hypabyssal_Setting
  rdf:type owl:Class ;
  rdfs:comment "Igneous environment close to the Earth's surface, characterized by more rapid cooling than plutonic setting to produce generally fine-grained intrusive igneous rock that is commonly associated with co-magmatic volcanic rocks."@en ;
  rdfs:comment "dct:source--  this vocabulary"@en ;
  rdfs:label "hypabyssal setting"@en ;
  rdfs:subClassOf gsen:Planet_Interior_Setting ;
  rdfs:subClassOf [
      rdf:type owl:Restriction ;
      owl:onProperty gsoc:isStaticPartOf ;
      owl:someValuesFrom gsen:Planet_Interior_Setting ;
    ] ;
.
gsen:Inactive_Spreading_Center_Setting
  rdf:type owl:Class ;
  rdfs:comment "Setting on oceanic crust formed at a spreading center that has been abandoned."@en ;
  rdfs:comment "dct:source--  This vocabulary"@en ;
  rdfs:label "inactive spreading center setting"@en ;
  rdfs:subClassOf gsen:Intraplate_Tectonic_Setting ;
  rdfs:subClassOf gsen:Plate_Spreading_Center_Setting ;
.
gsen:Inner_Neritic_Setting
  rdf:type owl:Class ;
  rdfs:comment "The ocean environment at depths between low tide level and 30 metres"@en ;
  rdfs:comment "dct:source--  this vocabulary"@en ;
  rdfs:label "inner neritic setting"@en ;
  rdfs:subClassOf gsen:Neritic_Setting ;
.
gsen:Interdistributary_Bay_Setting
  rdf:type owl:Class ;
  rdfs:comment "A pronounced indentation of the delta front between advancing stream distributaries, occupied by shallow water, and either open to the sea or partly enclosed by minor distributaries"@en ;
  rdfs:comment "dct:source--  Neuendorf et al., 2005"@en ;
  rdfs:label "interdistributary bay setting"@en ;
  rdfs:subClassOf gsen:Delta_System_Setting ;
  rdfs:subClassOf gsen:Subaqueous_Setting ;
  rdfs:subClassOf [
      rdf:type owl:Restriction ;
      owl:onProperty gsoc:isStaticPartOf ;
      owl:someValuesFrom gsen:Delta_System_Setting ;
    ] ;
.
gsen:Intertidal_Setting
  rdf:type owl:Class ;
  rdfs:comment "Pertaining to the benthic ocean environment or depth zone between high water and low water, also, pertaining to the organisms of that environment"@en ;
  rdfs:comment "dct:source--  Neuendorf et al., 2005"@en ;
  rdfs:label "intertidal setting"@en ;
  rdfs:subClassOf gsen:Subaqueous_Setting ;
  rdfs:subClassOf gsen:Tidal_Setting ;
  rdfs:subClassOf [
      rdf:type owl:Restriction ;
      owl:onProperty gsoc:isStaticPartOf ;
      owl:someValuesFrom gsen:Tidal_Setting ;
    ] ;
.
gsen:Intraplate_Tectonic_Setting
  rdf:type owl:Class ;
  rdfs:comment "Tectonically stable setting far from any active plate margins."@en ;
  rdfs:comment "dct:source--  This vocabulary"@en ;
  rdfs:label "intraplate tectonic setting"@en ;
  rdfs:subClassOf gsen:Tectonic_Setting ;
.
gsen:Lacustrine_Delta_Setting
  rdf:type owl:Class ;
  rdfs:comment "The low, nearly flat, alluvial tract of land at or near the mouth of a river, commonly forming a triangular or fan-shaped plain of considerable area, crossed by many distributaries of the main river, perhaps extending beyond the general trend of the lake shore, resulting from the accumulation of sediment supplied by the river in such quantities that it is not removed by waves or currents. Most deltas are partly subaerial and partly below water."@en ;
  rdfs:comment "dct:source--  Neuendorf et al., 2005"@en ;
  rdfs:label "lacustrine delta setting"@en ;
  rdfs:subClassOf gsen:Delta_System_Setting ;
  rdfs:subClassOf gsen:Lacustrine_Setting ;
  rdfs:subClassOf [
      rdf:type owl:Restriction ;
      owl:onProperty gsoc:isStaticPartOf ;
      owl:someValuesFrom gsen:Delta_System_Setting ;
    ] ;
.
gsen:Lacustrine_Setting
  rdf:type owl:Class ;
  rdfs:comment "Setting associated with a lake. Always overlaps with terrestrial, may overlap with subaerial, subaqueous, or shoreline."@en ;
  rdfs:comment "dct:source--  this vocabulary"@en ;
  rdfs:label "lacustrine setting"@en ;
  rdfs:subClassOf gsen:Terrestrial_Setting ;
.
gsen:Lagoonal_Setting
  rdf:type owl:Class ;
  rdfs:comment "A shallow stretch of salt or brackish water, partly or completely separated from a sea or lake by an offshore reef, barrier island, sand or spit (Jackson, 1997). Water is shallow, tidal and wave-produced effects on sediments, strong light reaches sediment.."@en ;
  rdfs:comment "dct:source--  generalize from Jackson 1997 and North American Geologic-map Data Model Science Language Technical Team, 2004, Sedimentary materials:science language for their classification, description, and interpretation in digital geologic-map databases, Version 1.0 (12/18/2004): U.S. Geological Survey Open-File Report 2004-1451 appendix C, 595 p., accessed at http://pubs.usgs.gov/of/2004/1451/sltt/appendixC/"@en ;
  rdfs:label "lagoonal setting"@en ;
  rdfs:subClassOf gsen:Shoreline_Setting ;
.
gsen:Low_Energy_Shoreline_Setting
  rdf:type owl:Class ;
  rdfs:comment "Settings characterized by very low surface slope and proximity to shoreline. Generally within peritidal setting, but characterized by low surface gradients and generally low-energy sedimentary processes."@en ;
  rdfs:comment "dct:source--  this vocabulary"@en ;
  rdfs:label "low energy shoreline setting"@en ;
  rdfs:subClassOf gsen:Shoreline_Setting ;
.
gsen:Low_Pressure_High_Temperature_Setting
  rdf:type owl:Class ;
  rdfs:comment "Setting characterized by temperatures significantly higher that those associated with normal continental geothermal gradient."@en ;
  rdfs:comment "dct:source--  this vocabulary"@en ;
  rdfs:label "low pressure high temperature setting"@en ;
  rdfs:subClassOf gsen:Planet_Interior_Setting ;
  rdfs:subClassOf [
      rdf:type owl:Restriction ;
      owl:onProperty gsoc:isStaticPartOf ;
      owl:someValuesFrom gsen:Planet_Interior_Setting ;
    ] ;
.
gsen:Lower_Bathyal_Setting
  rdf:type owl:Class ;
  rdfs:comment "The ocean environment at depths between 1000 and 3500 metres"@en ;
  rdfs:comment "dct:source--  Neuendorf, K.K.E., Mehl, J.P. & Jackson, J.A. (eds), 2005. Glossary of geology, 5th Edition. American Geological Institute, Alexandria, 779 p., Berggren, W.A. & Miller, K.G., 1989. Cenozoic bathyal and abyssal calcareous benthic foraminiferal zonation. Micropalaeontology 35, 308-320"@en ;
  rdfs:label "lower bathyal setting"@en ;
  rdfs:subClassOf gsen:Bathyal_Setting ;
.
gsen:Lower_Continental_Crust_Setting
  rdf:type owl:Class ;
  rdfs:comment "Continental crustal setting characterized by upper amphibolite to granulite facies metamorphism, insitu melting, residual anhydrous metamorphic rocks, and ductile flow of rock bodies."@en ;
  rdfs:comment "dct:source--  this vocabulary"@en ;
  rdfs:label "lower continental crustal setting"@en ;
  rdfs:subClassOf gsen:Continental_Crust_Setting ;
  rdfs:subClassOf [
      rdf:type owl:Restriction ;
      owl:onProperty gsoc:isStaticPartOf ;
      owl:someValuesFrom gsen:Continental_Crust_Setting ;
    ] ;
.
gsen:Lower_Delta_Plain_Setting
  rdf:type owl:Class ;
  rdfs:comment "The part of a delta plain which is penetrated by saline water and is subject to tidal processes"@en ;
  rdfs:comment "dct:source--  Readingh.G. & Collinson, J.D., 1996. Clastic coasts. 154-231 in Readingh.G. (ed.), Sedimentary Environments: Processses, Facies and Stratigraphy, third edition. Blackwell Science, Oxford"@en ;
  rdfs:label "lower delta plain setting"@en ;
  rdfs:subClassOf gsen:Delta_Plain_Setting ;
  rdfs:subClassOf gsen:Tidal_Setting ;
  rdfs:subClassOf [
      rdf:type owl:Restriction ;
      owl:onProperty gsoc:isStaticPartOf ;
      owl:someValuesFrom gsen:Delta_Plain_Setting ;
    ] ;
  rdfs:subClassOf [
      rdf:type owl:Restriction ;
      owl:onProperty gsoc:isStaticPartOf ;
      owl:someValuesFrom gsen:Tidal_Setting ;
    ] ;
.
gsen:Lower_Mantle_Setting
  rdf:type owl:Class ;
  rdfs:comment "That part of the mantle that lies below a depth of about 660 km. With increasing depth, density increases from ~4.4 g/cm3-to ~5.6 g/cm3, and velocity of compressional seismic waves increases from ~10.7 km/s to ~13.7 km/s (Dziewonski and Anderson, 1981)."@en ;
  rdfs:comment "dct:source--  Neuendorf et al., 2005"@en ;
  rdfs:label "lower mantle setting"@en ;
  rdfs:subClassOf gsen:Mantle_Setting ;
  rdfs:subClassOf [
      rdf:type owl:Restriction ;
      owl:onProperty gsoc:isStaticPartOf ;
      owl:someValuesFrom gsen:Mantle_Setting ;
    ] ;
.
gsen:Lower_Oceanic_Crust_Setting
  rdf:type owl:Class ;
  rdfs:comment "Setting characterized by dominantly intrusive mafic rocks, with sheeted dike complexes in upper part and gabbroic to ultramafic intrusive or metamorphic rocks in lower part."@en ;
  rdfs:comment "dct:source--  this vocabulary"@en ;
  rdfs:label "lower oceanic crustal setting"@en ;
  rdfs:subClassOf gsen:Oceanic_Crust_Setting ;
  rdfs:subClassOf [
      rdf:type owl:Restriction ;
      owl:onProperty gsoc:isStaticPartOf ;
      owl:someValuesFrom gsen:Oceanic_Crust_Setting ;
    ] ;
.
gsen:Mantle_Setting
  rdf:type owl:Class ;
  rdfs:comment "The zone of the Earth below the crust and above the core, which is divided into the upper mantle and the lower mantle, with a transition zone separating them."@en ;
  rdfs:comment "dct:source--  Neuendorf et al., 2005"@en ;
  rdfs:label "mantle setting"@en ;
  rdfs:subClassOf gsen:Planet_Interior_Setting ;
  rdfs:subClassOf gsen:Tectonic_Setting ;
  rdfs:subClassOf [
      rdf:type owl:Restriction ;
      owl:onProperty gsoc:isStaticPartOf ;
      owl:someValuesFrom gsen:Planet_Interior_Setting ;
    ] ;
.
gsen:Marginal_Marine_Sabkha_Setting
  rdf:type owl:Class ;
  rdfs:comment "Setting characterized by arid to semi-arid conditions on restricted coastal plains mostly above normal high tide level, with evaporite-saline mineral, tidal-flood, and eolian deposits. Boundaries with intertidal setting and non-tidal terrestrial setting are gradational. (Jackson, 1997, p. 561)."@en ;
  rdfs:comment "dct:source--  North American Geologic-map Data Model Science Language Technical Team, 2004, Sedimentary materials:science language for their classification, description, and interpretation in digital geologic-map databases, Version 1.0 (12/18/2004): U.S. Geological Survey Open-File Report 2004-1451 appendix C, 595 p., accessed at http://pubs.usgs.gov/of/2004/1451/sltt/appendixC/, based on Jackson 1997, Neuendorf et al. 2005"@en ;
  rdfs:label "marginal marine sabkha setting"@en ;
  rdfs:subClassOf gsen:Arid_Or_Semi_Arid_Environment_Setting ;
  rdfs:subClassOf gsen:Low_Energy_Shoreline_Setting ;
.
gsen:Marine_Carbonate_Platform_Setting
  rdf:type owl:Class ;
  rdfs:comment "A shallow submerged plateau separated from continental landmasses, on which high biological carbonate production rates produce enough sediment to maintain the platform surface near sea level. Grades into atoll as area becomes smaller and ringing coral reefs become more prominent part of the setting."@en ;
  rdfs:comment "dct:source--  this vocabulary"@en ;
  rdfs:label "marine carbonate platform setting"@en ;
  rdfs:subClassOf gsen:Marine_Setting ;
  rdfs:subClassOf [
      rdf:type owl:Restriction ;
      owl:onProperty gsoc:isStaticPartOf ;
      owl:someValuesFrom gsen:Marine_Setting ;
    ] ;
.
gsen:Marine_Setting
  rdf:type owl:Class ;
  rdfs:comment "Setting characterized by location under the surface of the sea."@en ;
  rdfs:comment "dct:source--  North American Geologic-map Data Model Science Language Technical Team, 2004, Sedimentary materials:science language for their classification, description, and interpretation in digital geologic-map databases, Version 1.0 (12/18/2004): U.S. Geological Survey Open-File Report 2004-1451 appendix C, 595 p., accessed at http://pubs.usgs.gov/of/2004/1451/sltt/appendixC/, Webster's Encyclopedic Unabridged Dictionary of the English Language, 2001, p. 1894."@en ;
  rdfs:label "marine setting"@en ;
  rdfs:subClassOf gsen:Planet_Surface_Setting ;
  rdfs:subClassOf [
      rdf:type owl:Restriction ;
      owl:onProperty gsoc:isStaticPartOf ;
      owl:someValuesFrom gsen:Planet_Surface_Setting ;
    ] ;
.
gsen:Meandering_Channel_Setting
  rdf:type owl:Class ;
  rdfs:comment "Produced by a mature stream swinging from side to side as it flows across its floodplain or shifts its course laterally toward the convex side of an original curve"@en ;
  rdfs:comment "dct:source--  Neuendorf et al., 2005"@en ;
  rdfs:label "meandering river channel setting"@en ;
  rdfs:subClassOf gsen:River_Channel_Setting ;
.
gsen:Medium_Spreading_Center_Setting
  rdf:type owl:Class ;
  rdfs:comment "Spreading center at which the opening rate is between 50 and 100 mm per year."@en ;
  rdfs:comment "dct:source--  Macdonald 1982"@en ;
  rdfs:label "medium rate spreading center setting"@en ;
  rdfs:subClassOf gsen:Active_Spreading_Center_Setting ;
.
gsen:Mid_Ocean_Ridge_Setting
  rdf:type owl:Class ;
  rdfs:comment "Ocean highland associated with a divergent continental margin (spreading center). Setting is characterized by active volcanism, locally steep reliefhydrothermal activity, and pelagic sedimentation."@en ;
  rdfs:comment "dct:source--  this vocabulary"@en ;
  rdfs:label "mid ocean ridge setting"@en ;
  rdfs:subClassOf gsen:Ocean_Highland_Setting ;
.
gsen:Middle_Bathyal_Setting
  rdf:type owl:Class ;
  rdfs:comment "The ocean environment at water depths between 600 and 1000 metres"@en ;
  rdfs:comment "dct:source--  Berggren, W.A. & Miller, K.G., 1989. Cenozoic bathyal and abyssal calcareous benthic foraminiferal zonation. Micropalaeontology 35, 308-320"@en ;
  rdfs:label "middle bathyal setting"@en ;
  rdfs:subClassOf gsen:Bathyal_Setting ;
.
gsen:Middle_Continental_Crust_Setting
  rdf:type owl:Class ;
  rdfs:comment "Continental crustal setting characterized by greenschist to upper amphibolite facies metamorphism, plutonic igneous rocks, and ductile deformation."@en ;
  rdfs:comment "dct:source--  this vocabulary"@en ;
  rdfs:label "middle continental crust setting"@en ;
  rdfs:subClassOf gsen:Continental_Crust_Setting ;
  rdfs:subClassOf [
      rdf:type owl:Restriction ;
      owl:onProperty gsoc:isStaticPartOf ;
      owl:someValuesFrom gsen:Continental_Crust_Setting ;
    ] ;
.
gsen:Middle_Neritic_Setting
  rdf:type owl:Class ;
  rdfs:comment "The ocean environment at depths between 30 and 100 metres"@en ;
  rdfs:comment "dct:source--  this vocabulary"@en ;
  rdfs:label "middle neritic setting"@en ;
  rdfs:subClassOf gsen:Neritic_Setting ;
.
gsen:Mud_Flat_Setting
  rdf:type owl:Class ;
  rdfs:comment "A relatively level area of fine grained material (e.g. silt) along a shore (as in a sheltered estuary or chenier-plain) or around an island, alternately covered and uncovered by the tide or covered by shallow water, and barren of vegetation. Includes most tidal flats, but lacks denotation of tidal influence.."@en ;
  rdfs:comment "dct:source--  North American Geologic-map Data Model Science Language Technical Team, 2004, Sedimentary materials:science language for their classification, description, and interpretation in digital geologic-map databases, Version 1.0 (12/18/2004): U.S. Geological Survey Open-File Report 2004-1451 appendix C, 595 p., accessed at http://pubs.usgs.gov/of/2004/1451/sltt/appendixC/, Jackson, 1997"@en ;
  rdfs:label "mud flat setting"@en ;
  rdfs:subClassOf gsen:Low_Energy_Shoreline_Setting ;
.
gsen:Neritic_Setting
  rdf:type owl:Class ;
  rdfs:comment "The ocean environment at depths between low-tide level and 200 metres, or between low-tide level and approximately the edge of the continental shelf"@en ;
  rdfs:comment "dct:source--  Neuendorf et al., 2005"@en ;
  rdfs:label "neritic setting"@en ;
  rdfs:subClassOf gsen:Marine_Setting ;
  rdfs:subClassOf [
      rdf:type owl:Restriction ;
      owl:onProperty gsoc:hasStaticPart ;
      owl:someValuesFrom gsen:Inner_Neritic_Setting ;
    ] ;
  rdfs:subClassOf [
      rdf:type owl:Restriction ;
      owl:onProperty gsoc:hasStaticPart ;
      owl:someValuesFrom gsen:Middle_Neritic_Setting ;
    ] ;
  rdfs:subClassOf [
      rdf:type owl:Restriction ;
      owl:onProperty gsoc:hasStaticPart ;
      owl:someValuesFrom gsen:Outer_Neritic_Setting ;
    ] ;
.
gsen:Ocean_Highland_Setting
  rdf:type owl:Class ;
  rdfs:comment "Broad category for subaqueous marine settings characterized by significant relief above adjacent sea floor."@en ;
  rdfs:comment "dct:source--  this vocabulary"@en ;
  rdfs:label "ocean highland setting"@en ;
  rdfs:subClassOf gsen:Marine_Setting ;
  rdfs:subClassOf [
      rdf:type owl:Restriction ;
      owl:onProperty gsoc:isStaticPartOf ;
      owl:someValuesFrom gsen:Marine_Setting ;
    ] ;
.
gsen:Oceanic_Crust_Setting
  rdf:type owl:Class ;
  rdfs:comment "That type of the Earth's crust which underlies the ocean basins. The oceanic crust is 5-10 km thick, it has a density of 2.9 g/cm3, and compressional seismic-wave velocities travelling through it at 4-7.2 km/sec. Setting in crust produced by submarine volcanism at a mid ocean ridge."@en ;
  rdfs:comment "dct:source--  Neuendorf et al., 2005"@en ;
  rdfs:label "oceanic crustal setting"@en ;
  rdfs:subClassOf gsen:Crustal_Setting ;
.
gsen:Oceanic_Plateau_Setting
  rdf:type owl:Class ;
  rdfs:comment "Region of elevated ocean crust that commonly rises to within 2-3 km of the surface above an abyssal sea floor that lies several km deeper. Climate and water depths are such that a marine carbonate platform does not develop."@en ;
  rdfs:comment "dct:source--  Reading 1978"@en ;
  rdfs:label "oceanic plateau setting"@en ;
  rdfs:subClassOf gsen:Ocean_Highland_Setting ;
.
gsen:Outer_Neritic_Setting
  rdf:type owl:Class ;
  rdfs:comment "The ocean environment at depths between 100 and 200 metres or between low-tide level and approximately the edge of the continental shelf"@en ;
  rdfs:comment "dct:source--  this vocabulary"@en ;
  rdfs:label "outer neritic setting"@en ;
  rdfs:subClassOf gsen:Neritic_Setting ;
.
gsen:Passive_Continental_Margin_Setting
  rdf:type owl:Class ;
  rdfs:comment "Boundary of continental crust into oceanic crust of an oceanic basin that is not a subduction zone or transform fault system. Generally is rifted margin formed when ocean basin was initially formed."@en ;
  rdfs:comment "dct:source--  This vocabulary"@en ;
  rdfs:label "passive continental margin setting"@en ;
  rdfs:subClassOf gsen:Tectonic_Setting ;
.
gsen:Pediment_Setting
  rdf:type owl:Class ;
  rdfs:comment "A gently sloping erosional surface developed at the foot of a receding hill or mountain slope. The surface may be essentially bare, exposing earth material that extends beneath adjacent uplands, or it may be thinly mantled with alluvium and colluvium, ultimately in transit from upland front to basin or valley lowland. In hill-foot slope terrain the mantle is designated \\pedisediment.\\ The term has been used in several geomorphic contexts: Pediments may be classed with respect to (a) landscape positions, for example, intermontane-basin piedmont or valley-border footslope surfaces (respectively, apron and terrace pediments (Cooke and Warren, 1973)), (b) type of material eroded, bedrock or regolith, or (c) combinations of the above. Compare - Piedmont slope.."@en ;
  rdfs:comment "dct:source--  North American Geologic-map Data Model Science Language Technical Team, 2004, Sedimentary materials:science language for their classification, description, and interpretation in digital geologic-map databases, Version 1.0 (12/18/2004): U.S. Geological Survey Open-File Report 2004-1451 appendix C, 595 p., accessed at http://pubs.usgs.gov/of/2004/1451/sltt/appendixC/, NRCS, 2001"@en ;
  rdfs:label "pediment setting"@en ;
  rdfs:subClassOf gsen:Piedmont_Slope_System_Setting ;
  rdfs:subClassOf [
      rdf:type owl:Restriction ;
      owl:onProperty gsoc:isStaticPartOf ;
      owl:someValuesFrom gsen:Piedmont_Slope_System_Setting ;
    ] ;
.
gsen:Piedmont_Slope_System_Setting
  rdf:type owl:Class ;
  rdfs:comment "Location on gentle slope at the foot of a mountain, generally used in terms of intermontane-basin terrain. Main components include: (a) An erosional surface on bedrock adjacent to the receding mountain front (pediment, rock pediment), (b) A constructional surface comprising individual alluvial fans and interfan valleys, also near the mountain front, and (c) A distal complex of coalescent fans (bajada), and alluvial slopes without fan form. Piedmont slopes grade to basin-floor depressions with alluvial and temporary lake plains or to surfaces associated with through drainage."@en ;
  rdfs:comment "dct:source--  Hawley and Parsons, 1980+F98"@en ;
  rdfs:label "piedmont slope system setting"@en ;
  rdfs:subClassOf gsen:Subaerial_Setting ;
  rdfs:subClassOf gsen:Terrestrial_Setting ;
.
gsen:Planet_Interior_Setting
  rdf:type owl:Class ;
  rdfs:comment "Geologic environments within the solid Earth."@en ;
  rdfs:comment "dct:source--  this vocabulary"@en ;
  rdfs:label "earth interior setting"@en ;
  rdfs:subClassOf gsoc:Setting ;
  owl:disjointWith gsen:Planet_Surface_Setting ;
.
gsen:Planet_Surface_Setting
  rdf:type owl:Class ;
  rdfs:comment "Geologic environments on all or part of the surface of the solid Earth. Based on an assumption that a particular setting may be specified by a combination of climatic, process or geomorpologic settings."@en ;
  rdfs:comment "dct:source--  this vocabulary"@en ;
  rdfs:label "earth surface setting"@en ;
  rdfs:subClassOf gsoc:Setting ;
  owl:disjointWith gsen:Planet_Interior_Setting ;
.
gsen:Plate_Margin_Setting
  rdf:type owl:Class ;
  rdfs:comment "Tectonic setting at the boundary between two tectonic plates."@en ;
  rdfs:comment "dct:source--  This vocabulary"@en ;
  rdfs:label "plate margin setting"@en ;
  rdfs:subClassOf gsen:Tectonic_Setting ;
.
gsen:Plate_Spreading_Center_Setting
  rdf:type owl:Class ;
  rdfs:comment "Tectonic setting where new oceanic crust is being or has been formed at a divergent plate boundary. Includes active and inactive spreading centers."@en ;
  rdfs:comment "dct:source--  this vocabulary"@en ;
  rdfs:label "plate spreading center setting"@en ;
  rdfs:subClassOf gsen:Tectonic_Setting ;
.
gsen:Playa_Setting
  rdf:type owl:Class ;
  rdfs:comment "The usually dry and nearly level plain that occupies the lowest parts of closed depressions, such as those occurring on intermontane basin floors. Temporary flooding occurs primarily in response to precipitation-runoff events."@en ;
  rdfs:comment "dct:source--  Based on Hawley and Parsons, 1980"@en ;
  rdfs:label "playa setting"@en ;
  rdfs:subClassOf gsen:Arid_Or_Semi_Arid_Environment_Setting ;
  rdfs:subClassOf gsen:Subaerial_Setting ;
  rdfs:subClassOf gsen:Terrestrial_Setting ;
.
gsen:Polar_Climatic_Setting
  rdf:type owl:Class ;
  rdfs:comment "Setting with climate dominated by temperatures below the freezing temperature of water. Includes polar deserts because precipitation is generally scant at high latitude. Climate controlled by arctic air masses, cold dry environment with short summer."@en ;
  rdfs:comment "dct:source--  Cleland, D.T., Avers, P.E., McNab, W.H., Jensen, M.E., Bailey, R.G., King, T., Russell, W.E. 1997. National Hierarchical Framework of Ecological Units, in Boyce, M. S., Haney, A., ed., Ecosystem Management Applications for Sustainable Forest and WildlifeResources: Yale University Press, New Haven, CT. pp. 181-200."@en ;
  rdfs:label "polar climatic setting"@en ;
  rdfs:subClassOf gsen:Planet_Surface_Setting ;
  rdfs:subClassOf [
      rdf:type owl:Restriction ;
      owl:onProperty gsoc:isStaticPartOf ;
      owl:someValuesFrom gsen:Planet_Surface_Setting ;
    ] ;
.
gsen:Prodelta_Setting
  rdf:type owl:Class ;
  rdfs:comment "The part of a delta that is below the effective depth of wave erosion, lying beyond the delta front, and sloping gently down to the floor of the basin into which the delta is advancing and where clastic river sediment ceases to be a significant part of the basin-floor deposits, it is entirely below the water level"@en ;
  rdfs:comment "dct:source--  Neuendorf et al., 2005"@en ;
  rdfs:label "prodelta setting"@en ;
  rdfs:subClassOf gsen:Delta_System_Setting ;
  rdfs:subClassOf gsen:Subaqueous_Setting ;
  rdfs:subClassOf [
      rdf:type owl:Restriction ;
      owl:onProperty gsoc:isStaticPartOf ;
      owl:someValuesFrom gsen:Delta_System_Setting ;
    ] ;
.
gsen:Proglacial_Setting
  rdf:type owl:Class ;
  rdfs:comment "Immediately in front of or just beyond the outer limits of a glacier or ice sheet, generally at or near its lower end, said of lakes, streams, deposits, and other features produced by or derived from the glacier ice"@en ;
  rdfs:comment "dct:source--  Neuendorf et al., 2005"@en ;
  rdfs:label "proglacial setting"@en ;
  rdfs:subClassOf gsen:Glacier_Related_Setting ;
  rdfs:subClassOf [
      rdf:type owl:Restriction ;
      owl:onProperty gsoc:isStaticPartOf ;
      owl:someValuesFrom gsen:Glacier_Related_Setting ;
    ] ;
.
gsen:Reef_Flat_Setting
  rdf:type owl:Class ;
  rdfs:comment "A stony platform of reef rock, landward of the reef crest at or above the low tide level, occasionally with patches of living coral and associated organisms, and commonly strewn with coral fragments and coral sand. It may include shallow pools, irregular gullies, low islands of sand or rubble (often vegetated, esp. by palms), and scattered colonies of the more hardy species of coral"@en ;
  rdfs:comment "dct:source--  Neuendorf et al., 2005"@en ;
  rdfs:label "reef flat setting"@en ;
  rdfs:subClassOf gsen:Biological_Reef_Setting ;
.
gsen:Regional_Metamorphic_Origin_Setting
  rdf:type owl:Class ;
  rdfs:comment "Metamorphism not obviously localized along contacts of igneous bodies, includes burial metamorphism and ocean ridge metamorphism"@en ;
  rdfs:comment "dct:source--  NADM metamorphic rock vocabulary SLTTm1.0, 2004"@en ;
  rdfs:label "regional metamorphic setting"@en ;
  rdfs:subClassOf gsen:Planet_Interior_Setting ;
  rdfs:subClassOf [
      rdf:type owl:Restriction ;
      owl:onProperty gsoc:isStaticPartOf ;
      owl:someValuesFrom gsen:Planet_Interior_Setting ;
    ] ;
.
gsen:River_Channel_Setting
  rdf:type owl:Class ;
  rdfs:comment "The bed where a natural body of surface water flows or may flow, a natural passageway or depression of perceptible extent containing continuously or periodically flowing water, or forming a connecting link between two bodies of water, a watercourse"@en ;
  rdfs:comment "dct:source--  Neuendorf et al., 2005"@en ;
  rdfs:label "river channel setting"@en ;
  rdfs:subClassOf gsen:River_Plain_System_Setting ;
  owl:equivalentClass [
      rdf:type owl:Restriction ;
      owl:onProperty gsoc:isStaticPartOf ;
      owl:someValuesFrom gsen:River_Plain_System_Setting ;
    ] ;
.
gsen:River_Plain_System_Setting
  rdf:type owl:Class ;
  rdfs:comment "Geologic setting dominated by a river system, river plains may occur in any climatic setting. Includes active channels, abandoned channels, levees, oxbow lakes, flood plain. May be part of an alluvial plain that includes terraces composed of abandoned river plain deposits."@en ;
  rdfs:comment "dct:source--  this vocabulary"@en ;
  rdfs:label "river plain system setting"@en ;
  rdfs:subClassOf gsen:Subaerial_Setting ;
  rdfs:subClassOf gsen:Terrestrial_Setting ;
.
gsen:Rocky_Coast_Setting
  rdf:type owl:Class ;
  rdfs:comment "Shoreline with significant relief and abundant rock outcrop."@en ;
  rdfs:comment "dct:source--  North American Geologic-map Data Model Science Language Technical Team, 2004, Sedimentary materials:science language for their classification, description, and interpretation in digital geologic-map databases, Version 1.0 (12/18/2004): U.S. Geological Survey Open-File Report 2004-1451 appendix C, 595 p., accessed at http://pubs.usgs.gov/of/2004/1451/sltt/appendixC/"@en ;
  rdfs:label "rocky coast setting"@en ;
  rdfs:subClassOf gsen:Shoreline_Setting ;
.
gsen:Sand_Plain_Setting
  rdf:type owl:Class ;
  rdfs:comment "A sand-covered plain dominated by aeolian processes."@en ;
  rdfs:comment "dct:source--  Neuendorf et al., 2005"@en ;
  rdfs:label "sand plain setting"@en ;
  rdfs:subClassOf gsen:Aeolian_Process_Setting ;
  rdfs:subClassOf gsen:Arid_Or_Semi_Arid_Environment_Setting ;
  rdfs:subClassOf gsen:Terrestrial_Setting ;
.
gsen:Seamount_Setting
  rdf:type owl:Class ;
  rdfs:comment "Setting that consists of a conical mountain on the ocean floor (guyot). Typically characterized by active volcanism, pelagic sedimentation. If the mountain is high enough to reach the photic zone, carbonate production may result in reef building to produce a carbonate platform or atoll setting."@en ;
  rdfs:comment "dct:source--  Reading 1978"@en ;
  rdfs:label "seamount setting"@en ;
  rdfs:subClassOf gsen:Intraplate_Tectonic_Setting ;
  rdfs:subClassOf gsen:Ocean_Highland_Setting ;
.
gsen:Shoreline_Setting
  rdf:type owl:Class ;
  rdfs:comment "Geologic settings characterized by location adjacent to the ocean or a lake. A zone of indefinite width (may be many kilometers), bordering a body of water that extends from the water line inland to the first major change in landform features. Includes settings that may be subaerial, intermittently subaqueous, or shallow subaqueous, but are intrinsically associated with the interface between land areas and water bodies."@en ;
  rdfs:comment "dct:source--  based on Neuendorf et al, 2005"@en ;
  rdfs:label "shoreline settings"@en ;
  rdfs:subClassOf gsen:Planet_Surface_Setting ;
  rdfs:subClassOf [
      rdf:type owl:Restriction ;
      owl:onProperty gsoc:isStaticPartOf ;
      owl:someValuesFrom gsen:Planet_Surface_Setting ;
    ] ;
.
gsen:Slope_Rise_Setting
  rdf:type owl:Class ;
  rdfs:comment "The part of a subaqueous basin that is between a bordering shelf setting, which separate the basin from an adjacent landmass, and a very low-relief basin plain setting."@en ;
  rdfs:comment "dct:source--  based on NADM SLTTs, 2004"@en ;
  rdfs:label "slope rise setting"@en ;
  rdfs:subClassOf gsen:Marine_Setting ;
  rdfs:subClassOf [
      rdf:type owl:Restriction ;
      owl:onProperty gsoc:isStaticPartOf ;
      owl:someValuesFrom gsen:Marine_Setting ;
    ] ;
.
gsen:Slow_Spreading_Center_Setting
  rdf:type owl:Class ;
  rdfs:comment "Spreading center at which the opening rate is less than 50 mm per year."@en ;
  rdfs:comment "dct:source--  Macdonald 1982"@en ;
  rdfs:label "slow spreading center setting"@en ;
  rdfs:subClassOf gsen:Active_Spreading_Center_Setting ;
.
gsen:Strandplain_Setting
  rdf:type owl:Class ;
  rdfs:comment "A prograded shore built seaward by waves and currents, and continuous for some distance along the coast. It is characterized by subparallel beach ridges and swales, in places with associated dunes."@en ;
  rdfs:comment "dct:source--  based on Jackson 1997, p. 626"@en ;
  rdfs:label "strandplain setting"@en ;
  rdfs:subClassOf gsen:Shoreline_Setting ;
  rdfs:subClassOf gsen:Subaerial_Setting ;
.
gsen:Subaerial_Setting
  rdf:type owl:Class ;
  rdfs:comment "Setting at the interface between the solid earth and the atmosphere, includes some shallow subaqueous settings in river channels and playas. Characterized by conditions and processes, such as erosion, that exist or operate in the open air on or immediately adjacent to the land surface"@en ;
  rdfs:comment "dct:source--  Neuendorf et al., 2005"@en ;
  rdfs:label "subaerial setting"@en ;
  rdfs:subClassOf gsen:Planet_Surface_Setting ;
  rdfs:subClassOf [
      rdf:type owl:Restriction ;
      owl:onProperty gsoc:isStaticPartOf ;
      owl:someValuesFrom gsen:Planet_Surface_Setting ;
    ] ;
.
gsen:Subaqueous_Setting
  rdf:type owl:Class ;
  rdfs:comment "Setting situated in or under permanent, standing water. Used for marine and lacustrine settings, but not for fluvial settings."@en ;
  rdfs:comment "dct:source--  based on North American Geologic-map Data Model Science Language Technical Team, 2004, Sedimentary materials:science language for their classification, description, and interpretation in digital geologic-map databases, Version 1.0 (12/18/2004): U.S. Geological Survey Open-File Report 2004-1451 appendix C, 595 p., accessed at http://pubs.usgs.gov/of/2004/1451/sltt/appendixC/,"@en ;
  rdfs:label "subaqueous setting"@en ;
  rdfs:subClassOf gsen:Planet_Surface_Setting ;
  rdfs:subClassOf [
      rdf:type owl:Restriction ;
      owl:onProperty gsoc:isStaticPartOf ;
      owl:someValuesFrom gsen:Planet_Surface_Setting ;
    ] ;
.
gsen:Subduction_Zone_Setting
  rdf:type owl:Class ;
  rdfs:comment "Tectonic setting at which a tectonic plate, usually oceanic, is moving down into the mantle beneath another overriding plate."@en ;
  rdfs:label "subduction zone setting"@en ;
  rdfs:subClassOf gsen:Plate_Margin_Setting ;
.
gsen:Subglacial_Setting
  rdf:type owl:Class ;
  rdfs:comment "Formed or accumulated in or by the bottom parts of a glacier or ice sheet, said of meltwater streams, till, moraine, etc."@en ;
  rdfs:comment "dct:source--  Neuendorf et al., 2005"@en ;
  rdfs:label "subglacial setting"@en ;
  rdfs:subClassOf gsen:Glacier_Related_Setting ;
  rdfs:subClassOf [
      rdf:type owl:Restriction ;
      owl:onProperty gsoc:isStaticPartOf ;
      owl:someValuesFrom gsen:Glacier_Related_Setting ;
    ] ;
.
gsen:Submarine_Fan_Setting
  rdf:type owl:Class ;
  rdfs:comment "Large fan-shaped cones of sediment on the ocean floor, generally associated with submarine canyons that provide sediment supply to build the fan.."@en ;
  rdfs:comment "dct:source--  this vocabulary"@en ;
  rdfs:label "submarine fan setting"@en ;
  rdfs:subClassOf gsen:Marine_Setting ;
  rdfs:subClassOf [
      rdf:type owl:Restriction ;
      owl:onProperty gsoc:isStaticPartOf ;
      owl:someValuesFrom gsen:Marine_Setting ;
    ] ;
.
gsen:Supraglacial_Setting
  rdf:type owl:Class ;
  rdfs:comment "Carried upon, deposited from, or pertaining to the top surface of a glacier or ice sheet, said of meltwater streams, till, drift, etc. (Jackson, 1997, p. 639). Dreimanis (1988, p. 39) recommendation that \\supraglacial\\ supersede \\superglacial\\ is followed."@en ;
  rdfs:comment "dct:source--  North American Geologic-map Data Model Science Language Technical Team, 2004, Sedimentary materials:science language for their classification, description, and interpretation in digital geologic-map databases, Version 1.0 (12/18/2004): U.S. Geological Survey Open-File Report 2004-1451 appendix C, 595 p., accessed at http://pubs.usgs.gov/of/2004/1451/sltt/appendixC/"@en ;
  rdfs:label "supraglacial setting"@en ;
  rdfs:subClassOf gsen:Glacier_Related_Setting ;
  rdfs:subClassOf [
      rdf:type owl:Restriction ;
      owl:onProperty gsoc:isStaticPartOf ;
      owl:someValuesFrom gsen:Glacier_Related_Setting ;
    ] ;
.
gsen:Supratidal_Setting
  rdf:type owl:Class ;
  rdfs:comment "Pertaining to the shore area marginal to the littoral zone, just above high-tide level"@en ;
  rdfs:comment "dct:source--  Neuendorf et al., 2005"@en ;
  rdfs:label "supratidal setting"@en ;
  rdfs:subClassOf gsen:Shoreline_Setting ;
  rdfs:subClassOf gsen:Subaerial_Setting ;
.
gsen:Swamp_Or_Marsh_Setting
  rdf:type owl:Class ;
  rdfs:comment "A water-saturated, periodically wet or continually flooded area with the surface not deeply submerged, essentially without the formation of peat. Marshes are characterized by sedges, cattails, rushes, or other aquatic and grasslike vegetation. Swamps are characterized by tree and brush vegetation."@en ;
  rdfs:comment "dct:source--  Neuendorf et al 2005, Soil Science Society of America, 1997."@en ;
  rdfs:label "swamp or marsh setting"@en ;
  rdfs:subClassOf gsen:Wetland_Setting ;
.
gsen:Tectonic_Setting
  rdf:type owl:Class ;
  rdfs:comment "Setting defined by relationships to tectonic plates on or in the Earth."@en ;
  rdfs:comment "dct:source--  This vocabulary"@en ;
  rdfs:label "tectonically defined setting"@en ;
  rdfs:subClassOf gsoc:Setting ;
  rdfs:subClassOf [
      rdf:type owl:Restriction ;
      owl:onProperty gsoc:hasStaticPart ;
      owl:someValuesFrom gspr:Tectonic_Process ;
    ] ;
.
gsen:Terrestrial_Setting
  rdf:type owl:Class ;
  rdfs:comment "Setting characterized by absence of direct marine influence. Most of the subaerial settings are also terrestrial, but lacustrine settings, while terrestrial, are not subaerial, so the subaerial settings are not included as subcategories."@en ;
  rdfs:comment "dct:source--  this vocabulary"@en ;
  rdfs:label "terrestrial setting"@en ;
  rdfs:subClassOf gsen:Planet_Surface_Setting ;
  rdfs:subClassOf [
      rdf:type owl:Restriction ;
      owl:onProperty gsoc:isStaticPartOf ;
      owl:someValuesFrom gsen:Planet_Surface_Setting ;
    ] ;
.
gsen:Tidal_Channel_Setting
  rdf:type owl:Class ;
  rdfs:comment "A major channel followed by the tidal currents, extending from offshore into a tidal marsh or a tidal flat."@en ;
  rdfs:comment "dct:source--  Neuendorf et al., 2005"@en ;
  rdfs:label "tidal channel setting"@en ;
  rdfs:subClassOf gsen:Subaqueous_Setting ;
  rdfs:subClassOf gsen:Tidal_Setting ;
  rdfs:subClassOf [
      rdf:type owl:Restriction ;
      owl:onProperty gsoc:isStaticPartOf ;
      owl:someValuesFrom gsen:Tidal_Setting ;
    ] ;
.
gsen:Tidal_Flat_Setting
  rdf:type owl:Class ;
  rdfs:comment "An extensive, nearly horizontal, barren tract of land that is alternately covered and uncovered by the tide, and consisting of unconsolidated sediment (mostly mud and sand). It may form the top surface of a deltaic deposit."@en ;
  rdfs:comment "dct:source--  Neuendorf et al., 2005"@en ;
  rdfs:label "tidal flat setting"@en ;
  rdfs:subClassOf gsen:Tidal_Setting ;
  rdfs:subClassOf [
      rdf:type owl:Restriction ;
      owl:onProperty gsoc:isStaticPartOf ;
      owl:someValuesFrom gsen:Tidal_Setting ;
    ] ;
.
gsen:Tidal_Marsh
  rdf:type owl:Class ;
  rdfs:comment "A marsh bordering a coast (as in a shallow lagoon or sheltered bay), formed of mud and of the resistant mat of roots of salt-tolerant plants, and regularly inundated during high tides, a marshy tidal flat."@en ;
  rdfs:comment "dct:source--  Neuendorf et al., 2005"@en ;
  rdfs:label "tidal marsh setting"@en ;
  rdfs:subClassOf gsen:Swamp_Or_Marsh_Setting ;
  rdfs:subClassOf gsen:Tidal_Flat_Setting ;
.
gsen:Tidal_Setting
  rdf:type owl:Class ;
  rdfs:comment "Setting subject to tidal processes"@en ;
  rdfs:comment "dct:source--  this vocabulary"@en ;
  rdfs:label "tidal setting"@en ;
  rdfs:subClassOf gsen:Shoreline_Setting ;
.
gsen:Transform_Plate_Boundary_Setting
  rdf:type owl:Class ;
  rdfs:comment "Plate boundary at which the adjacent plates are moving laterally relative to each other."@en ;
  rdfs:comment "dct:source--  This vocabulary"@en ;
  rdfs:label "transform plate boundary setting"@en ;
  rdfs:subClassOf gsen:Plate_Margin_Setting ;
.
gsen:Transitional_Crust_Setting
  rdf:type owl:Class ;
  rdfs:comment "Crust formed in the transition zone between continental and oceanic crust, during the history of continental rifting that culminates in the formation of a new ocean."@en ;
  rdfs:comment "dct:source--  Neuendorf et al., 2005"@en ;
  rdfs:label "transitional crustal setting"@en ;
  rdfs:subClassOf gsen:Crustal_Setting ;
.
gsen:Ultra_High_Pressure_Crustal_Setting
  rdf:type owl:Class ;
  rdfs:comment "Setting characterized by pressures characteristic of upper mantle, but indicated by mineral assemblage in crustal composition rocks."@en ;
  rdfs:comment "dct:source--  this vocabulary"@en ;
  rdfs:label "ultra high pressure crustal setting"@en ;
  rdfs:subClassOf gsen:Planet_Interior_Setting ;
  rdfs:subClassOf [
      rdf:type owl:Restriction ;
      owl:onProperty gsoc:isStaticPartOf ;
      owl:someValuesFrom gsen:Planet_Interior_Setting ;
    ] ;
.
gsen:Upper_Bathyal_Setting
  rdf:type owl:Class ;
  rdfs:comment "The ocean environment at water depths between 200 and 600 metres"@en ;
  rdfs:comment "dct:source--  Berggren, W.A. & Miller, K.G., 1989. Cenozoic bathyal and abyssal calcareous benthic foraminiferal zonation. Micropalaeontology 35, 308-320"@en ;
  rdfs:label "upper bathyal setting"@en ;
  rdfs:subClassOf gsen:Bathyal_Setting ;
.
gsen:Upper_Continental_Crust_Setting
  rdf:type owl:Class ;
  rdfs:comment "Continental crustal setting dominated by non metamorphosed to low greenschist facies metamorphic rocks, and brittle deformation."@en ;
  rdfs:comment "dct:source--  this vocabulary"@en ;
  rdfs:label "upper continental crustal setting"@en ;
  rdfs:subClassOf gsen:Continental_Crust_Setting ;
  rdfs:subClassOf [
      rdf:type owl:Restriction ;
      owl:onProperty gsoc:isStaticPartOf ;
      owl:someValuesFrom gsen:Continental_Crust_Setting ;
    ] ;
.
gsen:Upper_Delta_Plain_Setting
  rdf:type owl:Class ;
  rdfs:comment "The part of a delta plain essentially unaffected by basinal processes. They do not differ substantially from alluvial environments except that areas of swamp, marsh and lakes are usually more widespread and channels may bifurcate downstream"@en ;
  rdfs:comment "dct:source--  Readingh.G. & Collinson, J.D., 1996. Clastic coasts. 154-231 in Readingh.G. (ed.), Sedimentary Environments: Processses, Facies and Stratigraphy, third edition. Blackwell Science, Oxford"@en ;
  rdfs:label "upper delta plain setting"@en ;
  rdfs:subClassOf gsen:Delta_Plain_Setting ;
  rdfs:subClassOf gsen:Terrestrial_Setting ;
  rdfs:subClassOf [
      rdf:type owl:Restriction ;
      owl:onProperty gsoc:isStaticPartOf ;
      owl:someValuesFrom gsen:Delta_Plain_Setting ;
    ] ;
.
gsen:Upper_Mantle_Setting
  rdf:type owl:Class ;
  rdfs:comment "That part of the mantle which lies above a depth of about 660 km and has a density of 3.4 g/cm3 to 4.0 g/cm3 with increasing depth. Similarly, P-wave velocity increases from about 8 to 11 km/sec with depth and S wave velocity increases from about 4.5 to 6 km/sec with depth. It is presumed to be peridotitic in composition. It includes the subcrustal lithosphere the asthenosphere and the transition zone,"@en ;
  rdfs:comment "dct:source--  Neuendorf et al., 2005"@en ;
  rdfs:label "upper mantle setting"@en ;
  rdfs:subClassOf gsen:Mantle_Setting ;
  rdfs:subClassOf [
      rdf:type owl:Restriction ;
      owl:onProperty gsoc:isStaticPartOf ;
      owl:someValuesFrom gsen:Mantle_Setting ;
    ] ;
.
gsen:Upper_Oceanic_Crust_Setting
  rdf:type owl:Class ;
  rdfs:comment "Oceanic crustal setting dominated by extrusive rocks, abyssal oceanic sediment, with increasing mafic intrusive rock in lower part."@en ;
  rdfs:comment "dct:source--  this vocabulary"@en ;
  rdfs:label "upper oceanic crustal setting"@en ;
  rdfs:subClassOf gsen:Oceanic_Crust_Setting ;
  rdfs:subClassOf [
      rdf:type owl:Restriction ;
      owl:onProperty gsoc:isStaticPartOf ;
      owl:someValuesFrom gsen:Oceanic_Crust_Setting ;
    ] ;
.
gsen:Volcanic_Arc_Setting
  rdf:type owl:Class ;
  rdfs:comment "A generally curvillinear belt of volcanoes above a subduction zone."@en ;
  rdfs:comment "dct:source--  1-GE WP3, Neuendorf et al.(2005), p. 710"@en ;
  rdfs:label "volcanic arc setting"@en ;
  rdfs:subClassOf gsen:Plate_Margin_Setting ;
.
gsen:Wetland_Setting
  rdf:type owl:Class ;
  rdfs:comment "Setting characterized by gentle surface slope, and at least intermittent presence of standing water, which may be fresh, brackish, or saline. Wetland may be terrestrial setting or shoreline setting."@en ;
  rdfs:comment "dct:source--  this vocabulary"@en ;
  rdfs:label "wetland setting"@en ;
  rdfs:subClassOf gsen:Planet_Surface_Setting ;
.
gsen:ontology
  rdf:type owl:Ontology ;
  rdfs:comment "This ontology contains terms and definitions based on the 2016 SKOS-RDF version of the IUGS Commission for Geoscience Information (CGI) Geoscience Terminology Working Group Event Environment vocabulary to describe the physical setting within which a GeologicEvent takes place. GeologicEnvironment is construed broadly to include physical settings on the Earth surface specified by climate, tectonics, physiography or geography, and settings in the Earths interior specified by pressure, temperature, chemical environment, or tectonics. Environments are places. Designed for use in the eventEnvironment property in GeoSciML GeologicEvent features."@en ;
  rdfs:comment "dct:creator--  CGI Geoscience Terminology Working Group"@en ;
  rdfs:comment "dct:date--  2016-06-15"@en ;
  rdfs:label "Setting"@en ;
  owl:imports gsoc:ontology ;
  owl:imports gspr:ontology ;
  owl:imports gsog:ontology ;
  owl:imports gsro:ontology ;
.
