# baseURI: https://w3id.org/gso/1.0/geologicfold/ontology
# imports: https://w3id.org/gso/1.0/common/ontology
# imports: https://w3id.org/gso/1.0/geologicquality/ontology
# imports: https://w3id.org/gso/1.0/geology/ontology
# imports: https://w3id.org/gso/1.0/quality/ontology

@prefix : <https://w3id.org/gso/1.0/geologicfold/> .
@prefix dct: <http://purl.org/dc/terms/> .
@prefix gsfd: <https://w3id.org/gso/1.0/geologicfold/> .
@prefix gsgq: <https://w3id.org/gso/1.0/geologicquality/> .
@prefix gsoc: <https://w3id.org/gso/1.0/common/> .
@prefix gsog: <https://w3id.org/gso/1.0/geology/> .
@prefix gsoq: <https://w3id.org/gso/1.0/quality/> .
@prefix owl: <http://www.w3.org/2002/07/owl#> .
@prefix rdf: <http://www.w3.org/1999/02/22-rdf-syntax-ns#> .
@prefix rdfs: <http://www.w3.org/2000/01/rdf-schema#> .
@prefix skos: <http://www.w3.org/2004/02/skos/core#> .   @prefix schema: <https://schema.org/> .
@prefix xsd: <http://www.w3.org/2001/XMLSchema#> .

gsfd:Anticline
  rdf:type owl:Class ;
  dct:source "https://inspire.ec.europa.eu/codelist/FoldProfileTypeValue/anticline" ;
  rdfs:comment "A fold whose core contains the stratigraphically older rocks"@en ;
  rdfs:label "Anticline "@en ;
  rdfs:subClassOf gsfd:Fold ;
.
gsfd:Antiform
  rdf:type owl:Class ;
  dct:source "https://inspire.ec.europa.eu/codelist/FoldProfileTypeValue/antiform" ;
  rdfs:comment "A convex-upward, concave downward fold."@en ;
  rdfs:label "Antiform"@en ;
  rdfs:subClassOf gsfd:Fold ;
.
gsfd:Chevron_Fold
  rdf:type owl:Class ;
  dct:source "http://www.geologyin.com/2015/02/types-of-folds-with-photos.html" ;
  rdfs:comment "A fold with straight limbs and sharp hinges. Well developed, these folds develop repeated set of v-shaped beds.  Inter-limb angles are generally 60 degrees or less. Chevron folding preferentially occurs in well bedded units where  bedding regularly alternates between contrasting competences."@en ;
  rdfs:label "Chevron Fold "@en ;
  rdfs:subClassOf gsfd:Fold ;
.
gsfd:Fold
  rdf:type owl:Class ;
  rdfs:comment "A curve or bend of a planar structure, such as rock strata, bedding planes, foliation or cleavage. A fold is usually the product of deformation, involving the compression of strata, but may include primary structures, as its definition is descriptive, not genetic. (Neuendorf et al., 2011)."@en ;
  rdfs:comment "One or more systematically curved layers, surfaces, or lines in a rock body. Fold denotes a structure formed by the deformation of a GeologicStructure to form a structure that may be described by the translation of an abstract line (the fold axis) parallel to itself along some curvilinear path (the fold profile). Folds have a hinge zone (zone of maximum curvature along the surface) and limbs (parts of the deformed surface not in the hinge zone).  Folds are described by an axial surface, hinge line , profile geometry, the solid angle between the limbs, and the relationships between adjacent folded surfaces if the folded structure is a Layering fabric (similar, parallel). (GeoSciML v3.2)"@en ;
  rdfs:comment "Subclasses are defined based on concave/convex geometry of fold relative to earth surface, and relationship to younging direction in folded strata if known."@en ;
  rdfs:label "Fold"@en ;
  rdfs:seeAlso <http://linked.data.gov.au/def/geofeatures/Fold> ;
  rdfs:subClassOf gsoc:Nonphysical_Morphologic_Feature ;
  rdfs:subClassOf gsog:Geologic_Structure ;
  rdfs:subClassOf [
      rdf:type owl:Restriction ;
      owl:onClass gsfd:Fold_Axial_Surface ;
      owl:onProperty gsoc:crosses ;
      owl:qualifiedCardinality "1"^^xsd:nonNegativeInteger ;
    ] ;
  rdfs:subClassOf [
      rdf:type owl:Restriction ;
      owl:onProperty gsoc:contains ;
      owl:someValuesFrom gsfd:Fold_Hinge ;
    ] ;
  rdfs:subClassOf [
      rdf:type owl:Restriction ;
      owl:onProperty gsoc:hasPersistentPart ;
      owl:someValuesFrom gsoc:Shape_Value ;
    ] ;
  rdfs:subClassOf [
      rdf:type owl:Restriction ;
      owl:onProperty gsoc:hasStaticPart ;
      owl:someValuesFrom gsfd:Fold_Limb ;
    ] ;
  rdfs:subClassOf [
      rdf:type owl:Restriction ;
      owl:onProperty gsoc:hostedBy ;
      owl:someValuesFrom gsog:Rock_Body ;
    ] ;
.
gsfd:Fold_Amplitude
  rdf:type owl:Class ;
  rdfs:comment "the length of half the distance from the crest of a fold to the adjacent troughs. "@en ;
  rdfs:label "Fold Amplitude"@en ;
  rdfs:subClassOf gsoc:Physical_Quality ;
  rdfs:subClassOf [
      rdf:type owl:Restriction ;
      owl:allValuesFrom gsfd:Fold ;
      owl:onProperty gsoc:isQualityOf ;
    ] ;
.
gsfd:Fold_Axial_Surface
  rdf:type owl:Class ;
  rdfs:comment "Abstract surface that bisects the limbs of a fold or is the normal to a surface defined by the poles to the folded surface (typically visualized on a stereonet).  The axial surface of a particular fold may be located based on observations of the folded geologic structure, but in general it has no direct physical manifestation. Contrast with hinge surface, which is defined as the surface containing a set of hinge lines in the stack of folded surfaces defining a fold structure.  As a geologic surface, the axial surface has geometric properties, including orientation, which may be specified by observations at one or more locations, or generalized using terminology (upright, inclined, reclined, recumbent, overturned). (revised from GeoSciML 3.2)"@en ;
  rdfs:isDefinedBy "Revised from GeoSciML v3.2"@en ;
  rdfs:label "Fold axial surface"@en ;
  rdfs:subClassOf gsoc:Low_Dimension_Feature ;
  rdfs:subClassOf [
      rdf:type owl:Restriction ;
      owl:onProperty gsoc:hasEssentialPart ;
      owl:someValuesFrom gsoc:Spatial_Region_2D ;
    ] ;
  rdfs:subClassOf [
      rdf:type owl:Restriction ;
      owl:onProperty gsoc:hasQuality ;
      owl:someValuesFrom gsoq:Orientation ;
    ] ;
  rdfs:subClassOf [
      rdf:type owl:Restriction ;
      owl:onProperty gsoc:hostedBy ;
      owl:someValuesFrom gsfd:Fold ;
    ] ;
.
gsfd:Fold_Hinge
  rdf:type owl:Class ;
  rdfs:comment "the line linking points of maximum curvature on a folded surface (http://www.geosci.usyd.edu.au/users/prey/Teaching/Geos-2123/Folds/Sld22.html). A low-dimensional feature"@en ;
  rdfs:label "Fold Hinge"@en ;
  rdfs:subClassOf gsoc:Low_Dimension_Feature ;
  rdfs:subClassOf [
      rdf:type owl:Restriction ;
      owl:onProperty gsoc:hasEssentialPart ;
      owl:someValuesFrom gsoc:Spatial_Region_1D ;
    ] ;
  rdfs:subClassOf [
      rdf:type owl:Restriction ;
      owl:onProperty gsoc:hostedBy ;
      owl:someValuesFrom gsfd:Fold ;
    ] ;
.
gsfd:Fold_Hinge_Surface
  rdf:type owl:Class ;
  rdfs:comment "Surface that contains the hinge lines in a stack of folded layers"@en ;
  rdfs:label "Fold - Hinge surface"@en ;
  rdfs:subClassOf gsoc:Low_Dimension_Feature ;
  rdfs:subClassOf [
      rdf:type owl:Restriction ;
      owl:minQualifiedCardinality "2"^^xsd:nonNegativeInteger ;
      owl:onClass gsfd:Fold_Hinge ;
      owl:onProperty gsoc:hostedBy ;
    ] ;
  rdfs:subClassOf [
      rdf:type owl:Restriction ;
      owl:onProperty gsoc:hasEssentialPart ;
      owl:someValuesFrom gsoc:Spatial_Region_2D ;
    ] ;
.
gsfd:Fold_InterLimb_Angle
  rdf:type owl:Class ;
  dct:source "Neuendorf et al., 2005" ;
  rdfs:comment "The angle between adjacent limbs of a fold, normally determined by drawing tangents to the fold limbs at the inflection points."@en ;
  rdfs:isDefinedBy "GeoSciML v4"@en ;
  rdfs:label "Fold limb shape"@en ;
  rdfs:subClassOf gsoc:Physical_Quality ;
  rdfs:subClassOf [
      rdf:type owl:Restriction ;
      owl:allValuesFrom gsfd:Fold ;
      owl:onProperty gsoc:isQualityOf ;
    ] ;
.
gsfd:Fold_Limb
  rdf:type owl:Class ;
  rdfs:comment "The generally planar region of a fold which lies between two adjacent hinge lines and is confined between the zones of maximum curvature. A role played by some layered rock reated to the adjacent fold hinges.  Not necessarily a feature"@en ;
  rdfs:label "Fold Limb"@en ;
  rdfs:subClassOf gsoc:Nonphysical_Morphologic_Feature ;
  rdfs:subClassOf gsog:Geologic_Structure ;
  rdfs:subClassOf [
      rdf:type owl:Restriction ;
      owl:allValuesFrom gsfd:Fold ;
      owl:onProperty gsoc:isPartOf ;
    ] ;
  rdfs:subClassOf [
      rdf:type owl:Restriction ;
      owl:onProperty gsoc:hasPersistentPart ;
      owl:someValuesFrom gsoc:Shape_Value ;
    ] ;
  rdfs:subClassOf [
      rdf:type owl:Restriction ;
      owl:onProperty gsoc:staticHostedBy ;
      owl:someValuesFrom gsfd:Fold ;
    ] ;
.
gsfd:Fold_Limb_Shape
  rdf:type owl:Class ;
  rdfs:comment "Straight vs curved limbs, eg kink, chevron, sinusoidal, box"@en ;
  rdfs:isDefinedBy "GeoSciML v4"@en ;
  rdfs:label "Fold limb shape"@en ;
  rdfs:subClassOf gsoc:Shape ;
  rdfs:subClassOf [
      rdf:type owl:Restriction ;
      owl:allValuesFrom gsfd:Fold ;
      owl:onProperty gsoc:isQualityOf ;
    ] ;
.
gsfd:Fold_Span
  rdf:type owl:Class ;
  rdfs:comment "linear distance between inflection points in a single fold (GeoSciML v3.2)"@en ;
  rdfs:isDefinedBy "GeoSciML v3.2"@en ;
  rdfs:label "Fold span"@en ;
  rdfs:subClassOf gsoc:Physical_Quality ;
  rdfs:subClassOf [
      rdf:type owl:Restriction ;
      owl:allValuesFrom gsfd:Fold ;
      owl:onProperty gsoc:isQualityOf ;
    ] ;
.
gsfd:Fold_Symmetry
  rdf:type owl:Class ;
  rdfs:comment "Concordance or discordance of bisecting surface and axial surface, or ratio of length of limbs. Folded surface may have asymmetry defined by limb length ratio if inflection points are defined. Definition based on bisecting surface/axial surface angle depends on having multiple surfaces defined such that the axial surface may be identified. (symmetric, assymetric)"@en ;
  rdfs:isDefinedBy "GeoSciML v4"@en ;
  rdfs:label "Fold symmetry"@en ;
  rdfs:subClassOf gsoc:Physical_Quality ;
  rdfs:subClassOf [
      rdf:type owl:Restriction ;
      owl:allValuesFrom gsfd:Fold ;
      owl:onProperty gsoc:isQualityOf ;
    ] ;
.
gsfd:Fold_System
  rdf:type owl:Class ;
  rdfs:comment "A collection of congruent folds  (axis and axial surface are parallel) produced by the same tectonic event. Sometimes referred to as a \"Fold Train\". (GeoSciML 4.0.1)"@en ;
  rdfs:label "Fold System"@en ;
  rdfs:subClassOf gsoc:Inherant_Feature ;
  rdfs:subClassOf gsog:Geologic_Structure ;
  rdfs:subClassOf [
      rdf:type owl:Restriction ;
      owl:minQualifiedCardinality "2"^^xsd:nonNegativeInteger ;
      owl:onClass gsfd:Fold ;
      owl:onProperty gsoc:hasEssentialPart ;
    ] ;
  rdfs:subClassOf [
      rdf:type owl:Restriction ;
      owl:onClass [
          rdf:type owl:Class ;
          owl:unionOf (
              gsog:Geologic_Event
              gsog:Geologic_Process
            ) ;
        ] ;
      owl:onProperty gsoc:staticHostedBy ;
      owl:qualifiedCardinality "1"^^xsd:nonNegativeInteger ;
    ] ;
.
gsfd:Fold_Wavelength
  rdf:type owl:Class ;
  rdfs:comment "The distance between adjacent crest or trough of  a single fold, or the average distance between adjacent crests or troughs in a fold system. "@en ;
  rdfs:label "Fold wavelength"@en ;
  rdfs:subClassOf gsoc:Physical_Quality ;
  rdfs:subClassOf [
      rdf:type owl:Restriction ;
      owl:allValuesFrom [
          rdf:type owl:Class ;
          owl:unionOf [
              rdf:type rdf:List ;
              rdf:first gsfd:Fold ;
              rdf:rest [
                  rdf:type rdf:List ;
                  rdf:first gsfd:Fold_System ;
                  rdf:rest () ;
                ] ;
            ] ;
        ] ;
      owl:onProperty gsoc:isQualityOf ;
    ] ;
.
gsfd:Hinge_Line_Curvature
  rdf:type owl:Class ;
  rdfs:comment "Variation in orientation of fold hinge along trend of fold, distinguish sheath from cylindrical folds. Specify with terminology eg sheath, dome, basin, cylindrical."@en ;
  rdfs:isDefinedBy "GeoSciML v4"@en ;
  rdfs:label "Fold hinge line curvature"@en ;
  rdfs:subClassOf gsoc:Physical_Quality ;
  rdfs:subClassOf [
      rdf:type owl:Restriction ;
      owl:allValuesFrom gsfd:Fold ;
      owl:onProperty gsoc:isQualityOf ;
    ] ;
.
gsfd:Hinge_Shape
  rdf:type owl:Class ;
  rdfs:comment "Rounded vs. angular hinge zones; has to do with the proportion of the wavelength that is considered part of hinge"@en ;
  rdfs:isDefinedBy "GeoSciML v4"@en ;
  rdfs:label "Fold hinge shape"@en ;
  rdfs:subClassOf gsoc:Shape ;
  rdfs:subClassOf [
      rdf:type owl:Restriction ;
      owl:allValuesFrom gsfd:Fold ;
      owl:onProperty gsoc:isQualityOf ;
    ] ;
.
gsfd:Is_Periodic
  rdf:type owl:Class ;
  rdfs:comment "boolean value, true if wavelength of folds in a fold system is approximately the same"@en ;
  rdfs:label "Folds are periodic"@en ;
  rdfs:subClassOf gsoc:Physical_Quality ;
  rdfs:subClassOf [
      rdf:type owl:Restriction ;
      owl:allValuesFrom gsfd:Fold_System ;
      owl:onProperty gsoc:isQualityOf ;
    ] ;
.
gsfd:Monocline
  rdf:type owl:Class ;
  dct:source "https://en.wikipedia.org/wiki/Monocline" ;
  rdfs:comment "step-like fold in rock strata consisting of a zone of steeper dip within an otherwise horizontal or gently-dipping sequence."@en ;
  rdfs:label "Monocline "@en ;
  rdfs:subClassOf gsfd:Fold ;
.
gsfd:Neutral_Fold
  rdf:type owl:Class ;
  dct:source "https://www.encyclopedia.com/science/dictionaries-thesauruses-pictures-and-press-releases/neutral-fold" ;
  rdfs:comment "A fold which closes laterally and is therefore neither antiformal nor synformal.  "@en ;
  rdfs:label "Neutral Fold "@en ;
  rdfs:subClassOf gsfd:Fold ;
.
gsfd:Ptygmatic_Fold
  rdf:type owl:Class ;
  rdfs:comment "Chaotic and highly sinuous fold typically in an isolated layer within a more homogeneous rock body. Typical of sedimentary slump folding and veins or dikes in medium to high-grade metamorphic rocks"@en ;
  rdfs:label "Ptygmatic Fold "@en ;
  rdfs:subClassOf gsfd:Fold ;
.
gsfd:Recumbent
  rdf:type owl:Class ;
  dct:source "Fleuty (1964) Folds classification." ;
  rdfs:comment "Surface dips between 0 and 10 degrees; typically used to describe orientation of fold hing surface or axial surface, use equivalent term 'Horizontal inclination' for other geologic surfaces."@en ;
  rdfs:label "Recumbent "@en ;
  rdfs:subClassOf gsgq:Plane_Orientation ;
.
gsfd:Recumbent_Fold
  rdf:type owl:Class ;
  dct:source "Fleuty (1964) Folds classification." ;
  rdfs:comment "A fold that has an essentially horizontal axial plane."@en ;
  rdfs:label "Recumbent Fold "@en ;
  rdfs:subClassOf gsfd:Neutral_Fold ;
.
gsfd:Syncline
  rdf:type owl:Class ;
  dct:source "https://inspire.ec.europa.eu/codelist/FoldProfileTypeValue/syncline" ;
  rdfs:comment "A fold of which the core contains the stratigraphically younger rocks"@en ;
  rdfs:label "Syncline "@en ;
  rdfs:subClassOf gsfd:Fold ;
.
gsfd:Synform
  rdf:type owl:Class ;
  dct:source "based on https://inspire.ec.europa.eu/codelist/FoldProfileTypeValue/antiform" ;
  rdfs:comment "A convex-downward, concave upward fold."@en ;
  rdfs:label "Synform"@en ;
  rdfs:subClassOf gsfd:Fold ;
.
gsfd:Upright_Inclination
  rdf:type owl:Class ;
  dct:source "Fleuty (1964) Folds classification." ;
  rdfs:comment "Surface dips between 80 and 90 degrees, used to describe orientation of fold hinge surface or axial surface;  use equivalent term 'Vertical inclination' for other geologic surfaces."@en ;
  rdfs:label "Upright Inclination"@en ;
  rdfs:subClassOf gsgq:Plane_Orientation ;
.
gsfd:Vertical_Fold
  rdf:type owl:Class ;
  dct:source "Fleuty (1964) Folds classification." ;
  rdfs:comment "A fold for which the fold axis is vertical and axial surface is upright."@en ;
  rdfs:label "Vertical Fold "@en ;
  rdfs:subClassOf gsfd:Neutral_Fold ;
.
gsoc:boyan_brodaric rdf:type schema:Person ; rdf:type owl:NamedIndividual ;
  schema:affiliation "Natural Resources Canada, Geological Survey of Canada"  ;
  rdfs:comment "e-mail: mailto:boyan.brodaric@canada.ca " ;
  schema:identifier <https://orcid.org/0000-0002-7987-3810> ;
  schema:name "Dr. Boyan Brodaric" ; rdfs:label "Dr. Boyan Brodaric" ;
.
gsfd:ontology
  rdf:type owl:Ontology ;
  dct:created "2021-03-26"^^xsd:date ;
  dct:creator gsoc:boyan_brodaric ;
  dct:creator gsoc:stephen_richard ;
  dct:license <https://creativecommons.org/licenses/by/4.0/legalcode> ;
  dct:modified "2021-03-26"^^xsd:date ;
  dct:publisher "ARC Loop3D project;  https://loop3d.org/" ;
  dct:publisher "Geological Survey of Canada, Natural Resources Canada, Government of Canada" ;
    schema:codeRepository "https://github.com/Loop3D/GKM";  dct:rights  "Copyright (c) 2021 Government of Canada" ;
  rdfs:comment "Fold types and qualities related to folds."@en ;
  rdfs:label "Geoscience Ontology, Fold"@en ;
  dct:bibliographicCitation "Brodaric, B., and Richard, S.M., 2021, The GeoScience Ontology Reference: Geological Survey of Canada Open File 8796, 34 p., https://doi.org/10.4095/328296";
  owl:imports gsoc:ontology ;
  owl:imports gsgq:ontology ;
  owl:imports gsog:ontology ;
  owl:imports gsoq:ontology ;
  skos:definition "Fold types and properties related to folds."@en ;
  skos:prefLabel "Geoscience Ontology, Fold"@en ;
.
gsoc:stephen_richard    rdf:type schema:Person ;     rdf:type owl:NamedIndividual ;
  rdfs:comment "e-mail: mailto:smrTucson@gmail.com " ;
  schema:identifier <https://orcid.org/0000-0001-6041-5302> ;   schema:name "Dr. Stephen M. Richard" ;
   rdfs:label "Dr. Stephen M. Richard" ;
.
