# baseURI: https://w3id.org/gso/1.0/geologictime/ontology
# imports: https://w3id.org/gso/1.0/common/ontology
# imports: https://w3id.org/gso/1.0/geologicunit/ontology
# imports: https://w3id.org/gso/1.0/geology/ontology
# imports: https://w3id.org/gso/1.0/qudt/voc/ontology

@prefix : <https://w3id.org/gso/1.0/geologictime/> .
@prefix gscn: <https://w3id.org/gso/1.0/geologiccontact/> .
@prefix gsgu: <https://w3id.org/gso/1.0/geologicunit/> .
@prefix gsoc: <https://w3id.org/gso/1.0/common/> .
@prefix gsog: <https://w3id.org/gso/1.0/geology/> .
@prefix gst: <https://w3id.org/gso/1.0/geologictime/> .

@prefix owl: <http://www.w3.org/2002/07/owl#> .
@prefix rdf: <http://www.w3.org/1999/02/22-rdf-syntax-ns#> .
@prefix rdfs: <http://www.w3.org/2000/01/rdf-schema#> .
@prefix dct: <http://purl.org/dc/terms/> .
@prefix skos: <http://www.w3.org/2004/02/skos/core#> .   @prefix schema: <https://schema.org/> .
@prefix xsd: <http://www.w3.org/2001/XMLSchema#> .
@prefix unit: <http://qudt.org/vocab/unit/> .


gst:ontology
  rdf:type owl:Ontology ;
  rdfs:comment "generated by S.M.Richard for Loop3D project"@en ;
  rdfs:comment "generic definition of time ordinal eras and older boundaries for eras, based on all eras defined in ISC 2020 time scale. The intention is to define generic time scale concepts to unify the materialization of those concepts in different versions of the time scale. Each specific materialization is linked to the unifying element as 'part of'. "@en ;
  rdfs:label "Geoscience Ontology, Geologic Timescale Framework"@en ;
  owl:imports gsoc:ontology ;
  owl:imports gsgu:ontology ;
  owl:imports gsog:ontology ;
  owl:imports <https://w3id.org/gso/1.0/qudt/voc/ontology> ;
  owl:versionInfo "2021-03-10"@en ;
  dct:bibliographicCitation "Brodaric, B., and Richard, S.M., 2021, The GeoScience Ontology Reference, Geologic Time: Geological Survey of Canada Open File 8796, 34 p., https://doi.org/10.4095/328296";
  skos:definition "Defines named ordinal eras and their older boundaries that are used to build the geologic time scale, without anchoring to particular geologic features"@en ;
  skos:prefLabel "Geoscience Ontology, Geologic Timescale Framework"@en ;
  dct:created "2021-03-10"^^xsd:date ;
  dct:creator gsoc:stephen_richard ;
  dct:creator gsoc:boyan_brodaric ;
  dct:license <https://creativecommons.org/licenses/by/4.0/legalcode> ;
    schema:codeRepository "https://github.com/Loop3D/GKM";  dct:rights   "Copyright (c) 2021 Government of Canada" ; 
  dct:modified "2021-03-26"^^xsd:date ;
  dct:publisher "ARC Loop3D project;  https://loop3d.org/" ;
  dct:publisher "Geological Survey of Canada, Natural Resources Canada, Government of Canada" ;
.
gsoc:stephen_richard    rdf:type schema:Person ;     rdf:type owl:NamedIndividual ;
  rdfs:comment "e-mail: mailto:smrTucson@gmail.com " ;
  schema:identifier <https://orcid.org/0000-0001-6041-5302> ;   schema:name "Dr. Stephen M. Richard" ;
.
gsoc:boyan_brodaric rdf:type schema:Person ; rdf:type owl:NamedIndividual ;
  schema:affiliation "Natural Resources Canada, Geological Survey of Canada"  ;
  rdfs:comment "e-mail: mailto:boyan.brodaric@canada.ca " ;
  schema:identifier <https://orcid.org/0000-0002-7987-3810> ;
  schema:name "Dr. Boyan Brodaric" ; rdfs:label "Dr. Boyan Brodaric" ;
.


gst:AalenianAge
  rdf:type gst:Age ;
  rdf:type gsog:Generic_Geologic_Time_Unit ;
  gsoc:timeStarts gst:BaseMiddleJurassic ;
  rdfs:comment "Interval for grouping all specific instances of the Aalenian Age"@en ;
  rdfs:label "Aalenian Age"@en ;
.
gst:AeronianAge
  rdf:type gst:Age ;
  rdf:type gsog:Generic_Geologic_Time_Unit ;
  gsoc:timeStarts gst:BaseAeronian ;
  rdfs:comment "Interval for grouping all specific instances of the Aeronian Age"@en ;
  rdfs:label "Aeronian Age"@en ;
.
gst:Age
  rdf:type owl:Class ;
  rdfs:comment "Most granular geochronologic time interval;  one or more Ages are grouped into an Epoch"@en ;
  rdfs:label "Age (time scale rank)"@en ;
  rdfs:subClassOf gsog:Geologic_Time_Interval ;
  rdfs:subClassOf [
      rdf:type owl:Restriction ;
      owl:allValuesFrom [
          rdf:type owl:Class ;
          owl:complementOf gst:Age ;
        ] ;
      owl:onProperty gsoc:timeIncludedBy ;
    ] ;
  rdfs:subClassOf [
      rdf:type owl:Restriction ;
      owl:onProperty gsoc:hostedBy ;
      owl:someValuesFrom [
          rdf:type owl:Class ;
          owl:unionOf (
              gsgu:Stage
              gsgu:Substage
            ) ;
        ] ;
    ] ;
.
gst:AlbianAge
  rdf:type gst:Age ;
  rdf:type gsog:Generic_Geologic_Time_Unit ;
  gsoc:timeStarts gst:BaseAlbian ;
  rdfs:comment "Interval for grouping all specific instances of the Albian Age"@en ;
  rdfs:label "Albian Age"@en ;
.
gst:AnisianAge
  rdf:type gst:Age ;
  rdf:type gsog:Generic_Geologic_Time_Unit ;
  gsoc:timeStarts gst:BaseMiddleTriassic ;
  rdfs:comment "Interval for grouping all specific instances of the Anisian Age"@en ;
  rdfs:label "Anisian Age"@en ;
.
gst:AptianAge
  rdf:type gst:Age ;
  rdf:type gsog:Generic_Geologic_Time_Unit ;
  gsoc:timeStarts gst:BaseAptian ;
  rdfs:comment "Interval for grouping all specific instances of the Aptian Age"@en ;
  rdfs:label "Aptian Age"@en ;
.
gst:AquitanianAge
  rdf:type gst:Age ;
  rdf:type gsog:Generic_Geologic_Time_Unit ;
  gsoc:timeStarts gst:BaseNeogene ;
  rdfs:comment "Interval for grouping all specific instances of the Aquitanian Age"@en ;
  rdfs:label "Aquitanian Age"@en ;
.
gst:ArcheanEon
  rdf:type gst:Eon ;
  rdf:type gsog:Generic_Geologic_Time_Unit ;
  gsoc:timeStarts gst:BaseArchean ;
  rdfs:comment "Interval for grouping all specific instances of the Archean Eon"@en ;
  rdfs:label "Archean Eon"@en ;
.
gst:ArtinskianAge
  rdf:type gst:Age ;
  rdf:type gsog:Generic_Geologic_Time_Unit ;
  rdfs:comment "Interval for grouping all specific instances of the Artinskian Age"@en ;
  rdfs:label "Artinskian Age"@en ;
.
gst:AsselianAge
  rdf:type gst:Age ;
  rdf:type gsog:Generic_Geologic_Time_Unit ;
  gsoc:timeStarts gst:BasePermian ;
  rdfs:comment "Interval for grouping all specific instances of the Asselian Age"@en ;
  rdfs:label "Asselian Age"@en ;
.
gst:BajocianAge
  rdf:type gst:Age ;
  rdf:type gsog:Generic_Geologic_Time_Unit ;
  gsoc:timeStarts gst:BaseBajocian ;
  rdfs:comment "Interval for grouping all specific instances of the Bajocian Age"@en ;
  rdfs:label "Bajocian Age"@en ;
.
gst:BarremianAge
  rdf:type gst:Age ;
  rdf:type gsog:Generic_Geologic_Time_Unit ;
  gsoc:timeStarts gst:BaseBarremian ;
  rdfs:comment "Interval for grouping all specific instances of the Barremian Age"@en ;
  rdfs:label "Barremian Age"@en ;
.
gst:BartonianAge
  rdf:type gst:Age ;
  rdf:type gsog:Generic_Geologic_Time_Unit ;
  gsoc:timeStarts gst:BaseBartonian ;
  rdfs:comment "Interval for grouping all specific instances of the Bartonian Age"@en ;
  rdfs:label "Bartonian Age"@en ;
.
gst:BaseAalenian
  rdf:type gsog:Geologic_Time_Boundary ;
  gsoc:timeEquivalentTo gst:BaseMiddleJurassic ;
  rdfs:label "shared boundary with BaseMiddleJurassic"@en ;
.
gst:BaseAeronian
  rdf:type gsog:Geologic_Time_Boundary ;
  rdfs:comment "Interval for grouping all specific instances of the Base of Aeronian"@en ;
  rdfs:label "Base of Aeronian"@en ;
.
gst:BaseAlbian
  rdf:type gsog:Geologic_Time_Boundary ;
  rdfs:comment "Interval for grouping all specific instances of the Base of Albian"@en ;
  rdfs:label "Base of Albian"@en ;
.
gst:BaseAnisian
  rdf:type gsog:Geologic_Time_Boundary ;
  gsoc:timeEquivalentTo gst:BaseMiddleTriassic ;
  rdfs:label "shared boundary with BaseMiddleTriassic"@en ;
.
gst:BaseAptian
  rdf:type gsog:Geologic_Time_Boundary ;
  rdfs:comment "Interval for grouping all specific instances of the Base of Aptian"@en ;
  rdfs:label "Base of Aptian"@en ;
.
gst:BaseAquitanian
  rdf:type gsog:Geologic_Time_Boundary ;
  gsoc:timeEquivalentTo gst:BaseNeogene ;
  rdfs:label "shared boundary with BaseNeogene"@en ;
.
gst:BaseArchean
  rdf:type gsog:GSSA ;
  rdfs:comment "Interval for grouping all specific instances of the Base of Archean"@en ;
  rdfs:label "Base of Archean"@en ;
.
gst:BaseArtinskian
  rdf:type gsog:Geologic_Time_Boundary ;
  gsoc:timeStarts gst:ArtinskianAge ;
  rdfs:comment "Interval for grouping all specific instances of the Base of Artinskian"@en ;
  rdfs:label "Base of Artinskian"@en ;
.
gst:BaseAsselian
  rdf:type gsog:Geologic_Time_Boundary ;
  gsoc:timeEquivalentTo gst:BasePermian ;
  rdfs:label "shared boundary with BasePermian"@en ;
.
gst:BaseBajocian
  rdf:type gsog:Geologic_Time_Boundary ;
  rdfs:comment "Interval for grouping all specific instances of the Base of Bajocian"@en ;
  rdfs:label "Base of Bajocian"@en ;
.
gst:BaseBarremian
  rdf:type gsog:Geologic_Time_Boundary ;
  rdfs:comment "Interval for grouping all specific instances of the Base of Barremian"@en ;
  rdfs:label "Base of Barremian"@en ;
.
gst:BaseBartonian
  rdf:type gsog:Geologic_Time_Boundary ;
  rdfs:comment "Interval for grouping all specific instances of the Base of Bartonian"@en ;
  rdfs:label "Base of Bartonian"@en ;
.
gst:BaseBashkirian
  rdf:type gsog:Geologic_Time_Boundary ;
  gsoc:timeEquivalentTo gst:BasePennsylvanian ;
  rdfs:label "shared boundary with BasePennsylvanian"@en ;
.
gst:BaseBathonian
  rdf:type gsog:Geologic_Time_Boundary ;
  rdfs:comment "Interval for grouping all specific instances of the Base of Bathonian"@en ;
  rdfs:label "Base of Bathonian"@en ;
.
gst:BaseBerriasian
  rdf:type gsog:Geologic_Time_Boundary ;
  gsoc:timeEquivalentTo gst:BaseCretaceous ;
  rdfs:label "shared boundary with BaseCretaceous"@en ;
.
gst:BaseBurdigalian
  rdf:type gsog:Geologic_Time_Boundary ;
  rdfs:comment "Interval for grouping all specific instances of the Base of Burdigalian"@en ;
  rdfs:label "Base of Burdigalian"@en ;
.
gst:BaseCalabrian
  rdf:type gsog:Geologic_Time_Boundary ;
  rdfs:comment "Interval for grouping all specific instances of the Base of Calabrian"@en ;
  rdfs:label "Base of Calabrian"@en ;
.
gst:BaseCallovian
  rdf:type gsog:Geologic_Time_Boundary ;
  rdfs:comment "Interval for grouping all specific instances of the Base of Callovian"@en ;
  rdfs:label "Base of Callovian"@en ;
.
gst:BaseCalymmian
  rdf:type gsog:GSSA ;
  gsoc:timeEquivalentTo gst:BaseMesoproterozoic ;
  rdfs:label "shared boundary with BaseMesoproterozoic"@en ;
.
gst:BaseCambrian
  rdf:type gsog:Geologic_Time_Boundary ;
  gsoc:timeEquivalentTo gst:BasePhanerozoic ;
  rdfs:label "shared boundary with BasePhanerozoic"@en ;
.
gst:BaseCambrianSeries2
  rdf:type gsog:Geologic_Time_Boundary ;
  rdfs:comment "Interval for grouping all specific instances of the Base of Cambrian Series 2"@en ;
  rdfs:label "Base of Cambrian Series 2"@en ;
.
gst:BaseCambrianSeries3
  rdf:type gsog:Geologic_Time_Boundary ;
  rdfs:comment "Interval for grouping all specific instances of the Base of Cambrian Series 3"@en ;
  rdfs:label "Base of Cambrian Series 3"@en ;
.
gst:BaseCambrianStage10
  rdf:type gsog:Geologic_Time_Boundary ;
  rdfs:comment "Interval for grouping all specific instances of the Base of Cambrian Stage 10"@en ;
  rdfs:label "Base of Cambrian Stage 10"@en ;
.
gst:BaseCambrianStage2
  rdf:type gsog:Geologic_Time_Boundary ;
  rdfs:comment "Interval for grouping all specific instances of the Base of Cambrian Stage 2"@en ;
  rdfs:label "Base of Cambrian Stage 2"@en ;
.
gst:BaseCambrianStage3
  rdf:type gsog:Geologic_Time_Boundary ;
  gsoc:timeEquivalentTo gst:BaseCambrianSeries2 ;
  rdfs:label "shared boundary with BaseCambrianSeries2"@en ;
.
gst:BaseCambrianStage4
  rdf:type gsog:Geologic_Time_Boundary ;
  rdfs:comment "Interval for grouping all specific instances of the Base of Cambrian Stage 4"@en ;
  rdfs:label "Base of Cambrian Stage 4"@en ;
.
gst:BaseCambrianStage5
  rdf:type gsog:Geologic_Time_Boundary ;
  gsoc:timeEquivalentTo gst:BaseCambrianSeries3 ;
  rdfs:label "shared boundary with BaseCambrianSeries3"@en ;
.
gst:BaseCampanian
  rdf:type gsog:Geologic_Time_Boundary ;
  rdfs:comment "Interval for grouping all specific instances of the Base of Campanian"@en ;
  rdfs:label "Base of Campanian"@en ;
.
gst:BaseCapitanian
  rdf:type gsog:Geologic_Time_Boundary ;
  rdfs:comment "Interval for grouping all specific instances of the Base of Capitanian"@en ;
  rdfs:label "Base of Capitanian"@en ;
.
gst:BaseCarboniferous
  rdf:type gsog:Geologic_Time_Boundary ;
  rdfs:comment "Interval for grouping all specific instances of the Base of Carboniferous"@en ;
  rdfs:label "Base of Carboniferous"@en ;
.
gst:BaseCarnian
  rdf:type gsog:Geologic_Time_Boundary ;
  gsoc:timeEquivalentTo gst:BaseUpperTriassic ;
  rdfs:label "shared boundary with BaseUpperTriassic"@en ;
.
gst:BaseCenomanian
  rdf:type gsog:Geologic_Time_Boundary ;
  gsoc:timeEquivalentTo gst:BaseUpperCretaceous ;
  rdfs:label "shared boundary with BaseUpperCretaceous"@en ;
.
gst:BaseCenozoic
  rdf:type gsog:Geologic_Time_Boundary ;
  gsoc:timeStarts gst:BaseCenozoic ;
  rdfs:comment "Interval for grouping all specific instances of the Base of Cenozoic"@en ;
  rdfs:label "Base of Cenozoic"@en ;
.
gst:BaseChanghsingian
  rdf:type gsog:Geologic_Time_Boundary ;
  rdfs:comment "Interval for grouping all specific instances of the Base of Changhsingian"@en ;
  rdfs:label "Base of Changhsingian"@en ;
.
gst:BaseChattian
  rdf:type gsog:Geologic_Time_Boundary ;
  rdfs:comment "Interval for grouping all specific instances of the Base of Chattian"@en ;
  rdfs:label "Base of Chattian"@en ;
.
gst:BaseChibanianStage
  rdf:type gsog:Geologic_Time_Boundary ;
  rdfs:comment "Interval for grouping all specific instances of the Base of Chibanian Stage"@en ;
  rdfs:label "Base of Chibanian Stage"@en ;
.
gst:BaseCisuralian
  rdf:type gsog:Geologic_Time_Boundary ;
  gsoc:timeEquivalentTo gst:BasePermian ;
  rdfs:label "shared boundary with BasePermian"@en ;
.
gst:BaseConiacian
  rdf:type gsog:Geologic_Time_Boundary ;
  rdfs:comment "Interval for grouping all specific instances of the Base of Coniacian"@en ;
  rdfs:label "Base of Coniacian"@en ;
.
gst:BaseCretaceous
  rdf:type gsog:Geologic_Time_Boundary ;
  rdfs:comment "Interval for grouping all specific instances of the Base of Cretaceous"@en ;
  rdfs:label "Base of Cretaceous"@en ;
.
gst:BaseCryogenian
  rdf:type gsog:Geologic_Time_Boundary ;
  rdfs:comment "Interval for grouping all specific instances of the Base of Cryogenian"@en ;
  rdfs:label "Base of Cryogenian"@en ;
.
gst:BaseDanian
  rdf:type gsog:Geologic_Time_Boundary ;
  gsoc:timeEquivalentTo gst:BaseCenozoic ;
  rdfs:label "shared boundary with BaseCenozoic"@en ;
.
gst:BaseDapingian
  rdf:type gsog:Geologic_Time_Boundary ;
  gsoc:timeEquivalentTo gst:BaseMiddleOrdovician ;
  rdfs:label "shared boundary with BaseMiddleOrdovician"@en ;
.
gst:BaseDarriwilian
  rdf:type gsog:Geologic_Time_Boundary ;
  gsoc:timeEquivalentTo gst:BaseDarriwillian ;
  rdfs:label "shared boundary with BaseDarriwillian"@en ;
.
gst:BaseDarriwillian
  rdf:type gsog:Geologic_Time_Boundary ;
  rdfs:comment "Interval for grouping all specific instances of the Base of Darriwillian"@en ;
  rdfs:label "Base of Darriwillian"@en ;
.
gst:BaseDevonian
  rdf:type gsog:Geologic_Time_Boundary ;
  rdfs:comment "Interval for grouping all specific instances of the Base of Devonian"@en ;
  rdfs:label "Base of Devonian"@en ;
.
gst:BaseDrumian
  rdf:type gsog:Geologic_Time_Boundary ;
  rdfs:comment "Interval for grouping all specific instances of the Base of Drumian"@en ;
  rdfs:label "Base of Drumian"@en ;
.
gst:BaseEctasian
  rdf:type gsog:GSSA ;
  rdfs:comment "Interval for grouping all specific instances of the Base of Ectasian"@en ;
  rdfs:label "Base of Ectasian"@en ;
.
gst:BaseEdiacaran
  rdf:type gsog:Geologic_Time_Boundary ;
  rdfs:comment "Interval for grouping all specific instances of the Base of Ediacaran"@en ;
  rdfs:label "Base of Ediacaran"@en ;
.
gst:BaseEifelian
  rdf:type gsog:Geologic_Time_Boundary ;
  gsoc:timeEquivalentTo gst:BaseMiddleDevonian ;
  rdfs:label "shared boundary with BaseMiddleDevonian"@en ;
.
gst:BaseEmsian
  rdf:type gsog:Geologic_Time_Boundary ;
  rdfs:comment "Interval for grouping all specific instances of the Base of Emsian"@en ;
  rdfs:label "Base of Emsian"@en ;
.
gst:BaseEoarchean
  rdf:type gsog:GSSA ;
  gsoc:timeEquivalentTo gst:BaseArchean ;
  rdfs:label "shared boundary with BaseArchean"@en ;
.
gst:BaseEocene
  rdf:type gsog:Geologic_Time_Boundary ;
  rdfs:comment "Interval for grouping all specific instances of the Base of Eocene"@en ;
  rdfs:label "Base of Eocene"@en ;
.
gst:BaseFamennian
  rdf:type gsog:Geologic_Time_Boundary ;
  rdfs:comment "Interval for grouping all specific instances of the Base of Famennian"@en ;
  rdfs:label "Base of Famennian"@en ;
.
gst:BaseFloian
  rdf:type gsog:Geologic_Time_Boundary ;
  rdfs:comment "Interval for grouping all specific instances of the Base of Floian"@en ;
  rdfs:label "Base of Floian"@en ;
.
gst:BaseFortunian
  rdf:type gsog:Geologic_Time_Boundary ;
  gsoc:timeEquivalentTo gst:BasePhanerozoic ;
  rdfs:label "shared boundary with BasePhanerozoic"@en ;
.
gst:BaseFrasnian
  rdf:type gsog:Geologic_Time_Boundary ;
  gsoc:timeEquivalentTo gst:BaseUpperDevonian ;
  rdfs:label "shared boundary with BaseUpperDevonian"@en ;
.
gst:BaseFurongian
  rdf:type gsog:Geologic_Time_Boundary ;
  rdfs:comment "Interval for grouping all specific instances of the Base of Furongian"@en ;
  rdfs:label "Base of Furongian"@en ;
.
gst:BaseGelasian
  rdf:type gsog:Geologic_Time_Boundary ;
  rdfs:comment "Interval for grouping all specific instances of the Base of Gelasian"@en ;
  rdfs:label "Base of Gelasian"@en ;
.
gst:BaseGivetian
  rdf:type gsog:Geologic_Time_Boundary ;
  rdfs:comment "Interval for grouping all specific instances of the Base of Givetian"@en ;
  rdfs:label "Base of Givetian"@en ;
.
gst:BaseGorstian
  rdf:type gsog:Geologic_Time_Boundary ;
  gsoc:timeEquivalentTo gst:BaseLudlow ;
  rdfs:label "shared boundary with BaseLudlow"@en ;
.
gst:BaseGreenlandian
  rdf:type gsog:Geologic_Time_Boundary ;
  gsoc:timeEquivalentTo gst:BaseHolocene ;
  rdfs:label "shared boundary with BaseHolocene"@en ;
.
gst:BaseGuadalupian
  rdf:type gsog:Geologic_Time_Boundary ;
  rdfs:comment "Interval for grouping all specific instances of the Base of Guadalupian"@en ;
  rdfs:label "Base of Guadalupian"@en ;
.
gst:BaseGuzhangian
  rdf:type gsog:Geologic_Time_Boundary ;
  rdfs:comment "Interval for grouping all specific instances of the Base of Guzhangian"@en ;
  rdfs:label "Base of Guzhangian"@en ;
.
gst:BaseGzhelian
  rdf:type gsog:Geologic_Time_Boundary ;
  rdfs:comment "Interval for grouping all specific instances of the Base of Gzhelian"@en ;
  rdfs:label "Base of Gzhelian"@en ;
.
gst:BaseHadean
  rdf:type gsog:GSSA ;
  gsoc:timeEquivalentTo gst:FormationoftheEarth ;
  rdfs:label "shared boundary with FormationoftheEarth"@en ;
.
gst:BaseHauterivian
  rdf:type gsog:Geologic_Time_Boundary ;
  rdfs:comment "Interval for grouping all specific instances of the Base of Hauterivian"@en ;
  rdfs:label "Base of Hauterivian"@en ;
.
gst:BaseHettangian
  rdf:type gsog:Geologic_Time_Boundary ;
  gsoc:timeEquivalentTo gst:BaseJurassic ;
  rdfs:label "shared boundary with BaseJurassic"@en ;
.
gst:BaseHirnantian
  rdf:type gsog:Geologic_Time_Boundary ;
  rdfs:comment "Interval for grouping all specific instances of the Base of Hirnantian"@en ;
  rdfs:label "Base of Hirnantian"@en ;
.
gst:BaseHolocene
  rdf:type gsog:Geologic_Time_Boundary ;
  rdfs:comment "Interval for grouping all specific instances of the Base Holocene  "@en ;
  rdfs:label "Base Holocene  "@en ;
.
gst:BaseHomerian
  rdf:type gsog:Geologic_Time_Boundary ;
  rdfs:comment "Interval for grouping all specific instances of the Base of Homerian"@en ;
  rdfs:label "Base of Homerian"@en ;
.
gst:BaseInduan
  rdf:type gsog:Geologic_Time_Boundary ;
  gsoc:timeEquivalentTo gst:BaseMesozoic ;
  rdfs:label "shared boundary with BaseMesozoic"@en ;
.
gst:BaseJiangshanian
  rdf:type gsog:Geologic_Time_Boundary ;
  rdfs:comment "Interval for grouping all specific instances of the Base of Jiangshanian"@en ;
  rdfs:label "Base of Jiangshanian"@en ;
.
gst:BaseJurassic
  rdf:type gsog:Geologic_Time_Boundary ;
  rdfs:comment "Interval for grouping all specific instances of the Base of Jurassic"@en ;
  rdfs:label "Base of Jurassic"@en ;
.
gst:BaseKasimovian
  rdf:type gsog:Geologic_Time_Boundary ;
  gsoc:timeEquivalentTo gst:BaseUpperPennsylvanian ;
  rdfs:label "shared boundary with BaseUpperPennsylvanian"@en ;
.
gst:BaseKatian
  rdf:type gsog:Geologic_Time_Boundary ;
  rdfs:comment "Interval for grouping all specific instances of the Base of Katian"@en ;
  rdfs:label "Base of Katian"@en ;
.
gst:BaseKimmeridgian
  rdf:type gsog:Geologic_Time_Boundary ;
  rdfs:comment "Interval for grouping all specific instances of the Base of Kimmeridgian"@en ;
  rdfs:label "Base of Kimmeridgian"@en ;
.
gst:BaseKungurian
  rdf:type gsog:Geologic_Time_Boundary ;
  rdfs:comment "Interval for grouping all specific instances of the Base of Kungurian"@en ;
  rdfs:label "Base of Kungurian"@en ;
.
gst:BaseLadinian
  rdf:type gsog:Geologic_Time_Boundary ;
  rdfs:comment "Interval for grouping all specific instances of the Base of Ladinian"@en ;
  rdfs:label "Base of Ladinian"@en ;
.
gst:BaseLanghian
  rdf:type gsog:Geologic_Time_Boundary ;
  rdfs:comment "Interval for grouping all specific instances of the Base of Langhian"@en ;
  rdfs:label "Base of Langhian"@en ;
.
gst:BaseLlandovery
  rdf:type gsog:Geologic_Time_Boundary ;
  gsoc:timeEquivalentTo gst:BaseSilurian ;
  rdfs:label "shared boundary with BaseSilurian"@en ;
.
gst:BaseLochkovian
  rdf:type gsog:Geologic_Time_Boundary ;
  gsoc:timeEquivalentTo gst:BaseDevonian ;
  rdfs:label "shared boundary with BaseDevonian"@en ;
.
gst:BaseLopingian
  rdf:type gsog:Geologic_Time_Boundary ;
  rdfs:comment "Interval for grouping all specific instances of the Base of Lopingian"@en ;
  rdfs:label "Base of Lopingian"@en ;
.
gst:BaseLowerCambrian
  rdf:type gsog:Geologic_Time_Boundary ;
  gsoc:timeEquivalentTo gst:BasePhanerozoic ;
  rdfs:label "shared boundary with BasePhanerozoic"@en ;
.
gst:BaseLowerCretaceous
  rdf:type gsog:Geologic_Time_Boundary ;
  gsoc:timeEquivalentTo gst:BaseCretaceous ;
  rdfs:label "shared boundary with BaseCretaceous"@en ;
.
gst:BaseLowerDevonian
  rdf:type gsog:Geologic_Time_Boundary ;
  gsoc:timeEquivalentTo gst:BaseDevonian ;
  rdfs:label "shared boundary with BaseDevonian"@en ;
.
gst:BaseLowerJurassic
  rdf:type gsog:Geologic_Time_Boundary ;
  gsoc:timeEquivalentTo gst:BaseJurassic ;
  rdfs:label "shared boundary with BaseJurassic"@en ;
.
gst:BaseLowerMississippian
  rdf:type gsog:Geologic_Time_Boundary ;
  gsoc:timeEquivalentTo gst:BaseCarboniferous ;
  rdfs:label "shared boundary with BaseCarboniferous"@en ;
.
gst:BaseLowerOrdovician
  rdf:type gsog:Geologic_Time_Boundary ;
  gsoc:timeEquivalentTo gst:BaseOrdovician ;
  rdfs:label "shared boundary with BaseOrdovician"@en ;
.
gst:BaseLowerPennsylvanian
  rdf:type gsog:Geologic_Time_Boundary ;
  gsoc:timeEquivalentTo gst:BasePennsylvanian ;
  rdfs:label "shared boundary with BasePennsylvanian"@en ;
.
gst:BaseLowerTriassic
  rdf:type gsog:Geologic_Time_Boundary ;
  gsoc:timeEquivalentTo gst:BaseMesozoic ;
  rdfs:label "shared boundary with BaseMesozoic"@en ;
.
gst:BaseLudfordianStage
  rdf:type gsog:Geologic_Time_Boundary ;
  rdfs:comment "Interval for grouping all specific instances of the Base of Ludfordian Stage"@en ;
  rdfs:label "Base of Ludfordian Stage"@en ;
.
gst:BaseLudlow
  rdf:type gsog:Geologic_Time_Boundary ;
  rdfs:comment "Interval for grouping all specific instances of the Base of Ludlow - Gorstian"@en ;
  rdfs:label "Base of Ludlow - Gorstian"@en ;
.
gst:BaseLutetian
  rdf:type gsog:Geologic_Time_Boundary ;
  rdfs:comment "Interval for grouping all specific instances of the Base of Lutetian"@en ;
  rdfs:label "Base of Lutetian"@en ;
.
gst:BaseMaastrichtian
  rdf:type gsog:Geologic_Time_Boundary ;
  rdfs:comment "Interval for grouping all specific instances of the Base of Maastrichtian"@en ;
  rdfs:label "Base of Maastrichtian"@en ;
.
gst:BaseMeghalayan
  rdf:type gsog:Geologic_Time_Boundary ;
  rdfs:comment "Interval for grouping all specific instances of the Base of Meghalayan"@en ;
  rdfs:label "Base of Meghalayan"@en ;
.
gst:BaseMesoarchean
  rdf:type gsog:GSSA ;
  rdfs:comment "Interval for grouping all specific instances of the Base of Mesoarchean"@en ;
  rdfs:label "Base of Mesoarchean"@en ;
.
gst:BaseMesoproterozoic
  rdf:type gsog:GSSA ;
  rdfs:comment "Interval for grouping all specific instances of the Base of Mesoproterozoic"@en ;
  rdfs:label "Base of Mesoproterozoic"@en ;
.
gst:BaseMesozoic
  rdf:type gsog:Geologic_Time_Boundary ;
  rdfs:comment "Interval for grouping all specific instances of the Base of Mesozoic"@en ;
  rdfs:label "Base of Mesozoic"@en ;
.
gst:BaseMessinian
  rdf:type gsog:Geologic_Time_Boundary ;
  rdfs:comment "Interval for grouping all specific instances of the Base of Messinian"@en ;
  rdfs:label "Base of Messinian"@en ;
.
gst:BaseMiddleCambrianEpoch
  rdf:type gsog:Geologic_Time_Boundary ;
  rdfs:comment "Interval for grouping all specific instances of the Base Middle Cambrian Epoch  "@en ;
  rdfs:label "Base Middle Cambrian Epoch  "@en ;
.
gst:BaseMiddleDevonian
  rdf:type gsog:Geologic_Time_Boundary ;
  rdfs:comment "Interval for grouping all specific instances of the Base of Middle Devonian - Eifelian"@en ;
  rdfs:label "Base of Middle Devonian - Eifelian"@en ;
.
gst:BaseMiddleJurassic
  rdf:type gsog:Geologic_Time_Boundary ;
  rdfs:comment "Interval for grouping all specific instances of the Base of Middle Jurassic"@en ;
  rdfs:label "Base of Middle Jurassic"@en ;
.
gst:BaseMiddleMississippian
  rdf:type gsog:Geologic_Time_Boundary ;
  rdfs:comment "Interval for grouping all specific instances of the Base of Middle Mississippian - Visean"@en ;
  rdfs:label "Base of Middle Mississippian - Visean"@en ;
.
gst:BaseMiddleOrdovician
  rdf:type gsog:Geologic_Time_Boundary ;
  rdfs:comment "Interval for grouping all specific instances of the Base of Middle Ordovician"@en ;
  rdfs:label "Base of Middle Ordovician"@en ;
.
gst:BaseMiddlePennsylvanian
  rdf:type gsog:Geologic_Time_Boundary ;
  rdfs:comment "Interval for grouping all specific instances of the Base of Middle Pennsylvanian"@en ;
  rdfs:label "Base of Middle Pennsylvanian"@en ;
.
gst:BaseMiddlePleistocene
  rdf:type gsog:Geologic_Time_Boundary ;
  rdfs:comment "Interval for grouping all specific instances of the Base of Middle Pleistocene"@en ;
  rdfs:label "Base of Middle Pleistocene"@en ;
.
gst:BaseMiddleTriassic
  rdf:type gsog:Geologic_Time_Boundary ;
  rdfs:comment "Interval for grouping all specific instances of the Base of Middle Triassic"@en ;
  rdfs:label "Base of Middle Triassic"@en ;
.
gst:BaseMiocene
  rdf:type gsog:Geologic_Time_Boundary ;
  gsoc:timeEquivalentTo gst:BaseNeogene ;
  rdfs:label "shared boundary with BaseNeogene"@en ;
.
gst:BaseMississippian
  rdf:type gsog:Geologic_Time_Boundary ;
  gsoc:timeEquivalentTo gst:BaseCarboniferous ;
  rdfs:label "shared boundary with BaseCarboniferous"@en ;
.
gst:BaseMoscovian
  rdf:type gsog:Geologic_Time_Boundary ;
  gsoc:timeEquivalentTo gst:BaseMiddlePennsylvanian ;
  rdfs:label "shared boundary with BaseMiddlePennsylvanian"@en ;
.
gst:BaseNeoarchean
  rdf:type gsog:GSSA ;
  rdfs:comment "Interval for grouping all specific instances of the Base of Neoarchean"@en ;
  rdfs:label "Base of Neoarchean"@en ;
.
gst:BaseNeogene
  rdf:type gsog:Geologic_Time_Boundary ;
  rdfs:comment "Interval for grouping all specific instances of the Base of Neogene"@en ;
  rdfs:label "Base of Neogene"@en ;
.
gst:BaseNeoproterozoic
  rdf:type gsog:GSSA ;
  rdfs:comment "Interval for grouping all specific instances of the Base of Neoproterozoic"@en ;
  rdfs:label "Base of Neoproterozoic"@en ;
.
gst:BaseNorian
  rdf:type gsog:Geologic_Time_Boundary ;
  rdfs:comment "Interval for grouping all specific instances of the Base of Norian"@en ;
  rdfs:label "Base of Norian"@en ;
.
gst:BaseNorthgrippian
  rdf:type gsog:Geologic_Time_Boundary ;
  rdfs:comment "Interval for grouping all specific instances of the Base of Northgrippian"@en ;
  rdfs:label "Base of Northgrippian"@en ;
.
gst:BaseOlenekian
  rdf:type gsog:Geologic_Time_Boundary ;
  rdfs:comment "Interval for grouping all specific instances of the Base of Olenekian"@en ;
  rdfs:label "Base of Olenekian"@en ;
.
gst:BaseOligocene
  rdf:type gsog:Geologic_Time_Boundary ;
  rdfs:comment "Interval for grouping all specific instances of the Base of Oligocene"@en ;
  rdfs:label "Base of Oligocene"@en ;
.
gst:BaseOrdovician
  rdf:type gsog:Geologic_Time_Boundary ;
  rdfs:comment "Interval for grouping all specific instances of the Base of Ordovician"@en ;
  rdfs:label "Base of Ordovician"@en ;
.
gst:BaseOrosirian
  rdf:type gsog:GSSA ;
  rdfs:comment "Interval for grouping all specific instances of the Base of Orosirian"@en ;
  rdfs:label "Base of Orosirian"@en ;
.
gst:BaseOxfordian
  rdf:type gsog:Geologic_Time_Boundary ;
  gsoc:timeEquivalentTo gst:BaseUpperJurassic ;
  rdfs:label "shared boundary with BaseUpperJurassic"@en ;
.
gst:BasePaibian
  rdf:type gsog:Geologic_Time_Boundary ;
  gsoc:timeEquivalentTo gst:BaseFurongian ;
  rdfs:label "shared boundary with BaseFurongian"@en ;
.
gst:BasePaleoarchean
  rdf:type gsog:GSSA ;
  rdfs:comment "Interval for grouping all specific instances of the Base of Paleoarchean"@en ;
  rdfs:label "Base of Paleoarchean"@en ;
.
gst:BasePaleocene
  rdf:type gsog:Geologic_Time_Boundary ;
  gsoc:timeEquivalentTo gst:BaseCenozoic ;
  rdfs:label "shared boundary with BaseCenozoic"@en ;
.
gst:BasePaleogene
  rdf:type gsog:Geologic_Time_Boundary ;
  gsoc:timeEquivalentTo gst:BaseCenozoic ;
  rdfs:label "shared boundary with BaseCenozoic"@en ;
.
gst:BasePaleoproterozoic
  rdf:type gsog:GSSA ;
  gsoc:timeEquivalentTo gst:BaseProterozoic ;
  rdfs:label "shared boundary with BaseProterozoic"@en ;
.
gst:BasePaleozoic
  rdf:type gsog:Geologic_Time_Boundary ;
  gsoc:timeEquivalentTo gst:BasePhanerozoic ;
  rdfs:label "shared boundary with BasePhanerozoic"@en ;
.
gst:BasePennsylvanian
  rdf:type gsog:Geologic_Time_Boundary ;
  rdfs:comment "Interval for grouping all specific instances of the Base of Pennsylvanian"@en ;
  rdfs:label "Base of Pennsylvanian"@en ;
.
gst:BasePermian
  rdf:type gsog:Geologic_Time_Boundary ;
  rdfs:comment "Interval for grouping all specific instances of the Base of Permian"@en ;
  rdfs:label "Base of Permian"@en ;
.
gst:BasePhanerozoic
  rdf:type gsog:Geologic_Time_Boundary ;
  rdfs:comment "Interval for grouping all specific instances of the Base of Phanerozoic"@en ;
  rdfs:label "Base of Phanerozoic"@en ;
.
gst:BasePiacenzian
  rdf:type gsog:Geologic_Time_Boundary ;
  rdfs:comment "Interval for grouping all specific instances of the Base of Piacenzian"@en ;
  rdfs:label "Base of Piacenzian"@en ;
.
gst:BasePleistocene
  rdf:type gsog:Geologic_Time_Boundary ;
  gsoc:timeEquivalentTo gst:BaseCalabrian ;
  gsoc:timeEquivalentTo gst:BaseGelasian ;
  rdfs:label "shared boundary with BaseCalabrian"@en ;
  rdfs:label "shared boundary with BaseGelasian"@en ;
.
gst:BasePliensbachian
  rdf:type gsog:Geologic_Time_Boundary ;
  rdfs:comment "Interval for grouping all specific instances of the Base of Pliensbachian"@en ;
  rdfs:label "Base of Pliensbachian"@en ;
.
gst:BasePliocene
  rdf:type gsog:Geologic_Time_Boundary ;
  rdfs:comment "Interval for grouping all specific instances of the Base of Pliocene"@en ;
  rdfs:label "Base of Pliocene"@en ;
.
gst:BasePragian
  rdf:type gsog:Geologic_Time_Boundary ;
  rdfs:comment "Interval for grouping all specific instances of the Base of Pragian"@en ;
  rdfs:label "Base of Pragian"@en ;
.
gst:BasePrecambrian
  rdf:type gsog:GSSA ;
  gsoc:timeEquivalentTo gst:FormationoftheEarth ;
  rdfs:label "shared boundary with FormationoftheEarth"@en ;
.
gst:BasePriabonian
  rdf:type gsog:Geologic_Time_Boundary ;
  rdfs:comment "Interval for grouping all specific instances of the Base of Priabonian"@en ;
  rdfs:label "Base of Priabonian"@en ;
.
gst:BasePridoli
  rdf:type gsog:Geologic_Time_Boundary ;
  rdfs:comment "Interval for grouping all specific instances of the Base of Pridoli"@en ;
  rdfs:label "Base of Pridoli"@en ;
.
gst:BaseProterozoic
  rdf:type gsog:GSSA ;
  rdfs:comment "Interval for grouping all specific instances of the Base of Proterozoic"@en ;
  rdfs:label "Base of Proterozoic"@en ;
.
gst:BaseQuaternary
  rdf:type gsog:Geologic_Time_Boundary ;
  gsoc:timeEquivalentTo gst:BaseGelasian ;
  rdfs:label "shared boundary with BaseGelasian"@en ;
.
gst:BaseRhaetian
  rdf:type gsog:Geologic_Time_Boundary ;
  rdfs:comment "Interval for grouping all specific instances of the Base of Rhaetian"@en ;
  rdfs:label "Base of Rhaetian"@en ;
.
gst:BaseRhuddanian
  rdf:type gsog:Geologic_Time_Boundary ;
  gsoc:timeEquivalentTo gst:BaseSilurian ;
  rdfs:label "shared boundary with BaseSilurian"@en ;
.
gst:BaseRhyacian
  rdf:type gsog:GSSA ;
  rdfs:comment "Interval for grouping all specific instances of the Base of Rhyacian"@en ;
  rdfs:label "Base of Rhyacian"@en ;
.
gst:BaseRoadian
  rdf:type gsog:Geologic_Time_Boundary ;
  gsoc:timeEquivalentTo gst:BaseGuadalupian ;
  rdfs:label "shared boundary with BaseGuadalupian"@en ;
.
gst:BaseRupelian
  rdf:type gsog:Geologic_Time_Boundary ;
  gsoc:timeEquivalentTo gst:BaseOligocene ;
  rdfs:label "shared boundary with BaseOligocene"@en ;
.
gst:BaseSakmarian
  rdf:type gsog:Geologic_Time_Boundary ;
  rdfs:comment "Interval for grouping all specific instances of the Base of Sakmarian"@en ;
  rdfs:label "Base of Sakmarian"@en ;
.
gst:BaseSandbian
  rdf:type gsog:Geologic_Time_Boundary ;
  gsoc:timeEquivalentTo gst:BaseUpperOrdovician ;
  rdfs:label "shared boundary with BaseUpperOrdovician"@en ;
.
gst:BaseSantonian
  rdf:type gsog:Geologic_Time_Boundary ;
  rdfs:comment "Interval for grouping all specific instances of the Base of Santonian"@en ;
  rdfs:label "Base of Santonian"@en ;
.
gst:BaseSelandian
  rdf:type gsog:Geologic_Time_Boundary ;
  rdfs:comment "Interval for grouping all specific instances of the Base of Selandian"@en ;
  rdfs:label "Base of Selandian"@en ;
.
gst:BaseSerpukhovian
  rdf:type gsog:Geologic_Time_Boundary ;
  gsoc:timeEquivalentTo gst:BaseUpperMississippian ;
  rdfs:label "shared boundary with BaseUpperMississippian"@en ;
.
gst:BaseSerravallian
  rdf:type gsog:Geologic_Time_Boundary ;
  rdfs:comment "Interval for grouping all specific instances of the Base of Serravallian"@en ;
  rdfs:label "Base of Serravallian"@en ;
.
gst:BaseSheinwoodian
  rdf:type gsog:Geologic_Time_Boundary ;
  gsoc:timeEquivalentTo gst:BaseWenlock ;
  rdfs:label "Shared boundary with Base Wenlock "@en ;
.
gst:BaseSiderian
  rdf:type gsog:GSSA ;
  gsoc:timeEquivalentTo gst:BaseProterozoic ;
  rdfs:label "shared boundary with BaseProterozoic"@en ;
.
gst:BaseSilurian
  rdf:type gsog:Geologic_Time_Boundary ;
  rdfs:comment "Interval for grouping all specific instances of the Base of Silurian - Llandovery - Rhuddanian"@en ;
  rdfs:label "Base of Silurian - Llandovery - Rhuddanian"@en ;
.
gst:BaseSinemurian
  rdf:type gsog:Geologic_Time_Boundary ;
  rdfs:comment "Interval for grouping all specific instances of the Base of Sinemurian"@en ;
  rdfs:label "Base of Sinemurian"@en ;
.
gst:BaseStatherian
  rdf:type gsog:GSSA ;
  rdfs:comment "Interval for grouping all specific instances of the Base of Statherian"@en ;
  rdfs:label "Base of Statherian"@en ;
.
gst:BaseStenian
  rdf:type gsog:GSSA ;
  rdfs:comment "Interval for grouping all specific instances of the Base of Stenian"@en ;
  rdfs:label "Base of Stenian"@en ;
.
gst:BaseTelychian
  rdf:type gsog:Geologic_Time_Boundary ;
  rdfs:comment "Interval for grouping all specific instances of the Base of Telychian"@en ;
  rdfs:label "Base of Telychian"@en ;
.
gst:BaseTerreneuvian
  rdf:type gsog:Geologic_Time_Boundary ;
  gsoc:timeEquivalentTo gst:BasePhanerozoic ;
  rdfs:label "shared boundary with BasePhanerozoic"@en ;
.
gst:BaseThanetian
  rdf:type gsog:Geologic_Time_Boundary ;
  rdfs:comment "Interval for grouping all specific instances of the Base of Thanetian"@en ;
  rdfs:label "Base of Thanetian"@en ;
.
gst:BaseTithonian
  rdf:type gsog:Geologic_Time_Boundary ;
  rdfs:comment "Interval for grouping all specific instances of the Base of Tithonian"@en ;
  rdfs:label "Base of Tithonian"@en ;
.
gst:BaseToarcian
  rdf:type gsog:Geologic_Time_Boundary ;
  rdfs:comment "Interval for grouping all specific instances of the Base of Toarcian"@en ;
  rdfs:label "Base of Toarcian"@en ;
.
gst:BaseTonian
  rdf:type gsog:GSSA ;
  gsoc:timeEquivalentTo gst:BaseNeoproterozoic ;
  rdfs:label "shared boundary with BaseNeoproterozoic"@en ;
.
gst:BaseTortonian
  rdf:type gsog:Geologic_Time_Boundary ;
  rdfs:comment "Interval for grouping all specific instances of the Base of Tortonian"@en ;
  rdfs:label "Base of Tortonian"@en ;
.
gst:BaseTournaisian
  rdf:type gsog:Geologic_Time_Boundary ;
  gsoc:timeEquivalentTo gst:BaseCarboniferous ;
  rdfs:label "shared boundary with BaseCarboniferous"@en ;
.
gst:BaseTremadocian
  rdf:type gsog:Geologic_Time_Boundary ;
  gsoc:timeEquivalentTo gst:BaseOrdovician ;
  rdfs:label "shared boundary with BaseOrdovician"@en ;
.
gst:BaseTriassic
  rdf:type gsog:Geologic_Time_Boundary ;
  gsoc:timeEquivalentTo gst:BaseMesozoic ;
  rdfs:label "shared boundary with BaseMesozoic"@en ;
.
gst:BaseTuronian
  rdf:type gsog:Geologic_Time_Boundary ;
  rdfs:comment "Interval for grouping all specific instances of the Base of Turonian"@en ;
  rdfs:label "Base of Turonian"@en ;
.
gst:BaseUpperCretaceous
  rdf:type gsog:Geologic_Time_Boundary ;
  rdfs:comment "Interval for grouping all specific instances of the Base of Upper Cretaceous"@en ;
  rdfs:label "Base of Upper Cretaceous"@en ;
.
gst:BaseUpperDevonian
  rdf:type gsog:Geologic_Time_Boundary ;
  rdfs:comment "Interval for grouping all specific instances of the Base of Upper Devonian - Frasnian"@en ;
  rdfs:label "Base of Upper Devonian - Frasnian"@en ;
.
gst:BaseUpperJurassic
  rdf:type gsog:Geologic_Time_Boundary ;
  rdfs:comment "Interval for grouping all specific instances of the Base of Upper Jurassic"@en ;
  rdfs:label "Base of Upper Jurassic"@en ;
.
gst:BaseUpperMississippian
  rdf:type gsog:Geologic_Time_Boundary ;
  rdfs:comment "Interval for grouping all specific instances of the Base of Upper Mississippian"@en ;
  rdfs:label "Base of Upper Mississippian"@en ;
.
gst:BaseUpperOrdovician
  rdf:type gsog:Geologic_Time_Boundary ;
  rdfs:comment "Interval for grouping all specific instances of the Base of Upper Ordovician"@en ;
  rdfs:label "Base of Upper Ordovician"@en ;
.
gst:BaseUpperPennsylvanian
  rdf:type gsog:Geologic_Time_Boundary ;
  rdfs:comment "Interval for grouping all specific instances of the Base of Upper Pennsylvanian"@en ;
  rdfs:label "Base of Upper Pennsylvanian"@en ;
.
gst:BaseUpperPleistocene
  rdf:type gsog:Geologic_Time_Boundary ;
  rdfs:comment "Interval for grouping all specific instances of the Base of Upper Pleistocene"@en ;
  rdfs:label "Base of Upper Pleistocene"@en ;
.
gst:BaseUpperTriassic
  rdf:type gsog:Geologic_Time_Boundary ;
  rdfs:comment "Interval for grouping all specific instances of the Base of Upper Triassic"@en ;
  rdfs:label "Base of Upper Triassic"@en ;
.
gst:BaseValanginian
  rdf:type gsog:Geologic_Time_Boundary ;
  rdfs:comment "Interval for grouping all specific instances of the Base of Valanginian"@en ;
  rdfs:label "Base of Valanginian"@en ;
.
gst:BaseVisean
  rdf:type gsog:Geologic_Time_Boundary ;
  gsoc:timeEquivalentTo gst:BaseMiddleMississippian ;
  rdfs:label "shared boundary with BaseMiddleMississippian"@en ;
.
gst:BaseWenlock
  rdf:type gsog:Geologic_Time_Boundary ;
  rdfs:comment "Interval for grouping all specific instances of the Base of Wenlock - Sheinwoodian"@en ;
  rdfs:label "Base of Wenlock - Sheinwoodian"@en ;
.
gst:BaseWordian
  rdf:type gsog:Geologic_Time_Boundary ;
  rdfs:comment "Interval for grouping all specific instances of the Base of Wordian"@en ;
  rdfs:label "Base of Wordian"@en ;
.
gst:BaseWuchiapingian
  rdf:type gsog:Geologic_Time_Boundary ;
  gsoc:timeEquivalentTo gst:BaseLopingian ;
  rdfs:label "shared boundary with BaseLopingian"@en ;
.
gst:BaseWuliuanAge
  rdf:type gsog:Geologic_Time_Boundary ;
  gsoc:timeEquivalentTo gst:BaseCambrianSeries3 ;
  gsoc:timeStarts gst:BaseCambrianSeries3 ;
  rdfs:comment "Interval for grouping all specific instances of the Base of Wuliuan Age"@en ;
  rdfs:label "Base of Wuliuan Age"@en ;
  rdfs:label "shared boundary with BaseCambrianSeries3"@en ;
.
gst:BaseYpresian
  rdf:type gsog:Geologic_Time_Boundary ;
  gsoc:timeEquivalentTo gst:BaseEocene ;
  rdfs:label "shared boundary with BaseEocene"@en ;
.
gst:BaseZanclean
  rdf:type gsog:Geologic_Time_Boundary ;
  gsoc:timeEquivalentTo gst:BasePliocene ;
  rdfs:label "shared boundary with BasePliocene"@en ;
.
gst:BashkirianAge
  rdf:type gst:Age ;
  rdf:type gsog:Generic_Geologic_Time_Unit ;
  gsoc:timeStarts gst:BasePennsylvanian ;
  rdfs:comment "Interval for grouping all specific instances of the Bashkirian Age"@en ;
  rdfs:label "Bashkirian Age"@en ;
.
gst:BathonianAge
  rdf:type gst:Age ;
  rdf:type gsog:Generic_Geologic_Time_Unit ;
  gsoc:timeStarts gst:BaseBathonian ;
  rdfs:comment "Interval for grouping all specific instances of the Bathonian Age"@en ;
  rdfs:label "Bathonian Age"@en ;
.
gst:BerriasianAge
  rdf:type gst:Age ;
  rdf:type gsog:Generic_Geologic_Time_Unit ;
  gsoc:timeStarts gst:BaseCretaceous ;
  rdfs:comment "Interval for grouping all specific instances of the Berriasian Age"@en ;
  rdfs:label "Berriasian Age"@en ;
.
gst:BurdigalianAge
  rdf:type gst:Age ;
  rdf:type gsog:Generic_Geologic_Time_Unit ;
  gsoc:timeStarts gst:BaseBurdigalian ;
  rdfs:comment "Interval for grouping all specific instances of the Burdigalian Age"@en ;
  rdfs:label "Burdigalian Age"@en ;
.
gst:CalabrianAge
  rdf:type gst:Age ;
  rdf:type gsog:Generic_Geologic_Time_Unit ;
  gsoc:timeStarts gst:BaseCalabrian ;
  rdfs:comment "Interval for grouping all specific instances of the Calabrian Age"@en ;
  rdfs:label "Calabrian Age"@en ;
.
gst:CallovianAge
  rdf:type gst:Age ;
  rdf:type gsog:Generic_Geologic_Time_Unit ;
  gsoc:timeStarts gst:BaseCallovian ;
  rdfs:comment "Interval for grouping all specific instances of the Callovian Age"@en ;
  rdfs:label "Callovian Age"@en ;
.
gst:CalymmianPeriod
  rdf:type gst:Period ;
  rdf:type gsog:Generic_Geologic_Time_Unit ;
  gsoc:timeStarts gst:BaseMesoproterozoic ;
  rdfs:comment "Interval for grouping all specific instances of the Calymmian Period"@en ;
  rdfs:label "Calymmian Period"@en ;
.
gst:CambrianPeriod
  rdf:type gst:Period ;
  rdf:type gsog:Generic_Geologic_Time_Unit ;
  gsoc:timeStarts gst:BasePhanerozoic ;
  rdfs:comment "Interval for grouping all specific instances of the Cambrian Period"@en ;
  rdfs:label "Cambrian Period"@en ;
.
gst:CambrianSeries2Epoch
  rdf:type gst:Epoch ;
  rdf:type gsog:Generic_Geologic_Time_Unit ;
  gsoc:timeStarts gst:BaseCambrianSeries2 ;
  rdfs:comment "Interval for grouping all specific instances of the Cambrian Series 2 Epoch"@en ;
  rdfs:label "Cambrian Series 2 Epoch"@en ;
.
gst:CambrianSeries3Epoch
  rdf:type gst:Epoch ;
  rdf:type gsog:Generic_Geologic_Time_Unit ;
  gsoc:timeStarts gst:BaseCambrianSeries3 ;
  rdfs:comment "Interval for grouping all specific instances of the Cambrian Series 3 Epoch"@en ;
  rdfs:label "Cambrian Series 3 Epoch"@en ;
.
gst:CambrianStage10Age
  rdf:type gst:Age ;
  rdf:type gsog:Generic_Geologic_Time_Unit ;
  gsoc:timeStarts gst:BaseCambrianStage10 ;
  rdfs:comment "Interval for grouping all specific instances of the Cambrian Stage 10 Age"@en ;
  rdfs:label "Cambrian Stage 10 Age"@en ;
.
gst:CambrianStage2Age
  rdf:type gst:Age ;
  rdf:type gsog:Generic_Geologic_Time_Unit ;
  gsoc:timeStarts gst:BaseCambrianStage2 ;
  rdfs:comment "Interval for grouping all specific instances of the Cambrian Stage 2 Age"@en ;
  rdfs:label "Cambrian Stage 2 Age"@en ;
.
gst:CambrianStage3Age
  rdf:type gst:Age ;
  rdf:type gsog:Generic_Geologic_Time_Unit ;
  gsoc:timeStarts gst:BaseCambrianSeries2 ;
  rdfs:comment "Interval for grouping all specific instances of the Cambrian Stage 3 Age"@en ;
  rdfs:label "Cambrian Stage 3 Age"@en ;
.
gst:CambrianStage4Age
  rdf:type gst:Age ;
  rdf:type gsog:Generic_Geologic_Time_Unit ;
  gsoc:timeStarts gst:BaseCambrianStage4 ;
  rdfs:comment "Interval for grouping all specific instances of the Cambrian Stage 4 Age"@en ;
  rdfs:label "Cambrian Stage 4 Age"@en ;
.
gst:CambrianStage5Age
  rdf:type gst:Age ;
  rdf:type gsog:Generic_Geologic_Time_Unit ;
  gsoc:timeStarts gst:BaseCambrianSeries3 ;
  rdfs:comment "Interval for grouping all specific instances of the Cambrian Stage 5 Age"@en ;
  rdfs:label "Cambrian Stage 5 Age"@en ;
.
gst:CampanianAge
  rdf:type gst:Age ;
  rdf:type gsog:Generic_Geologic_Time_Unit ;
  gsoc:timeStarts gst:BaseCampanian ;
  rdfs:comment "Interval for grouping all specific instances of the Campanian Age"@en ;
  rdfs:label "Campanian Age"@en ;
.
gst:CapitanianAge
  rdf:type gst:Age ;
  rdf:type gsog:Generic_Geologic_Time_Unit ;
  gsoc:timeStarts gst:BaseCapitanian ;
  rdfs:comment "Interval for grouping all specific instances of the Capitanian Age"@en ;
  rdfs:label "Capitanian Age"@en ;
.
gst:CarboniferousPeriod
  rdf:type gst:Period ;
  rdf:type gsog:Generic_Geologic_Time_Unit ;
  gsoc:timeStarts gst:BaseCarboniferous ;
  rdfs:comment "Interval for grouping all specific instances of the Carboniferous Period"@en ;
  rdfs:label "Carboniferous Period"@en ;
.
gst:CarnianAge
  rdf:type gst:Age ;
  rdf:type gsog:Generic_Geologic_Time_Unit ;
  gsoc:timeStarts gst:BaseUpperTriassic ;
  rdfs:comment "Interval for grouping all specific instances of the Carnian Age"@en ;
  rdfs:label "Carnian Age"@en ;
.
gst:CenomanianAge
  rdf:type gst:Age ;
  rdf:type gsog:Generic_Geologic_Time_Unit ;
  gsoc:timeStarts gst:BaseUpperCretaceous ;
  rdfs:comment "Interval for grouping all specific instances of the Cenomanian Age"@en ;
  rdfs:label "Cenomanian Age"@en ;
.
gst:CenozoicEra
  rdf:type gst:Era ;
  rdf:type gsog:Generic_Geologic_Time_Unit ;
  gsoc:timeStarts gst:BaseCenozoic ;
  rdfs:comment "Interval for grouping all specific instances of the Cenozoic Era"@en ;
  rdfs:label "Cenozoic Era"@en ;
.
gst:ChanghsingianAge
  rdf:type gst:Age ;
  rdf:type gsog:Generic_Geologic_Time_Unit ;
  gsoc:timeStarts gst:BaseChanghsingian ;
  rdfs:comment "Interval for grouping all specific instances of the Changhsingian Age"@en ;
  rdfs:label "Changhsingian Age"@en ;
.
gst:ChattianAge
  rdf:type gst:Age ;
  rdf:type gsog:Generic_Geologic_Time_Unit ;
  gsoc:timeStarts gst:BaseChattian ;
  rdfs:comment "Interval for grouping all specific instances of the Chattian Age"@en ;
  rdfs:label "Chattian Age"@en ;
.
gst:ChibanianAge
  rdf:type gst:Age ;
  rdf:type gsog:Generic_Geologic_Time_Unit ;
  gsoc:timeStarts gst:BaseChibanianStage ;
  rdfs:comment "Interval for grouping all specific instances of the Chibanian Age"@en ;
  rdfs:label "Chibanian Age"@en ;
.
gst:CisuralianEpoch
  rdf:type gst:Epoch ;
  rdf:type gsog:Generic_Geologic_Time_Unit ;
  gsoc:timeStarts gst:BasePermian ;
  rdfs:comment "Interval for grouping all specific instances of the Cisuralian Epoch"@en ;
  rdfs:label "Cisuralian Epoch"@en ;
.
gst:ConiacianAge
  rdf:type gst:Age ;
  rdf:type gsog:Generic_Geologic_Time_Unit ;
  gsoc:timeStarts gst:BaseConiacian ;
  rdfs:comment "Interval for grouping all specific instances of the Coniacian Age"@en ;
  rdfs:label "Coniacian Age"@en ;
.
gst:CretaceousPeriod
  rdf:type gst:Period ;
  rdf:type gsog:Generic_Geologic_Time_Unit ;
  gsoc:timeStarts gst:BaseCretaceous ;
  rdfs:comment "Interval for grouping all specific instances of the Cretaceous Period"@en ;
  rdfs:label "Cretaceous Period"@en ;
.
gst:CryogenianPeriod
  rdf:type gst:Period ;
  rdf:type gsog:Generic_Geologic_Time_Unit ;
  gsoc:timeStarts gst:BaseCryogenian ;
  rdfs:comment "Interval for grouping all specific instances of the Cryogenian Period"@en ;
  rdfs:label "Cryogenian Period"@en ;
.
gst:DanianAge
  rdf:type gst:Age ;
  rdf:type gsog:Generic_Geologic_Time_Unit ;
  gsoc:timeStarts gst:BaseCenozoic ;
  rdfs:comment "Interval for grouping all specific instances of the Danian Age"@en ;
  rdfs:label "Danian Age"@en ;
.
gst:DapingianAge
  rdf:type gst:Age ;
  rdf:type gsog:Generic_Geologic_Time_Unit ;
  gsoc:timeStarts gst:BaseMiddleOrdovician ;
  rdfs:comment "Interval for grouping all specific instances of the Dapingian Age"@en ;
  rdfs:label "Dapingian Age"@en ;
.
gst:DarriwilianAge
  rdf:type gst:Age ;
  rdf:type gsog:Generic_Geologic_Time_Unit ;
  gsoc:timeStarts gst:BaseDarriwillian ;
  rdfs:comment "Interval for grouping all specific instances of the Darriwilian Age"@en ;
  rdfs:label "Darriwilian Age"@en ;
.
gst:DevonianPeriod
  rdf:type gst:Period ;
  rdf:type gsog:Generic_Geologic_Time_Unit ;
  gsoc:timeStarts gst:BaseDevonian ;
  rdfs:comment "Interval for grouping all specific instances of the Devonian Period"@en ;
  rdfs:label "Devonian Period"@en ;
.
gst:DrumianAge
  rdf:type gst:Age ;
  rdf:type gsog:Generic_Geologic_Time_Unit ;
  gsoc:timeStarts gst:BaseDrumian ;
  rdfs:comment "Interval for grouping all specific instances of the Drumian Age"@en ;
  rdfs:label "Drumian Age"@en ;
.
gst:EctasianPeriod
  rdf:type gst:Period ;
  rdf:type gsog:Generic_Geologic_Time_Unit ;
  gsoc:timeStarts gst:BaseEctasian ;
  rdfs:comment "Interval for grouping all specific instances of the Ectasian Period"@en ;
  rdfs:label "Ectasian Period"@en ;
.
gst:EdiacaranPeriod
  rdf:type gst:Period ;
  rdf:type gsog:Generic_Geologic_Time_Unit ;
  gsoc:timeStarts gst:BaseEdiacaran ;
  rdfs:comment "Interval for grouping all specific instances of the Ediacaran Period"@en ;
  rdfs:label "Ediacaran Period"@en ;
.
gst:EifelianAge
  rdf:type gst:Age ;
  rdf:type gsog:Generic_Geologic_Time_Unit ;
  gsoc:timeStarts gst:BaseMiddleDevonian ;
  rdfs:comment "Interval for grouping all specific instances of the Eifelian Age"@en ;
  rdfs:label "Eifelian Age"@en ;
.
gst:EmsianAge
  rdf:type gst:Age ;
  rdf:type gsog:Generic_Geologic_Time_Unit ;
  gsoc:timeStarts gst:BaseEmsian ;
  rdfs:comment "Interval for grouping all specific instances of the Emsian Age"@en ;
  rdfs:label "Emsian Age"@en ;
.
gst:EoarcheanEra
  rdf:type gst:Era ;
  rdf:type gsog:Generic_Geologic_Time_Unit ;
  gsoc:timeStarts gst:BaseArchean ;
  rdfs:comment "Interval for grouping all specific instances of the Eoarchean Era"@en ;
  rdfs:label "Eoarchean Era"@en ;
.
gst:EoceneEpoch
  rdf:type gst:Epoch ;
  rdf:type gsog:Generic_Geologic_Time_Unit ;
  gsoc:timeStarts gst:BaseEocene ;
  rdfs:comment "Interval for grouping all specific instances of the Eocene Epoch"@en ;
  rdfs:label "Eocene Epoch"@en ;
.
gst:Eon
  rdf:type owl:Class ;
  rdfs:comment "How will this be defined?  Must contain at least one Era and have duration longer than some Era?"@en ;
  rdfs:subClassOf gsog:Geologic_Time_Interval ;
  rdfs:subClassOf [
      rdf:type owl:Restriction ;
      owl:allValuesFrom [
          rdf:type owl:Class ;
          owl:complementOf [
              rdf:type owl:Class ;
              owl:unionOf (
                  gst:Era
                  gst:Period
                  gst:Subperiod
                  gst:Epoch
                  gst:Age
                ) ;
            ] ;
        ] ;
      owl:onProperty gsoc:timeDuring ;
    ] ;
  rdfs:subClassOf [
      rdf:type owl:Restriction ;
      owl:allValuesFrom [
          rdf:type owl:Class ;
          owl:complementOf [
              rdf:type owl:Class ;
              owl:unionOf (
                  gst:Supereon
                  gst:Eon
                ) ;
            ] ;
        ] ;
      owl:onProperty gsoc:timeContains ;
    ] ;
  rdfs:subClassOf [
      rdf:type owl:Restriction ;
      owl:onProperty gsoc:hostedBy ;
      owl:someValuesFrom gsgu:Eonothem ;
    ] ;
.
gst:Epoch
  rdf:type owl:Class ;
  rdfs:comment "An Epoch may be subdivided into Ages. Epochs are grouped into Periods. Example epochs: Eocene, Pleistocene"@en ;
  rdfs:label "Epoch"@en ;
  rdfs:subClassOf gsog:Geologic_Time_Interval ;
  rdfs:subClassOf [
      rdf:type owl:Restriction ;
      owl:allValuesFrom [
          rdf:type owl:Class ;
          owl:complementOf [
              rdf:type owl:Class ;
              owl:unionOf (
                  gst:Epoch
                  gst:Age
                ) ;
            ] ;
        ] ;
      owl:onProperty gsoc:timeIncludedBy ;
    ] ;
  rdfs:subClassOf [
      rdf:type owl:Restriction ;
      owl:allValuesFrom [
          rdf:type owl:Class ;
          owl:complementOf [
              rdf:type owl:Class ;
              owl:unionOf (
                  gst:Epoch
                  gst:Period
                  gst:Subperiod
                  gst:Era
                  gst:Eon
                  gst:Supereon
                ) ;
            ] ;
        ] ;
      owl:onProperty gsoc:timeIncludes ;
    ] ;
  rdfs:subClassOf [
      rdf:type owl:Restriction ;
      owl:onProperty gsoc:hostedBy ;
      owl:someValuesFrom gsgu:Series ;
    ] ;
.
gst:Era
  rdf:type owl:Class ;
  rdfs:comment "Named rank for geochronologic time interval. An Era may be subdivided into Periods. Eras are grouped into Eons"@en ;
  rdfs:subClassOf gsog:Geologic_Time_Interval ;
  rdfs:subClassOf [
      rdf:type owl:Restriction ;
      owl:allValuesFrom [
          rdf:type owl:Class ;
          owl:complementOf [
              rdf:type owl:Class ;
              owl:unionOf (
                  gst:Era
                  gst:Eon
                  gst:Supereon
                ) ;
            ] ;
        ] ;
      owl:onProperty gsoc:timeContains ;
    ] ;
  rdfs:subClassOf [
      rdf:type owl:Restriction ;
      owl:allValuesFrom [
          rdf:type owl:Class ;
          owl:complementOf [
              rdf:type owl:Class ;
              owl:unionOf (
                  gst:Era
                  gst:Period
                  gst:Subperiod
                  gst:Epoch
                  gst:Age
                ) ;
            ] ;
        ] ;
      owl:onProperty gsoc:timeDuring ;
    ] ;
  rdfs:subClassOf [
      rdf:type owl:Restriction ;
      owl:onProperty gsoc:hostedBy ;
      owl:someValuesFrom gsgu:Erathem ;
    ] ;
.
gst:FamennianAge
  rdf:type gst:Age ;
  rdf:type gsog:Generic_Geologic_Time_Unit ;
  gsoc:timeStarts gst:BaseFamennian ;
  rdfs:comment "Interval for grouping all specific instances of the Famennian Age"@en ;
  rdfs:label "Famennian Age"@en ;
.
gst:FloianAge
  rdf:type gst:Age ;
  rdf:type gsog:Generic_Geologic_Time_Unit ;
  gsoc:timeStarts gst:BaseFloian ;
  rdfs:comment "Interval for grouping all specific instances of the Floian Age"@en ;
  rdfs:label "Floian Age"@en ;
.
gst:FormationoftheEarth
  rdf:type gsog:Geologic_Time_Date ;
  gsoc:timeStarts gst:FormationoftheEarth ;
  rdfs:comment "Interval for grouping all specific instances of the Formation of the Earth"@en ;
  rdfs:label "Formation of the Earth"@en ;
.
gst:FortunianAge
  rdf:type gst:Age ;
  rdf:type gsog:Generic_Geologic_Time_Unit ;
  gsoc:timeStarts gst:BasePhanerozoic ;
  rdfs:comment "Fortunian is the earliest of the five Siberian Early Cambrian ages, and also the most recently recognized. The stage and its equivalents were only added to the Cambrian in 1992. http://palaeos.com/paleozoic/cambrian/fortunian.html"@en ;
  rdfs:comment "Interval for grouping all specific instances of the Fortunian Age"@en ;
  rdfs:comment "The name 'Fortunian Stage' is proposed as the lowest stage of the Cambrian and the lower part of the proposed Terreneuvian Series. The base of the Fortunian Stage corresponds to the defined GSSP for the base of the Cambrian (FAD of Trichophycus pedum and base of the T. pedum Zone [ichnofossils] in the Fortune Head section, Burin Peninsula, Newfoundland, Canada). Its top will be defined by the base of the overlying stage, which is presently undefined. Prepared by E. Landing for ISCS, January 2007; http://www.palaeontology.geo.uu.se/ISCS/ISCS_Terreneuvian_Fortunian_2007.pdf"@en ;
  rdfs:label "Fortunian Age"@en ;
.
gst:FrasnianAge
  rdf:type gst:Age ;
  rdf:type gsog:Generic_Geologic_Time_Unit ;
  gsoc:timeStarts gst:BaseUpperDevonian ;
  rdfs:comment "Interval for grouping all specific instances of the Frasnian Age"@en ;
  rdfs:label "Frasnian Age"@en ;
.
gst:FurongianEpoch
  rdf:type gst:Epoch ;
  rdf:type gsog:Generic_Geologic_Time_Unit ;
  gsoc:timeStarts gst:BaseFurongian ;
  rdfs:comment "Interval for grouping all specific instances of the Furongian Epoch"@en ;
  rdfs:label "Furongian Epoch"@en ;
.
gst:GelasianAge
  rdf:type gst:Age ;
  rdf:type gsog:Generic_Geologic_Time_Unit ;
  gsoc:timeStarts gst:BaseGelasian ;
  rdfs:comment "Interval for grouping all specific instances of the Gelasian Age"@en ;
  rdfs:label "Gelasian Age"@en ;
.
gst:GivetianAge
  rdf:type gst:Age ;
  rdf:type gsog:Generic_Geologic_Time_Unit ;
  gsoc:timeStarts gst:BaseGivetian ;
  rdfs:comment "Interval for grouping all specific instances of the Givetian Age"@en ;
  rdfs:label "Givetian Age"@en ;
.
gst:GorstianAge
  rdf:type gst:Age ;
  rdf:type gsog:Generic_Geologic_Time_Unit ;
  gsoc:timeStarts gst:BaseLudlow ;
  rdfs:comment "Interval for grouping all specific instances of the Gorstian Age"@en ;
  rdfs:label "Gorstian Age"@en ;
.
gst:GreenlandianAge
  rdf:type gst:Age ;
  rdf:type gsog:Generic_Geologic_Time_Unit ;
  gsoc:timeStarts gst:BaseHolocene ;
  rdfs:comment "Interval for grouping all specific instances of the Greenlandian Age"@en ;
  rdfs:label "Greenlandian Age"@en ;
.
gst:GuadalupianEpoch
  rdf:type gst:Epoch ;
  rdf:type gsog:Generic_Geologic_Time_Unit ;
  gsoc:timeStarts gst:BaseGuadalupian ;
  rdfs:comment "Interval for grouping all specific instances of the Guadalupian Epoch"@en ;
  rdfs:label "Guadalupian Epoch"@en ;
.
gst:GuzhangianAge
  rdf:type gst:Age ;
  rdf:type gsog:Generic_Geologic_Time_Unit ;
  gsoc:timeStarts gst:BaseGuzhangian ;
  rdfs:comment "Interval for grouping all specific instances of the Guzhangian Age"@en ;
  rdfs:label "Guzhangian Age"@en ;
.
gst:GzhelianAge
  rdf:type gst:Age ;
  rdf:type gsog:Generic_Geologic_Time_Unit ;
  gsoc:timeStarts gst:BaseGzhelian ;
  rdfs:comment "Interval for grouping all specific instances of the Gzhelian Age"@en ;
  rdfs:label "Gzhelian Age"@en ;
.
gst:HadeanEon
  rdf:type gst:Eon ;
  rdf:type gsog:Generic_Geologic_Time_Unit ;
  gsoc:timeStarts gst:FormationoftheEarth ;
  rdfs:comment "Interval for grouping all specific instances of the Hadean Eon"@en ;
  rdfs:label "Hadean Eon"@en ;
.
gst:HauterivianAge
  rdf:type gst:Age ;
  rdf:type gsog:Generic_Geologic_Time_Unit ;
  gsoc:timeStarts gst:BaseHauterivian ;
  rdfs:comment "Interval for grouping all specific instances of the Hauterivian Age"@en ;
  rdfs:label "Hauterivian Age"@en ;
.
gst:HettangianAge
  rdf:type gst:Age ;
  rdf:type gsog:Generic_Geologic_Time_Unit ;
  gsoc:timeStarts gst:BaseJurassic ;
  rdfs:comment "Interval for grouping all specific instances of the Hettangian Age"@en ;
  rdfs:label "Hettangian Age"@en ;
.
gst:HirnantianAge
  rdf:type gst:Age ;
  rdf:type gsog:Generic_Geologic_Time_Unit ;
  gsoc:timeStarts gst:BaseHirnantian ;
  rdfs:comment "Interval for grouping all specific instances of the Hirnantian Age"@en ;
  rdfs:label "Hirnantian Age"@en ;
.
gst:HoloceneEpoch
  rdf:type gst:Epoch ;
  rdf:type gsog:Generic_Geologic_Time_Unit ;
  gsoc:timeStarts gst:BaseHolocene ;
  rdfs:comment "Interval for grouping all specific instances of the Holocene Epoch"@en ;
  rdfs:label "Holocene Epoch"@en ;
.
gst:HomerianAge
  rdf:type gst:Age ;
  rdf:type gsog:Generic_Geologic_Time_Unit ;
  gsoc:timeStarts gst:BaseHomerian ;
  rdfs:comment "Interval for grouping all specific instances of the Homerian Age"@en ;
  rdfs:label "Homerian Age"@en ;
.
gst:InduanAge
  rdf:type gst:Age ;
  rdf:type gsog:Generic_Geologic_Time_Unit ;
  gsoc:timeStarts gst:BaseMesozoic ;
  rdfs:comment "Interval for grouping all specific instances of the Induan Age"@en ;
  rdfs:label "Induan Age"@en ;
.
gst:JiangshanianAge
  rdf:type gst:Age ;
  rdf:type gsog:Generic_Geologic_Time_Unit ;
  gsoc:timeStarts gst:BaseJiangshanian ;
  rdfs:comment "Interval for grouping all specific instances of the Jiangshanian Age"@en ;
  rdfs:label "Jiangshanian Age"@en ;
.
gst:JurassicPeriod
  rdf:type gst:Period ;
  rdf:type gsog:Generic_Geologic_Time_Unit ;
  gsoc:timeDuring gst:MesozoicEra ;
  gsoc:timeContains gst:MiddleJurassicEpoch ;
  gsoc:timeStartedBy gst:LowerJurassicEpoch ;
  gsoc:timeStarts gst:BaseJurassic ;
  gsoc:timeFinishedBy gst:UpperJurassicEpoch ;
  gsoc:nextTimeInterval gst:BerriasianAge ;
  gsoc:nextTimeInterval gst:CretaceousPeriod ;
  gsoc:nextTimeInterval gst:LowerCretaceousEpoch ;
  gsoc:previousTimeInterval gst:RhaetianAge ;
  gsoc:previousTimeInterval gst:TriassicPeriod ;
  gsoc:previousTimeInterval gst:UpperTriassicEpoch ;
  rdfs:comment "Interval for grouping all specific instances of the Jurassic Period"@en ;
  rdfs:label "Jurassic Period"@en ;
.
gst:KasimovianAge
  rdf:type gst:Age ;
  rdf:type gsog:Generic_Geologic_Time_Unit ;
  gsoc:timeStarts gst:BaseUpperPennsylvanian ;
  rdfs:comment "Interval for grouping all specific instances of the Kasimovian Age"@en ;
  rdfs:label "Kasimovian Age"@en ;
.
gst:KatianAge
  rdf:type gst:Age ;
  rdf:type gsog:Generic_Geologic_Time_Unit ;
  gsoc:timeStarts gst:BaseKatian ;
  rdfs:comment "Interval for grouping all specific instances of the Katian Age"@en ;
  rdfs:label "Katian Age"@en ;
.
gst:KimmeridgianAge
  rdf:type gst:Age ;
  rdf:type gsog:Generic_Geologic_Time_Unit ;
  gsoc:timeStarts gst:BaseKimmeridgian ;
  rdfs:comment "Interval for grouping all specific instances of the Kimmeridgian Age"@en ;
  rdfs:label "Kimmeridgian Age"@en ;
.
gst:KungurianAge
  rdf:type gst:Age ;
  rdf:type gsog:Generic_Geologic_Time_Unit ;
  gsoc:timeStarts gst:BaseKungurian ;
  rdfs:comment "Interval for grouping all specific instances of the Kungurian Age"@en ;
  rdfs:label "Kungurian Age"@en ;
.
gst:LadinianAge
  rdf:type gst:Age ;
  rdf:type gsog:Generic_Geologic_Time_Unit ;
  gsoc:timeStarts gst:BaseLadinian ;
  rdfs:comment "Interval for grouping all specific instances of the Ladinian Age"@en ;
  rdfs:label "Ladinian Age"@en ;
.
gst:LanghianAge
  rdf:type gst:Age ;
  rdf:type gsog:Generic_Geologic_Time_Unit ;
  gsoc:timeStarts gst:BaseLanghian ;
  rdfs:comment "Interval for grouping all specific instances of the Langhian Age"@en ;
  rdfs:label "Langhian Age"@en ;
.
gst:LlandoveryEpoch
  rdf:type gst:Epoch ;
  rdf:type gsog:Generic_Geologic_Time_Unit ;
  gsoc:timeStarts gst:BaseSilurian ;
  rdfs:comment "Interval for grouping all specific instances of the Llandovery Epoch"@en ;
  rdfs:label "Llandovery Epoch"@en ;
.
gst:LochkovianAge
  rdf:type gst:Age ;
  rdf:type gsog:Generic_Geologic_Time_Unit ;
  gsoc:timeStarts gst:BaseDevonian ;
  rdfs:comment "Interval for grouping all specific instances of the Lochkovian Age"@en ;
  rdfs:label "Lochkovian Age"@en ;
.
gst:LopingianEpoch
  rdf:type gst:Epoch ;
  rdf:type gsog:Generic_Geologic_Time_Unit ;
  gsoc:timeStarts gst:BaseLopingian ;
  rdfs:comment "Interval for grouping all specific instances of the Lopingian Epoch"@en ;
  rdfs:label "Lopingian Epoch"@en ;
.
gst:LowerCambrianEpoch
  rdf:type gst:Epoch ;
  rdf:type gsog:Generic_Geologic_Time_Unit ;
  gsoc:timeStarts gst:BasePhanerozoic ;
  rdfs:comment "Interval for grouping all specific instances of the Lower Cambrian Epoch"@en ;
  rdfs:label "Lower Cambrian Epoch"@en ;
.
gst:LowerCretaceousEpoch
  rdf:type gst:Epoch ;
  rdf:type gsog:Generic_Geologic_Time_Unit ;
  gsoc:timeStarts gst:BaseCretaceous ;
  rdfs:comment "Interval for grouping all specific instances of the Lower Cretaceous Epoch"@en ;
  rdfs:label "Lower Cretaceous Epoch"@en ;
.
gst:LowerDevonianEpoch
  rdf:type gst:Epoch ;
  rdf:type gsog:Generic_Geologic_Time_Unit ;
  gsoc:timeStarts gst:BaseDevonian ;
  rdfs:comment "Interval for grouping all specific instances of the Lower Devonian Epoch"@en ;
  rdfs:label "Lower Devonian Epoch"@en ;
.
gst:LowerJurassicEpoch
  rdf:type gst:Epoch ;
  rdf:type gsog:Generic_Geologic_Time_Unit ;
  gsoc:timeStarts gst:BaseJurassic ;
  rdfs:comment "Interval for grouping all specific instances of the Lower Jurassic Epoch"@en ;
  rdfs:label "Lower Jurassic Epoch"@en ;
.
gst:LowerMississippianEpoch
  rdf:type gst:Epoch ;
  rdf:type gsog:Generic_Geologic_Time_Unit ;
  gsoc:timeStarts gst:BaseCarboniferous ;
  rdfs:comment "Interval for grouping all specific instances of the Lower Mississippian Epoch"@en ;
  rdfs:label "Lower Mississippian Epoch"@en ;
.
gst:LowerOrdovicianEpoch
  rdf:type gst:Epoch ;
  rdf:type gsog:Generic_Geologic_Time_Unit ;
  gsoc:timeStarts gst:BaseOrdovician ;
  rdfs:comment "Interval for grouping all specific instances of the Lower Ordovician Epoch"@en ;
  rdfs:label "Lower Ordovician Epoch"@en ;
.
gst:LowerPennsylvanianEpoch
  rdf:type gst:Epoch ;
  rdf:type gsog:Generic_Geologic_Time_Unit ;
  gsoc:timeStarts gst:BasePennsylvanian ;
  rdfs:comment "Interval for grouping all specific instances of the Lower Pennsylvanian Epoch"@en ;
  rdfs:label "Lower Pennsylvanian Epoch"@en ;
.
gst:LowerTriassicEpoch
  rdf:type gst:Epoch ;
  rdf:type gsog:Generic_Geologic_Time_Unit ;
  gsoc:timeStarts gst:BaseMesozoic ;
  rdfs:comment "Interval for grouping all specific instances of the Lower Triassic Epoch"@en ;
  rdfs:label "Lower Triassic Epoch"@en ;
.
gst:LudfordianAge
  rdf:type gst:Age ;
  rdf:type gsog:Generic_Geologic_Time_Unit ;
  gsoc:timeStarts gst:BaseLudfordianStage ;
  rdfs:comment "Interval for grouping all specific instances of the Ludfordian Age"@en ;
  rdfs:label "Ludfordian Age"@en ;
.
gst:LudlowEpoch
  rdf:type gst:Epoch ;
  rdf:type gsog:Generic_Geologic_Time_Unit ;
  gsoc:timeStarts gst:BaseLudlow ;
  rdfs:comment "Interval for grouping all specific instances of the Ludlow Epoch"@en ;
  rdfs:label "Ludlow Epoch"@en ;
.
gst:LutetianAge
  rdf:type gst:Age ;
  rdf:type gsog:Generic_Geologic_Time_Unit ;
  rdfs:comment "Interval for grouping all specific instances of the Lutetian Age"@en ;
  rdfs:label "Lutetian Age"@en ;
.
gst:MaastrichtianAge
  rdf:type gst:Age ;
  rdf:type gsog:Generic_Geologic_Time_Unit ;
  gsoc:timeStarts gst:BaseMaastrichtian ;
  rdfs:comment "Interval for grouping all specific instances of the Maastrichtian Age"@en ;
  rdfs:label "Maastrichtian Age"@en ;
.
gst:MeghalayanAge
  rdf:type gst:Age ;
  rdf:type gsog:Generic_Geologic_Time_Unit ;
  gsoc:timeStarts gst:BaseMeghalayan ;
  rdfs:comment "Interval for grouping all specific instances of the Meghalayan Age"@en ;
  rdfs:label "Meghalayan Age"@en ;
.
gst:MesoarcheanEra
  rdf:type gst:Era ;
  rdf:type gsog:Generic_Geologic_Time_Unit ;
  gsoc:timeStarts gst:BaseMesoarchean ;
  rdfs:comment "Interval for grouping all specific instances of the Mesoarchean Era"@en ;
  rdfs:label "Mesoarchean Era"@en ;
.
gst:MesoproterozoicEra
  rdf:type gst:Era ;
  rdf:type gsog:Generic_Geologic_Time_Unit ;
  gsoc:timeStarts gst:BaseMesoproterozoic ;
  rdfs:comment "Interval for grouping all specific instances of the Mesoproterozoic Era"@en ;
  rdfs:label "Mesoproterozoic Era"@en ;
.
gst:MesozoicEra
  rdf:type gst:Era ;
  rdf:type gsog:Generic_Geologic_Time_Unit ;
  gsoc:timeStarts gst:BaseMesozoic ;
  rdfs:comment "Interval for grouping all specific instances of the Mesozoic Era"@en ;
  rdfs:label "Mesozoic Era"@en ;
.
gst:MessinianAge
  rdf:type gst:Age ;
  rdf:type gsog:Generic_Geologic_Time_Unit ;
  gsoc:timeStarts gst:BaseMessinian ;
  rdfs:comment "Interval for grouping all specific instances of the Messinian Age"@en ;
  rdfs:label "Messinian Age"@en ;
.
gst:MiddleCambrianEpoch
  rdf:type gst:Epoch ;
  rdf:type gsog:Generic_Geologic_Time_Unit ;
  gsoc:timeStarts gst:BaseMiddleCambrianEpoch ;
  rdfs:comment "Interval for grouping all specific instances of the Middle Cambrian Epoch  "@en ;
  rdfs:label "Middle Cambrian Epoch  "@en ;
.
gst:MiddleDevonianEpoch
  rdf:type gst:Epoch ;
  rdf:type gsog:Generic_Geologic_Time_Unit ;
  gsoc:timeStarts gst:BaseMiddleDevonian ;
  rdfs:comment "Interval for grouping all specific instances of the Middle Devonian Epoch"@en ;
  rdfs:label "Middle Devonian Epoch"@en ;
.
gst:MiddleJurassicEpoch
  rdf:type gst:Epoch ;
  rdf:type gsog:Generic_Geologic_Time_Unit ;
  gsoc:timeStarts gst:BaseMiddleJurassic ;
  rdfs:comment "Interval for grouping all specific instances of the Middle Jurassic Epoch"@en ;
  rdfs:label "Middle Jurassic Epoch"@en ;
.
gst:MiddleMississippianEpoch
  rdf:type gst:Epoch ;
  rdf:type gsog:Generic_Geologic_Time_Unit ;
  gsoc:timeStarts gst:BaseMiddleMississippian ;
  rdfs:comment "Interval for grouping all specific instances of the Middle Mississippian Epoch"@en ;
  rdfs:label "Middle Mississippian Epoch"@en ;
.
gst:MiddleOrdovicianEpoch
  rdf:type gst:Epoch ;
  rdf:type gsog:Generic_Geologic_Time_Unit ;
  gsoc:timeStarts gst:BaseMiddleOrdovician ;
  rdfs:comment "Interval for grouping all specific instances of the Middle Ordovician Epoch"@en ;
  rdfs:label "Middle Ordovician Epoch"@en ;
.
gst:MiddlePennsylvanianEpoch
  rdf:type gst:Epoch ;
  rdf:type gsog:Generic_Geologic_Time_Unit ;
  gsoc:timeStarts gst:BaseMiddlePennsylvanian ;
  rdfs:comment "Interval for grouping all specific instances of the Middle Pennsylvanian Epoch"@en ;
  rdfs:label "Middle Pennsylvanian Epoch"@en ;
.
gst:MiddlePleistoceneAge
  rdf:type gst:Age ;
  rdf:type gsog:Generic_Geologic_Time_Unit ;
  gsoc:timeStarts gst:BaseMiddlePleistocene ;
  rdfs:comment "Interval for grouping all specific instances of the Middle Pleistocene Age"@en ;
  rdfs:label "Middle Pleistocene Age"@en ;
.
gst:MiddleTriassicEpoch
  rdf:type gst:Epoch ;
  rdf:type gsog:Generic_Geologic_Time_Unit ;
  gsoc:timeStarts gst:BaseMiddleTriassic ;
  rdfs:comment "Interval for grouping all specific instances of the Middle Triassic Epoch"@en ;
  rdfs:label "Middle Triassic Epoch"@en ;
.
gst:MioceneEpoch
  rdf:type gst:Epoch ;
  rdf:type gsog:Generic_Geologic_Time_Unit ;
  gsoc:timeStarts gst:BaseNeogene ;
  rdfs:comment "Interval for grouping all specific instances of the Miocene Epoch"@en ;
  rdfs:label "Miocene Epoch"@en ;
.
gst:MississippianSub-period
  rdf:type gst:Subperiod ;
  rdf:type gsog:Generic_Geologic_Time_Unit ;
  gsoc:timeStarts gst:BaseCarboniferous ;
  rdfs:comment "Interval for grouping all specific instances of the Mississippian Sub-period"@en ;
  rdfs:label "Mississippian Sub-period"@en ;
.
gst:MoscovianAge
  rdf:type gst:Age ;
  rdf:type gsog:Generic_Geologic_Time_Unit ;
  gsoc:timeStarts gst:BaseMiddlePennsylvanian ;
  rdfs:comment "Interval for grouping all specific instances of the Moscovian Age"@en ;
  rdfs:label "Moscovian Age"@en ;
.
gst:NeoarcheanEra
  rdf:type gst:Era ;
  rdf:type gsog:Generic_Geologic_Time_Unit ;
  gsoc:timeStarts gst:BaseNeoarchean ;
  rdfs:comment "Interval for grouping all specific instances of the Neoarchean Era"@en ;
  rdfs:label "Neoarchean Era"@en ;
.
gst:NeogenePeriod
  rdf:type gst:Period ;
  rdf:type gsog:Generic_Geologic_Time_Unit ;
  gsoc:timeStarts gst:BaseNeogene ;
  rdfs:comment "Interval for grouping all specific instances of the Neogene Period"@en ;
  rdfs:label "Neogene Period"@en ;
.
gst:NeoproterozoicEra
  rdf:type gst:Era ;
  rdf:type gsog:Generic_Geologic_Time_Unit ;
  gsoc:timeStarts gst:BaseNeoproterozoic ;
  rdfs:comment "Interval for grouping all specific instances of the Neoproterozoic Era"@en ;
  rdfs:label "Neoproterozoic Era"@en ;
.
gst:NorianAge
  rdf:type gst:Age ;
  rdf:type gsog:Generic_Geologic_Time_Unit ;
  gsoc:timeStarts gst:BaseNorian ;
  rdfs:comment "Interval for grouping all specific instances of the Norian Age"@en ;
  rdfs:label "Norian Age"@en ;
.
gst:NorthgrippianAge
  rdf:type gst:Age ;
  rdf:type gsog:Generic_Geologic_Time_Unit ;
  gsoc:timeStarts gst:BaseNorthgrippian ;
  rdfs:comment "Interval for grouping all specific instances of the Northgrippian Age"@en ;
  rdfs:label "Northgrippian Age"@en ;
.
gst:OlenekianAge
  rdf:type gst:Age ;
  rdf:type gsog:Generic_Geologic_Time_Unit ;
  gsoc:timeStarts gst:BaseOlenekian ;
  rdfs:comment "Interval for grouping all specific instances of the Olenekian Age"@en ;
  rdfs:label "Olenekian Age"@en ;
.
gst:OligoceneEpoch
  rdf:type gst:Epoch ;
  rdf:type gsog:Generic_Geologic_Time_Unit ;
  gsoc:timeStarts gst:BaseOligocene ;
  rdfs:comment "Interval for grouping all specific instances of the Oligocene Epoch"@en ;
  rdfs:label "Oligocene Epoch"@en ;
.
gst:OrdovicianPeriod
  rdf:type gst:Period ;
  rdf:type gsog:Generic_Geologic_Time_Unit ;
  gsoc:timeStarts gst:BaseOrdovician ;
  rdfs:comment "Interval for grouping all specific instances of the Ordovician Period"@en ;
  rdfs:label "Ordovician Period"@en ;
.
gst:OrosirianPeriod
  rdf:type gst:Period ;
  rdf:type gsog:Generic_Geologic_Time_Unit ;
  gsoc:timeStarts gst:BaseOrosirian ;
  rdfs:comment "Interval for grouping all specific instances of the Orosirian Period"@en ;
  rdfs:label "Orosirian Period"@en ;
.
gst:OxfordianAge
  rdf:type gst:Age ;
  rdf:type gsog:Generic_Geologic_Time_Unit ;
  gsoc:timeStarts gst:BaseUpperJurassic ;
  rdfs:comment "Interval for grouping all specific instances of the Oxfordian Age"@en ;
  rdfs:label "Oxfordian Age"@en ;
.
gst:PaibianAge
  rdf:type gst:Age ;
  rdf:type gsog:Generic_Geologic_Time_Unit ;
  gsoc:timeStarts gst:BaseFurongian ;
  rdfs:comment "Interval for grouping all specific instances of the Paibian Age"@en ;
  rdfs:label "Paibian Age"@en ;
.
gst:PaleoarcheanEra
  rdf:type gst:Era ;
  rdf:type gsog:Generic_Geologic_Time_Unit ;
  gsoc:timeStarts gst:BasePaleoarchean ;
  rdfs:comment "Interval for grouping all specific instances of the Paleoarchean Era"@en ;
  rdfs:label "Paleoarchean Era"@en ;
.
gst:PaleoceneEpoch
  rdf:type gst:Epoch ;
  rdf:type gsog:Generic_Geologic_Time_Unit ;
  gsoc:timeStarts gst:BaseCenozoic ;
  rdfs:comment "Interval for grouping all specific instances of the Paleocene Epoch"@en ;
  rdfs:label "Paleocene Epoch"@en ;
.
gst:PaleogenePeriod
  rdf:type gst:Period ;
  rdf:type gsog:Generic_Geologic_Time_Unit ;
  gsoc:timeStarts gst:BaseCenozoic ;
  rdfs:comment "Interval for grouping all specific instances of the Paleogene Period"@en ;
  rdfs:label "Paleogene Period"@en ;
.
gst:PaleoproterozoicEra
  rdf:type gst:Era ;
  rdf:type gsog:Generic_Geologic_Time_Unit ;
  gsoc:timeStarts gst:BaseProterozoic ;
  rdfs:comment "Interval for grouping all specific instances of the Paleoproterozoic Era"@en ;
  rdfs:label "Paleoproterozoic Era"@en ;
.
gst:PaleozoicEra
  rdf:type gst:Era ;
  rdf:type gsog:Generic_Geologic_Time_Unit ;
  gsoc:timeStarts gst:BasePhanerozoic ;
  rdfs:comment "Interval for grouping all specific instances of the Paleozoic Era"@en ;
  rdfs:label "Paleozoic Era"@en ;
.
gst:PennsylvanianSub-period
  rdf:type gst:Subperiod ;
  rdf:type gsog:Generic_Geologic_Time_Unit ;
  gsoc:timeStarts gst:BasePennsylvanian ;
  rdfs:comment "Interval for grouping all specific instances of the Pennsylvanian Sub-period"@en ;
  rdfs:label "Pennsylvanian Sub-period"@en ;
.
gst:Period
  rdf:type owl:Class ;
  rdfs:comment "Named rank for geochronologic time interval. Periods may be subdivided into Epochs. Periods are grouped into an Era."@en ;
  rdfs:subClassOf gsog:Geologic_Time_Interval ;
  rdfs:subClassOf [
      rdf:type owl:Restriction ;
      owl:allValuesFrom [
          rdf:type owl:Class ;
          owl:complementOf [
              rdf:type owl:Class ;
              owl:unionOf (
                  gst:Period
                  gst:Era
                  gst:Eon
                  gst:Supereon
                ) ;
            ] ;
        ] ;
      owl:onProperty gsoc:timeIncludes ;
    ] ;
  rdfs:subClassOf [
      rdf:type owl:Restriction ;
      owl:allValuesFrom [
          rdf:type owl:Class ;
          owl:complementOf [
              rdf:type owl:Class ;
              owl:unionOf (
                  gst:Period
                  gst:Subperiod
                  gst:Epoch
                  gst:Age
                ) ;
            ] ;
        ] ;
      owl:onProperty gsoc:timeIncludedBy ;
    ] ;
  rdfs:subClassOf [
      rdf:type owl:Restriction ;
      owl:onProperty gsoc:hostedBy ;
      owl:someValuesFrom gsgu:System ;
    ] ;
.
gst:PermianPeriod
  rdf:type gst:Period ;
  rdf:type gsog:Generic_Geologic_Time_Unit ;
  gsoc:timeStarts gst:BasePermian ;
  rdfs:comment "Interval for grouping all specific instances of the Permian Period"@en ;
  rdfs:label "Permian Period"@en ;
.
gst:PhanerozoicEon
  rdf:type gst:Eon ;
  rdf:type gsog:Generic_Geologic_Time_Unit ;
  gsoc:timeStarts gst:BasePhanerozoic ;
  rdfs:comment "Interval for grouping all specific instances of the Phanerozoic Eon"@en ;
  rdfs:label "Phanerozoic Eon"@en ;
.
gst:PiacenzianAge
  rdf:type gst:Age ;
  rdf:type gsog:Generic_Geologic_Time_Unit ;
  gsoc:timeStarts gst:BasePiacenzian ;
  rdfs:comment "Interval for grouping all specific instances of the Piacenzian Age"@en ;
  rdfs:label "Piacenzian Age"@en ;
.
gst:Pleistocene
  rdf:type gst:Epoch ;
  rdf:type gsog:Generic_Geologic_Time_Unit ;
  gsoc:timeStarts gst:BaseCalabrian ;
  rdfs:comment "Interval for grouping all specific instances of the Pleistocene  "@en ;
  rdfs:label "Pleistocene  "@en ;
.
gst:PleistoceneEpoch
  rdf:type gst:Epoch ;
  rdf:type gsog:Generic_Geologic_Time_Unit ;
  gsoc:timeStarts gst:BaseGelasian ;
  rdfs:comment "Interval for grouping all specific instances of the Pleistocene Epoch"@en ;
  rdfs:label "Pleistocene Epoch"@en ;
.
gst:PliensbachianAge
  rdf:type gst:Age ;
  rdf:type gsog:Generic_Geologic_Time_Unit ;
  gsoc:timeStarts gst:BasePliensbachian ;
  rdfs:comment "Interval for grouping all specific instances of the Pliensbachian Age"@en ;
  rdfs:label "Pliensbachian Age"@en ;
.
gst:PlioceneEpoch
  rdf:type gst:Epoch ;
  rdf:type gsog:Generic_Geologic_Time_Unit ;
  gsoc:timeStarts gst:BasePliocene ;
  rdfs:comment "Interval for grouping all specific instances of the Pliocene Epoch"@en ;
  rdfs:label "Pliocene Epoch"@en ;
.
gst:PragianAge
  rdf:type gst:Age ;
  rdf:type gsog:Generic_Geologic_Time_Unit ;
  gsoc:timeStarts gst:BasePragian ;
  rdfs:comment "Interval for grouping all specific instances of the Pragian Age"@en ;
  rdfs:label "Pragian Age"@en ;
.
gst:PrecambrianSupereon
  rdf:type gst:Supereon ;
  rdf:type gsog:Generic_Geologic_Time_Unit ;
  gsoc:timeStarts gst:FormationoftheEarth ;
  rdfs:comment "Interval for grouping all specific instances of the Precambrian Supereon"@en ;
  rdfs:label "Precambrian Supereon"@en ;
.
gst:PriabonianAge
  rdf:type gst:Age ;
  rdf:type gsog:Generic_Geologic_Time_Unit ;
  gsoc:timeStarts gst:BasePriabonian ;
  rdfs:comment "Interval for grouping all specific instances of the Priabonian Age"@en ;
  rdfs:label "Priabonian Age"@en ;
.
gst:PridoliEpoch
  rdf:type gst:Epoch ;
  rdf:type gsog:Generic_Geologic_Time_Unit ;
  gsoc:timeStarts gst:BasePridoli ;
  rdfs:comment "Interval for grouping all specific instances of the Pridoli Epoch"@en ;
  rdfs:label "Pridoli Epoch"@en ;
.
gst:ProterozoicEon
  rdf:type gst:Eon ;
  rdf:type gsog:Generic_Geologic_Time_Unit ;
  gsoc:timeStarts gst:BaseProterozoic ;
  rdfs:comment "Interval for grouping all specific instances of the Proterozoic Eon"@en ;
  rdfs:label "Proterozoic Eon"@en ;
.
gst:QuaternaryPeriod
  rdf:type gst:Period ;
  rdf:type gsog:Generic_Geologic_Time_Unit ;
  gsoc:timeStarts gst:BaseGelasian ;
  rdfs:comment "Interval for grouping all specific instances of the Quaternary Period"@en ;
  rdfs:label "Quaternary Period"@en ;
.
gst:RhaetianAge
  rdf:type gst:Age ;
  rdf:type gsog:Generic_Geologic_Time_Unit ;
  gsoc:timeStarts gst:BaseRhaetian ;
  rdfs:comment "Interval for grouping all specific instances of the Rhaetian Age"@en ;
  rdfs:label "Rhaetian Age"@en ;
.
gst:RhuddanianAge
  rdf:type gst:Age ;
  rdf:type gsog:Generic_Geologic_Time_Unit ;
  gsoc:timeStarts gst:BaseSilurian ;
  rdfs:comment "Interval for grouping all specific instances of the Rhuddanian Age"@en ;
  rdfs:label "Rhuddanian Age"@en ;
.
gst:RhyacianPeriod
  rdf:type gst:Period ;
  rdf:type gsog:Generic_Geologic_Time_Unit ;
  gsoc:timeStarts gst:BaseRhyacian ;
  rdfs:comment "Interval for grouping all specific instances of the Rhyacian Period"@en ;
  rdfs:label "Rhyacian Period"@en ;
.
gst:RoadianAge
  rdf:type gst:Age ;
  rdf:type gsog:Generic_Geologic_Time_Unit ;
  gsoc:timeStarts gst:BaseGuadalupian ;
  rdfs:comment "Interval for grouping all specific instances of the Roadian Age"@en ;
  rdfs:label "Roadian Age"@en ;
.
gst:RupelianAge
  rdf:type gst:Age ;
  rdf:type gsog:Generic_Geologic_Time_Unit ;
  gsoc:timeStarts gst:BaseOligocene ;
  rdfs:comment "Interval for grouping all specific instances of the Rupelian Age"@en ;
  rdfs:label "Rupelian Age"@en ;
.
gst:SakmarianAge
  rdf:type gst:Age ;
  rdf:type gsog:Generic_Geologic_Time_Unit ;
  gsoc:timeStarts gst:BaseSakmarian ;
  rdfs:comment "Interval for grouping all specific instances of the Sakmarian Age"@en ;
  rdfs:label "Sakmarian Age"@en ;
.
gst:SandbianAge
  rdf:type gst:Age ;
  rdf:type gsog:Generic_Geologic_Time_Unit ;
  gsoc:timeStarts gst:BaseUpperOrdovician ;
  rdfs:comment "Interval for grouping all specific instances of the Sandbian Age"@en ;
  rdfs:label "Sandbian Age"@en ;
.
gst:SantonianAge
  rdf:type gst:Age ;
  rdf:type gsog:Generic_Geologic_Time_Unit ;
  gsoc:timeStarts gst:BaseSantonian ;
  rdfs:comment "Interval for grouping all specific instances of the Santonian Age"@en ;
  rdfs:label "Santonian Age"@en ;
.
gst:SelandianAge
  rdf:type gst:Age ;
  rdf:type gsog:Generic_Geologic_Time_Unit ;
  gsoc:timeStarts gst:BaseSelandian ;
  rdfs:comment "Interval for grouping all specific instances of the Selandian Age"@en ;
  rdfs:label "Selandian Age"@en ;
.
gst:SerpukhovianAge
  rdf:type gst:Age ;
  rdf:type gsog:Generic_Geologic_Time_Unit ;
  gsoc:timeStarts gst:BaseUpperMississippian ;
  rdfs:comment "Interval for grouping all specific instances of the Serpukhovian Age"@en ;
  rdfs:label "Serpukhovian Age"@en ;
.
gst:SerravallianAge
  rdf:type gst:Age ;
  rdf:type gsog:Generic_Geologic_Time_Unit ;
  gsoc:timeStarts gst:BaseSerravallian ;
  rdfs:comment "Interval for grouping all specific instances of the Serravallian Age"@en ;
  rdfs:label "Serravallian Age"@en ;
.
gst:SheinwoodianAge
  rdf:type gst:Age ;
  rdf:type gsog:Generic_Geologic_Time_Unit ;
  gsoc:timeStarts gst:BaseWenlock ;
  rdfs:comment "Interval for grouping all specific instances of the Sheinwoodian Age"@en ;
  rdfs:label "Sheinwoodian Age"@en ;
.
gst:SiderianPeriod
  rdf:type gst:Period ;
  rdf:type gsog:Generic_Geologic_Time_Unit ;
  gsoc:timeStarts gst:BaseProterozoic ;
  rdfs:comment "Interval for grouping all specific instances of the Siderian Period"@en ;
  rdfs:label "Siderian Period"@en ;
.
gst:SilurianPeriod
  rdf:type gst:Period ;
  rdf:type gsog:Generic_Geologic_Time_Unit ;
  gsoc:timeStarts gst:BaseSilurian ;
  rdfs:comment "Interval for grouping all specific instances of the Silurian Period"@en ;
  rdfs:label "Silurian Period"@en ;
.
gst:SinemurianAge
  rdf:type gst:Age ;
  rdf:type gsog:Generic_Geologic_Time_Unit ;
  gsoc:timeStarts gst:BaseSinemurian ;
  rdfs:comment "Interval for grouping all specific instances of the Sinemurian Age"@en ;
  rdfs:label "Sinemurian Age"@en ;
.
gst:StatherianPeriod
  rdf:type gst:Period ;
  rdf:type gsog:Generic_Geologic_Time_Unit ;
  gsoc:timeStarts gst:BaseStatherian ;
  rdfs:comment "Interval for grouping all specific instances of the Statherian Period"@en ;
  rdfs:label "Statherian Period"@en ;
.
gst:StenianPeriod
  rdf:type gst:Period ;
  rdf:type gsog:Generic_Geologic_Time_Unit ;
  gsoc:timeStarts gst:BaseStenian ;
  rdfs:comment "Interval for grouping all specific instances of the Stenian Period"@en ;
  rdfs:label "Stenian Period"@en ;
.
gst:Subperiod
  rdf:type owl:Class ;
  rdfs:comment "Named rank for geochronologic time interval. Sub-Periods may be subdivided into Epochs. Sub-Periods are grouped into a period."@en ;
  rdfs:subClassOf gsog:Geologic_Time_Interval ;
  rdfs:subClassOf [
      rdf:type owl:Restriction ;
      owl:allValuesFrom [
          rdf:type owl:Class ;
          owl:complementOf [
              rdf:type owl:Class ;
              owl:unionOf (
                  gst:Subperiod
                  gst:Epoch
                  gst:Age
                ) ;
            ] ;
        ] ;
      owl:onProperty gsoc:timeDuring ;
    ] ;
  rdfs:subClassOf [
      rdf:type owl:Restriction ;
      owl:allValuesFrom [
          rdf:type owl:Class ;
          owl:complementOf [
              rdf:type owl:Class ;
              owl:unionOf (
                  gst:Subperiod
                  gst:Period
                  gst:Era
                  gst:Eon
                  gst:Supereon
                ) ;
            ] ;
        ] ;
      owl:onProperty gsoc:timeContains ;
    ] ;
  rdfs:subClassOf [
      rdf:type owl:Restriction ;
      owl:onProperty gsoc:hostedBy ;
      owl:someValuesFrom gsgu:System ;
    ] ;
.
gst:Supereon
  rdf:type owl:Class ;
  rdfs:comment "hight ranking geochronlogic time interval, parts are eons"@en ;
  rdfs:label "Supereon"@en ;
  rdfs:subClassOf gsog:Geologic_Time_Interval ;
  rdfs:subClassOf [
      rdf:type owl:Restriction ;
      owl:allValuesFrom [
          rdf:type owl:Class ;
          owl:complementOf gst:Supereon ;
        ] ;
      owl:onProperty gsoc:timeContains ;
    ] ;
  rdfs:subClassOf [
      rdf:type owl:Restriction ;
      owl:onProperty gsoc:hostedBy ;
      owl:someValuesFrom gsgu:Chronostratigraphic_Unit ;
    ] ;
.
gst:TelychianAge
  rdf:type gst:Age ;
  rdf:type gsog:Generic_Geologic_Time_Unit ;
  gsoc:timeStarts gst:BaseTelychian ;
  rdfs:comment "Interval for grouping all specific instances of the Telychian Age"@en ;
  rdfs:label "Telychian Age"@en ;
.
gst:TerreneuvianEpoch
  rdf:type gst:Epoch ;
  rdf:type gsog:Generic_Geologic_Time_Unit ;
  gsoc:timeStarts gst:BasePhanerozoic ;
  rdfs:comment "Interval for grouping all specific instances of the Terreneuvian Epoch"@en ;
  rdfs:label "Terreneuvian Epoch"@en ;
.
gst:ThanetianAge
  rdf:type gst:Age ;
  rdf:type gsog:Generic_Geologic_Time_Unit ;
  gsoc:timeStarts gst:BaseThanetian ;
  rdfs:comment "Interval for grouping all specific instances of the Thanetian Age"@en ;
  rdfs:comment "The Thanetian Stage concept was first used by Renevier (1873) who included the Thanet Sands with Cyprina morris and the Woolwich and Reading Beds with Cyrena cuneiformis. Its meaning was subsequently narrowed by Dollfus (1880), who included only the Thanet Sands, the original type-strata on the Isle of Thanet in southeast England. Since 1880 the term Thanetian has consistently been used with the restricted meaning of Dollfus (Bignot et al. 1997). https://doi.org/10.18814/epiiugs/2011/v34i4/002"@en ;
  rdfs:label "Thanetian Age"@en ;
.
gst:TithonianAge
  rdf:type gst:Age ;
  rdf:type gsog:Generic_Geologic_Time_Unit ;
  gsoc:timeStarts gst:BaseTithonian ;
  rdfs:comment "Interval for grouping all specific instances of the Tithonian Age"@en ;
  rdfs:label "Tithonian Age"@en ;
.
gst:ToarcianAge
  rdf:type gst:Age ;
  rdf:type gsog:Generic_Geologic_Time_Unit ;
  gsoc:timeStarts gst:BaseToarcian ;
  rdfs:comment "Interval for grouping all specific instances of the Toarcian Age"@en ;
  rdfs:label "Toarcian Age"@en ;
.
gst:TonianPeriod
  rdf:type gst:Period ;
  rdf:type gsog:Generic_Geologic_Time_Unit ;
  gsoc:timeStarts gst:BaseNeoproterozoic ;
  rdfs:comment "Interval for grouping all specific instances of the Tonian Period"@en ;
  rdfs:label "Tonian Period"@en ;
.
gst:TortonianAge
  rdf:type gst:Age ;
  rdf:type gsog:Generic_Geologic_Time_Unit ;
  gsoc:timeStarts gst:BaseTortonian ;
  rdfs:comment "Interval for grouping all specific instances of the Tortonian Age"@en ;
  rdfs:label "Tortonian Age"@en ;
.
gst:TournaisianAge
  rdf:type gst:Age ;
  rdf:type gsog:Generic_Geologic_Time_Unit ;
  gsoc:timeStarts gst:BaseCarboniferous ;
  rdfs:comment "Interval for grouping all specific instances of the Tournaisian Age"@en ;
  rdfs:label "Tournaisian Age"@en ;
.
gst:TremadocianAge
  rdf:type gst:Age ;
  rdf:type gsog:Generic_Geologic_Time_Unit ;
  gsoc:timeStarts gst:BaseOrdovician ;
  rdfs:comment "Interval for grouping all specific instances of the Tremadocian Age"@en ;
  rdfs:label "Tremadocian Age"@en ;
.
gst:TriassicPeriod
  rdf:type gst:Period ;
  rdf:type gsog:Generic_Geologic_Time_Unit ;
  gsoc:timeStarts gst:BaseMesozoic ;
  rdfs:comment "Interval for grouping all specific instances of the Triassic Period"@en ;
  rdfs:label "Triassic Period"@en ;
.
gst:TuronianAge
  rdf:type gst:Age ;
  rdf:type gsog:Generic_Geologic_Time_Unit ;
  gsoc:timeStarts gst:BaseTuronian ;
  rdfs:comment "Interval for grouping all specific instances of the Turonian Age"@en ;
  rdfs:label "Turonian Age"@en ;
.
gst:UpperCretaceousEpoch
  rdf:type gst:Epoch ;
  rdf:type gsog:Generic_Geologic_Time_Unit ;
  gsoc:timeStarts gst:BaseUpperCretaceous ;
  rdfs:comment "Interval for grouping all specific instances of the Upper Cretaceous Epoch"@en ;
  rdfs:label "Upper Cretaceous Epoch"@en ;
.
gst:UpperDevonianEpoch
  rdf:type gst:Epoch ;
  rdf:type gsog:Generic_Geologic_Time_Unit ;
  gsoc:timeStarts gst:BaseUpperDevonian ;
  rdfs:comment "Interval for grouping all specific instances of the Upper Devonian Epoch"@en ;
  rdfs:label "Upper Devonian Epoch"@en ;
.
gst:UpperJurassicEpoch
  rdf:type gst:Epoch ;
  rdf:type gsog:Generic_Geologic_Time_Unit ;
  gsoc:timeStarts gst:BaseUpperJurassic ;
  rdfs:comment "Interval for grouping all specific instances of the Upper Jurassic Epoch"@en ;
  rdfs:label "Upper Jurassic Epoch"@en ;
.
gst:UpperMississippianEpoch
  rdf:type gst:Epoch ;
  rdf:type gsog:Generic_Geologic_Time_Unit ;
  gsoc:timeStarts gst:BaseUpperMississippian ;
  rdfs:comment "Interval for grouping all specific instances of the Upper Mississippian Epoch"@en ;
  rdfs:label "Upper Mississippian Epoch"@en ;
.
gst:UpperOrdovicianEpoch
  rdf:type gst:Epoch ;
  rdf:type gsog:Generic_Geologic_Time_Unit ;
  gsoc:timeStarts gst:BaseUpperOrdovician ;
  rdfs:comment "Interval for grouping all specific instances of the Upper Ordovician Epoch"@en ;
  rdfs:label "Upper Ordovician Epoch"@en ;
.
gst:UpperPennsylvanianEpoch
  rdf:type gst:Epoch ;
  rdf:type gsog:Generic_Geologic_Time_Unit ;
  gsoc:timeStarts gst:BaseUpperPennsylvanian ;
  rdfs:comment "Interval for grouping all specific instances of the Upper Pennsylvanian Epoch"@en ;
  rdfs:label "Upper Pennsylvanian Epoch"@en ;
.
gst:UpperPleistoceneAge
  rdf:type gst:Age ;
  rdf:type gsog:Generic_Geologic_Time_Unit ;
  gsoc:timeStarts gst:BaseUpperPleistocene ;
  rdfs:comment "Interval for grouping all specific instances of the Upper Pleistocene Age"@en ;
  rdfs:label "Upper Pleistocene Age"@en ;
.
gst:UpperTriassicEpoch
  rdf:type gst:Epoch ;
  rdf:type gsog:Generic_Geologic_Time_Unit ;
  gsoc:timeStarts gst:BaseUpperTriassic ;
  rdfs:comment "Interval for grouping all specific instances of the Upper Triassic Epoch"@en ;
  rdfs:label "Upper Triassic Epoch"@en ;
.
gst:ValanginianAge
  rdf:type gst:Age ;
  rdf:type gsog:Generic_Geologic_Time_Unit ;
  gsoc:timeStarts gst:BaseValanginian ;
  rdfs:comment "Interval for grouping all specific instances of the Valanginian Age"@en ;
  rdfs:label "Valanginian Age"@en ;
.
gst:ViseanAge
  rdf:type gst:Age ;
  rdf:type gsog:Generic_Geologic_Time_Unit ;
  gsoc:timeStarts gst:BaseMiddleMississippian ;
  rdfs:comment "Interval for grouping all specific instances of the Visean Age"@en ;
  rdfs:label "Visean Age"@en ;
.
gst:WenlockEpoch
  rdf:type gst:Epoch ;
  rdf:type gsog:Generic_Geologic_Time_Unit ;
  gsoc:timeStarts gst:BaseWenlock ;
  rdfs:comment "Interval for grouping all specific instances of the Wenlock Epoch"@en ;
  rdfs:label "Wenlock Epoch"@en ;
.
gst:WordianAge
  rdf:type gst:Age ;
  rdf:type gsog:Generic_Geologic_Time_Unit ;
  gsoc:timeStarts gst:BaseWordian ;
  rdfs:comment "Interval for grouping all specific instances of the Wordian Age"@en ;
  rdfs:label "Wordian Age"@en ;
.
gst:WuchiapingianAge
  rdf:type gst:Age ;
  rdf:type gsog:Generic_Geologic_Time_Unit ;
  gsoc:timeStarts gst:BaseLopingian ;
  rdfs:comment "Interval for grouping all specific instances of the Wuchiapingian Age"@en ;
  rdfs:label "Wuchiapingian Age"@en ;
.
gst:YpresianAge
  rdf:type gst:Age ;
  rdf:type gsog:Generic_Geologic_Time_Unit ;
  gsoc:timeStarts gst:BaseEocene ;
  rdfs:comment "Interval for grouping all specific instances of the Ypresian Age"@en ;
  rdfs:label "Ypresian Age"@en ;
.
gst:ZancleanAge
  rdf:type gst:Age ;
  rdf:type gsog:Generic_Geologic_Time_Unit ;
  gsoc:timeStarts gst:BasePliocene ;
  rdfs:comment "Interval for grouping all specific instances of the Zanclean Age"@en ;
  rdfs:label "Zanclean Age"@en ;
.

