# baseURI: https://w3id.org/gso/1.0/geologicquality/ontology
# imports: https://w3id.org/gso/1.0/common/ontology
# imports: https://w3id.org/gso/1.0/geology/ontology
# imports: https://w3id.org/gso/1.0/quality/ontology

@prefix : <https://w3id.org/gso/1.0/geologicquality/> .
@prefix dct: <http://purl.org/dc/terms/> .
@prefix gsgq: <https://w3id.org/gso/1.0/geologicquality/> .
@prefix gsoc: <https://w3id.org/gso/1.0/common/> .
@prefix gsog: <https://w3id.org/gso/1.0/geology/> .
@prefix gsoq: <https://w3id.org/gso/1.0/quality/> .
@prefix owl: <http://www.w3.org/2002/07/owl#> .
@prefix rdf: <http://www.w3.org/1999/02/22-rdf-syntax-ns#> .
@prefix rdfs: <http://www.w3.org/2000/01/rdf-schema#> .
@prefix skos: <http://www.w3.org/2004/02/skos/core#> .   @prefix schema: <https://schema.org/> .
@prefix xsd: <http://www.w3.org/2001/XMLSchema#> .

gsoc:boyan_brodaric rdf:type schema:Person ; rdf:type owl:NamedIndividual ;
  schema:identifier <https://orcid.org/0000-0002-7987-3810> ;
  schema:affiliation "Natural Resources Canada, Geological Survey of Canada"  ;
  rdfs:comment "e-mail: mailto:boyan.brodaric@canada.ca " ;
  schema:name "Dr. Boyan Brodaric" ; rdfs:label "Dr. Boyan Brodaric" ;
.
gsoc:stephen_richard    rdf:type schema:Person ;     rdf:type owl:NamedIndividual ;
  schema:identifier <https://orcid.org/0000-0001-6041-5302> ;
  rdfs:comment "e-mail: mailto:smrTucson@gmail.com " ;
  schema:name "Dr. Stephen M. Richard" ; rdfs:label "Dr. Stephen M. Richard" ;
.
gsgq:Alteration_Degree
  rdf:type owl:Class ;
  rdfs:comment "Specification of the strength of observed alteration. Can be used on Geologic_Unit or Rock_Material"@en ;
  rdfs:isDefinedBy "GeoSciML v4"@en ;
  rdfs:label "Alteration degree"@en ;
  rdfs:subClassOf gsoc:Physical_Quality ;
  rdfs:subClassOf [
      rdf:type owl:Restriction ;
      owl:allValuesFrom gsog:Rock_Body ;
      owl:onProperty gsoc:isQualityOf ;
    ] ;
.
gsgq:Azimuth
  rdf:type owl:Class ;
  rdfs:comment "Bearing of a horizontal line relative to north. Use for specifying the orientation of planar or linear features."@en ;
  rdfs:label "Azimuth"@en ;
  rdfs:subClassOf gsoq:Orientation ;
  rdfs:subClassOf [
      rdf:type owl:Restriction ;
      owl:onProperty gsoc:hasValue ;
      owl:someValuesFrom [
          rdf:type owl:Class ;
          owl:unionOf (
              gsoc:Numeric_Value
              gsoc:Named_Value
              gsoc:Range_Value
            ) ;
        ] ;
    ] ;
.
gsgq:Bedding_Pattern
  rdf:type owl:Class ;
  rdfs:subClassOf gsoc:Physical_Quality ;
  rdfs:subClassOf [
      rdf:type owl:Restriction ;
      owl:allValuesFrom gsog:Rock_Body ;
      owl:onProperty gsoc:isQualityOf ;
    ] ;
.
gsgq:Bedding_Style
  rdf:type owl:Class ;
  rdfs:subClassOf gsoc:Physical_Quality ;
  rdfs:subClassOf [
      rdf:type owl:Restriction ;
      owl:allValuesFrom gsog:Rock_Body ;
      owl:onProperty gsoc:isQualityOf ;
    ] ;
.
gsgq:Bedding_Thickness
  rdf:type owl:Class ;
  rdfs:subClassOf gsoq:Thickness ;
  rdfs:subClassOf [
      rdf:type owl:Restriction ;
      owl:allValuesFrom gsog:Rock_Body ;
      owl:onProperty gsoc:isQualityOf ;
    ] ;
.
gsgq:Consolidation_Degree
  rdf:type owl:Class ;
  rdfs:comment "A property that specifies the degree to which an aggregation of EarthMaterial particles is a distinct solid material. Consolidation and induration are related concepts specified by this property. They define a continuum from unconsolidated material to very hard rock. Induration is the degree to which a consolidated material is made hard, operationally determined by how difficult it is to break a piece of the material. Consolidated materials may have varying degrees of induration (NADMSC, 2004)"@en ;
  rdfs:isDefinedBy "GeoSciML v4"@en ;
  rdfs:label "Consolidation degree"@en ;
  rdfs:subClassOf gsoc:Physical_Quality ;
  rdfs:subClassOf [
      rdf:type owl:Restriction ;
      owl:allValuesFrom gsog:Rock_Material ;
      owl:onProperty gsoc:isQualityOf ;
    ] ;
.
gsgq:Dip
  rdf:type owl:Class ;
  rdfs:comment "the maximum angle between a horizontal surface and a planar feature"@en ;
  rdfs:label "Dip"@en ;
  rdfs:subClassOf gsoq:Orientation ;
  rdfs:subClassOf [
      rdf:type owl:Restriction ;
      owl:onProperty gsoc:hasQuality ;
      owl:someValuesFrom [
          rdf:type owl:Class ;
          owl:unionOf (
              gsoc:Numeric_Value
              gsoc:Named_Value
              gsoc:Range_Value
            ) ;
        ] ;
    ] ;
.
gsgq:Dip_Value
  rdf:type owl:Class ;
  rdfs:subClassOf gsoq:Orientation_Value ;
  rdfs:subClassOf [
      rdf:type owl:Restriction ;
      owl:allValuesFrom gsgq:Dip ;
      owl:onProperty gsoc:isValueOf ;
    ] ;
.
gsgq:Facing
  rdf:type owl:Class ;
  rdfs:comment "property to specify if a surface is directed, i.e. has a top and bottom. Values: {upright, overturned, unknown}"@en ;
  rdfs:label "Facing direction"@en ;
  rdfs:subClassOf gsoq:Orientation ;
.
gsgq:Facing_Value
  rdf:type owl:Class ;
  rdfs:subClassOf gsoq:Orientation_Value ;
  rdfs:subClassOf [
      rdf:type owl:Restriction ;
      owl:allValuesFrom gsgq:Facing ;
      owl:onProperty gsoc:isValueOf ;
    ] ;
.
gsgq:Gently_Inclined
  rdf:type owl:Class ;
  dct:source "Fleuty (1964) Folds classification." ;
  rdfs:comment "Surface dips between 10 and 30 degrees; typically used to describe orientation of fold hinge surface or axial surface, but could be applied to any geologic surface."@en ;
  rdfs:label "Gently Inclinded "@en ;
  rdfs:subClassOf gsgq:Inclined ;
.
gsgq:Gently_Plunging_Line
  rdf:type owl:Class ;
  dct:source "Fleuty (1964) Folds classification." ;
  rdfs:comment "line plunges between 10 and 30 degrees."@en ;
  rdfs:label "Gently plunging line"@en ;
  rdfs:subClassOf gsgq:Plunging_Line ;
.
gsgq:High_Metamorphic_Grade
  rdf:type owl:Class ;
  dct:source "Smulikowski et al, 2003; Fry, 1984"@en ;
  rdfs:comment "Protolith structures almost always obliterated, evidence of partial melting common. Includes rocks metamorphosed in high-temperature amphibolite, pyroxene hornfels, and medium to high-temperature eclogite facies. Mineral assemblages according to Fry (1984) Table 10-1: ultramafic-olivine, anthophyllite, cummingtonite, enstatite, mafic-hornblende, (diopside, garnet), calc-aluminous basic-plagioclase, pelite, semi-pelite -- K-feldspar, biotite, quartz, Al-minerals (garnet), migmatite."@en ;
  rdfs:label "high metamorphic grade"@en ;
  rdfs:subClassOf gsgq:Metamorphosed ;
.
gsgq:Horizonatal_Inclination
  rdf:type owl:Class ;
  rdfs:comment "Surface dips between 0 and 10 degrees. Equivalent term 'recumbent' used to describe orientation of fold hing surface or axial surface"@en ;
  rdfs:label "Horizontal inclination "@en ;
  rdfs:subClassOf gsgq:Dip_Value ;
.
gsgq:Horizontal_Line
  rdf:type owl:Class ;
  dct:source "Fleuty (1964) Folds classification." ;
  rdfs:comment "line plunges between 0 and 10 degrees."@en ;
  rdfs:label "Horizontal line "@en ;
  rdfs:subClassOf gsgq:Plunge_Value ;
.
gsgq:Inclined
  rdf:type owl:Class ;
  dct:source "Fleuty (1964) Folds classification." ;
  rdfs:comment "Surface dips between 10 and 80 degrees; typically used to describe orientation of fold hinge surface or axial surface, but could be applied to any geologic surface."@en ;
  rdfs:label "Inclined"@en ;
  rdfs:subClassOf gsgq:Dip_Value ;
.
gsgq:Line_Orientation
  rdf:type owl:Class ;
  rdfs:comment "specification of the orientation of a line in space, using a trend (bearing of horizontal projection of line relative to geographic north) and plunge (inclination of line measured positive downward in degrees from local horizontal).  TBD:  add 'isdirected property to indicate if the line is directed (e.g. sense of shear), values should be Boolean,"@en ;
  rdfs:label "Line orientation"@en ;
  rdfs:subClassOf gsoq:Orientation ;
  rdfs:subClassOf [
      rdf:type owl:Restriction ;
      owl:allValuesFrom [
          rdf:type owl:Class ;
          owl:unionOf [
              rdf:type rdf:List ;
              rdf:first gsgq:Azimuth ;
              rdf:rest [
                  rdf:type rdf:List ;
                  rdf:first gsgq:Plunge ;
                  rdf:rest () ;
                ] ;
            ] ;
        ] ;
      owl:onProperty gsoc:hasQuality ;
    ] ;
.
gsgq:Low_Metamorphic_Grade
  rdf:type owl:Class ;
  dct:source "Smulikowski et al, 2003; Fry, 1984"@en ;
  rdfs:comment "Metamorphic effects clearly visible, protolith structures typically still observable, includes rocks metamorphosed in greenschisthigh-temperature blueschist, very low temperature eclogite facies. Mineral assemblages according to Fry (1984) Table 10-1: ultramafic-serpentine (talc, magnesite),  mafic-chlorite, actinolite (garnet), calc-aluminous basic-albite, epidote, pelite, semi-pelite -- white mica, chlorite, quartz, biotite (garnet, Al-minerals)."@en ;
  rdfs:label "low metamorphic grade"@en ;
  rdfs:subClassOf gsgq:Metamorphosed ;
.
gsgq:Magnetic_Susceptibility
  rdf:type owl:Class ;
  dct:source "https://en.wikipedia.org/wiki/Magnetic_susceptibility" ;
  rdfs:comment "a measure of how much a material will become magnetized in an applied magnetic field. It is the ratio of magnetization M (magnetic moment per unit volume) to the applied magnetizing field intensity H. This allows a simple classification, into two categories, of most materials' responses to an applied magnetic field: an alignment with the magnetic field, χ > 0, called paramagnetism, or an alignment against the field, χ < 0, called diamagnetism."@en ;
  rdfs:label "Magnetic susceptibility "@en ;
  rdfs:subClassOf gsoc:Physical_Quality ;
  rdfs:subClassOf [
      rdf:type owl:Restriction ;
      owl:allValuesFrom gsoc:Amount_Of_Matter ;
      owl:onProperty gsoc:isQualityOf ;
    ] ;
.
gsgq:Medium_Metamorphic_Grade
  rdf:type owl:Class ;
  dct:source "Smulikowski et al, 2003; Fry, 1984"@en ;
  rdfs:comment "Protolith structure typically obliterated. Includes rocks metamorphosed in high-temperature epidote-amphibolite, low-temperature amphibolite, and low temperature eclogite facies. Mineral assemblages according to Fry (1984) Table 10-1: ultramafic-olivine, talc (magnesite, anthophyllite), mafic-hornblende, (diopside, garnet), calc-aluminous basic-plagioclase, pelite, semi-pelite -- white mica, biotite, quartz (garnet, Al-minerals)."@en ;
  rdfs:label "medium metamorphic grade"@en ;
  rdfs:subClassOf gsgq:Metamorphosed ;
.
gsgq:Metamorphic_Grade
  rdf:type owl:Class ;
  rdfs:comment "A term to indicate the intensity or rank of metamorphism applied to an EarthMaterial (eg: high metamorphic grade, low metamorphic grade). Indicates in a general way the P-T environment in which the metamorphism took place. Determination of metamorphic grade is based on mineral assemblages (ie, facies) present in a rock that are interpreted to have crystallized in equilibrium during a particular metamorphic event."@en ;
  rdfs:comment "applies to Earth_Material or Geologic_Unit"@en ;
  rdfs:isDefinedBy "GeoSciML v4"@en ;
  rdfs:label "Metamorphic grade"@en ;
  rdfs:subClassOf gsoc:Physical_Quality ;
.
gsgq:Metamorphosed
  rdf:type owl:Class ;
  dct:source "CGI metamorphicgrade SKOS vocabulary 2016-11-22"@en ;
  rdfs:comment "Rock is metamorphosed, may have any value for metamorphic grade except 'not metamorphosed'."@en ;
  rdfs:label "Metamorphosed, grade not specified"@en ;
  rdfs:subClassOf gsoc:Named_Value ;
  rdfs:subClassOf [
      rdf:type owl:Restriction ;
      owl:allValuesFrom gsgq:Metamorphic_Grade ;
      owl:onProperty gsoc:isValueOf ;
    ] ;
  rdfs:subClassOf [
      rdf:type owl:Restriction ;
      owl:onClass gsgq:Metamorphic_Grade ;
      owl:onProperty gsoc:isValueOf ;
      owl:qualifiedCardinality "1"^^xsd:nonNegativeInteger ;
    ] ;
.
gsgq:Moderately_Inclined
  rdf:type owl:Class ;
  dct:source "Fleuty (1964) Folds classification." ;
  rdfs:comment "Surface dips between 30 and 60 degrees; typically used to describe orientation of fold hing surface or axial surface, but could be applied to any geologic surface."@en ;
  rdfs:label "Moderately Inclinded "@en ;
  rdfs:subClassOf gsgq:Inclined ;
.
gsgq:Moderately_Plunging_Line
  rdf:type owl:Class ;
  dct:source "Fleuty (1964) Folds classification." ;
  rdfs:comment "line plunges between 30 and 60 degrees."@en ;
  rdfs:label "Moderately plunging line"@en ;
  rdfs:subClassOf gsgq:Plunging_Line ;
.
gsgq:Not_Metamorphosed
  rdf:type owl:Class ;
  dct:source "CGI metamorphicgrade SKOS vocabulary 2016-11-22"@en ;
  rdfs:comment "Rock is not metamorphose'."@en ;
  rdfs:label "Not metamorphosed"@en ;
  rdfs:subClassOf gsoc:Named_Value ;
  rdfs:subClassOf [
      rdf:type owl:Restriction ;
      owl:allValuesFrom gsgq:Metamorphic_Grade ;
      owl:onProperty gsoc:isValueOf ;
    ] ;
  rdfs:subClassOf [
      rdf:type owl:Restriction ;
      owl:onClass gsgq:Metamorphic_Grade ;
      owl:onProperty gsoc:isValueOf ;
      owl:qualifiedCardinality "1"^^xsd:nonNegativeInteger ;
    ] ;
.
gsgq:Overturned
  rdf:type owl:Class ;
  rdfs:comment "top of surface is facing downward, toward Earth interior."@en ;
  rdfs:label "Overturned facing"@en ;
  rdfs:subClassOf gsgq:Facing_Value ;
.
gsgq:Plane_Orientation
  rdf:type owl:Class ;
  rdfs:comment "Quality to specify the orientation of a surface in a geogaphic reference system"@en ;
  rdfs:label "Plane orientation "@en ;
  rdfs:subClassOf gsoq:Orientation ;
.
gsgq:Plunge
  rdf:type owl:Class ;
  rdfs:comment "Numeric value should be between +90 and -90.   Negative values only valid if the linear feature is directed."@en ;
  rdfs:label "Plunge"@en ;
  rdfs:subClassOf gsoq:Orientation ;
  rdfs:subClassOf [
      rdf:type owl:Restriction ;
      owl:onProperty gsoc:hasQuality ;
      owl:someValuesFrom [
          rdf:type owl:Class ;
          owl:unionOf (
              gsoc:Numeric_Value
              gsoc:Named_Value
              gsoc:Range_Value
            ) ;
        ] ;
    ] ;
.
gsgq:Plunge_Value
  rdf:type owl:Class ;
  rdfs:subClassOf gsoq:Orientation_Value ;
  rdfs:subClassOf [
      rdf:type owl:Restriction ;
      owl:allValuesFrom gsgq:Plunge ;
      owl:onProperty gsoc:isValueOf ;
    ] ;
.
gsgq:Plunging_Line
  rdf:type owl:Class ;
  dct:source "Fleuty (1964) Folds classification." ;
  rdfs:comment "line plunges between 10 and 80 degrees."@en ;
  rdfs:label "Plunging line "@en ;
  rdfs:subClassOf gsgq:Plunge_Value ;
.
gsgq:Steeply_Inclined
  rdf:type owl:Class ;
  dct:source "Fleuty (1964) Folds classification." ;
  rdfs:comment "Surface dips between 60 and 80 degrees; typically used to describe orientation of fold hing surface or axial surface, but could be applied to any geologic surface."@en ;
  rdfs:label "Steeply Inclinded "@en ;
  rdfs:subClassOf gsgq:Inclined ;
.
gsgq:Steeply_Plunging_Line
  rdf:type owl:Class ;
  dct:source "Fleuty (1964) Folds classification." ;
  rdfs:comment "line plunges between 60 and 80 degrees."@en ;
  rdfs:label "Steeply plunging line"@en ;
  rdfs:subClassOf gsgq:Plunging_Line ;
.
gsgq:Unknown_Facing
  rdf:type owl:Class ;
  rdfs:comment "Facing direction is unknown {@en}	"@en ;
  rdfs:label "Unknown Facing Direction"@en ;
  rdfs:subClassOf gsgq:Facing_Value ;
.
gsgq:Upright_Facing
  rdf:type owl:Class ;
  dct:source "Fleuty (1964) Folds classification." ;
  rdfs:comment "top of surface is away from center of earth."@en ;
  rdfs:label "Upright facing"@en ;
  rdfs:subClassOf gsgq:Facing_Value ;
.
gsgq:Vertical_Inclination
  rdf:type owl:Class ;
  rdfs:comment "Surface dips between 80 and 90 degrees. Equivalent term 'upright' is used to describe orientation of fold hing surface or axial surface"@en ;
  rdfs:label "Vertical inclination "@en ;
  rdfs:subClassOf gsgq:Dip_Value ;
.
gsgq:Vertical_Line
  rdf:type owl:Class ;
  dct:source "Fleuty (1964) Folds classification." ;
  rdfs:comment "line plunges between 80 and 90 degrees."@en ;
  rdfs:label "Vertical line"@en ;
  rdfs:subClassOf gsgq:Plunge_Value ;
.
gsgq:Very_High_Metamorphic_Grade
  rdf:type owl:Class ;
  dct:source "Smulikowski et al, 2003; Fry, 1984"@en ;
  rdfs:comment "Protolith structures almost always obliterated. Includes rocks metamorphosed in granulite (or sanidinite), and high-temperature eclogite facies. Mineral assemblages according to Fry (1984) Table 10-1: ultramafic-olivine, enstatite, mafic-hypersthene, diopside (hornblende), calc-aluminous basic-plagioclase, pelite, semi-pelite -- hypersthene + Al-minerals (K-feldspar, quartz), or sapphirine."@en ;
  rdfs:label "very high metamorphic grade"@en ;
  rdfs:subClassOf gsgq:Metamorphosed ;
.
gsgq:Very_Low_Metamorphic_Grade
  rdf:type owl:Class ;
  dct:source "Smulikowski et al, 2003; Fry, 1984"@en ;
  rdfs:comment "Rock very slightly metamorphosed, protolith structure ubiquitous, mineral assemblage of zeolite facies, subgreenschist facies, or low temperature part of blueschist facies. Mineral assemblages according to Fry (1984) Table 10-1: ultramafic-serpentine (quartz, magnesite), mafic-clay, chlorite, relict igneous minerals, calc-aluminous basic-zeolite, pumpellite, epidote, albite, pelite, semi-pelite -- clays, chlorite, sericite, quartz."@en ;
  rdfs:label "very low metamorphic grade"@en ;
  rdfs:subClassOf gsgq:Metamorphosed ;
.
gsgq:ontology
  rdf:type owl:Ontology ;
  dct:created "2021-03-26"^^xsd:date ;
  dct:creator gsoc:boyan_brodaric ;
  dct:creator gsoc:stephen_richard ;
  dct:license <https://creativecommons.org/licenses/by/4.0/legalcode> ;
  dct:modified "2021-03-26"^^xsd:date ;
  dct:publisher "ARC Loop3D project;  https://loop3d.org/" ;
  dct:publisher "Geological Survey of Canada, Natural Resources Canada, Government of Canada" ;
    schema:codeRepository "https://github.com/Loop3D/GKM";  dct:rights  "Copyright (c) 2021 Government of Canada" ;
  rdfs:comment "Physical qualities used in multiple GSO modules."@en ;
  rdfs:label "Geoscience Ontology, Geologic Qualities"@en ;
  dct:bibliographicCitation "Brodaric, B., and Richard, S.M., 2021, The GeoScience Ontology Reference: Geological Survey of Canada Open File 8796, 34 p., https://doi.org/10.4095/328296";
  owl:imports gsoc:ontology ;
  owl:imports gsog:ontology ;
  owl:imports gsoq:ontology ;
  skos:definition "Physical qualities used in multiple GSO modules."@en ;
  skos:prefLabel "Geoscience Ontology, Geologic Qualities"@en ;
.
