# baseURI: http://loop3d.org/GSO/ontology/2020/1/geologiccontact/ontology
# imports: http://loop3d.org/GSO/ontology/2020/1/common/ontology
# imports: http://loop3d.org/GSO/ontology/2020/1/geologicfeature/ontology
# imports: http://loop3d.org/GSO/ontology/2020/1/geology/ontology
# imports: http://loop3d.org/GSO/ontology/2020/1/quality/ontology

@prefix : <http://loop3d.org/GSO/ontology/2020/1/geologiccontact/> .
@prefix gscn: <http://loop3d.org/GSO/ontology/2020/1/geologiccontact/> .
@prefix gsgf: <http://loop3d.org/GSO/ontology/2020/1/geologicfeature/> .
@prefix gsoc: <http://loop3d.org/GSO/ontology/2020/1/common/> .
@prefix gsog: <http://loop3d.org/GSO/ontology/2020/1/geology/> .
@prefix gsoq: <http://loop3d.org/GSO/ontology/2020/1/quality/> .
@prefix owl: <http://www.w3.org/2002/07/owl#> .
@prefix rdf: <http://www.w3.org/1999/02/22-rdf-syntax-ns#> .
@prefix rdfs: <http://www.w3.org/2000/01/rdf-schema#> .
@prefix xml: <http://www.w3.org/XML/1998/namespace> .
@prefix xsd: <http://www.w3.org/2001/XMLSchema#> .

gscn:Alteration_Facies_Contact
  rdf:type owl:Class ;
  rdfs:comment "A metasomatic facies contact separating rocks that have undergone alteration of a particular facies from those that have undergone metasomatism of another facies. Alteration is a kind of metasomatism that does not introduce economically important minerals."@en ;
  rdfs:comment "dct:source--  CGI contacttype SKOS vocabulary 2012-11-24"@en ;
  rdfs:label "alteration facies contact"@en ;
  rdfs:subClassOf gscn:Metamorphic_Contact ;
.
gscn:Angular_Unconformable_Contact
  rdf:type owl:Class ;
  rdfs:comment "An unconformable contact between two geological units in which the older, underlying rocks dip at an angle different from the younger, overlying strata, usually in which younger sediments rest upon the eroded surface of tilted or folded older rocks."@en ;
  rdfs:comment "dct:source--  Neuendorf, K.K.E, Mehl, J.P. & Jackson, J.A. (eds), 2005. Glossary of geology, 5th Edition. American Geological Institute, Alexandria, 779 p."@en ;
  rdfs:label "angular unconformable contact"@en ;
  rdfs:subClassOf gscn:Unconformable_Contact ;
.
gscn:Buttress_Unconformity
  rdf:type owl:Class ;
  rdfs:comment "An unconformity in which onlapping strata are truncated against a steep topographic scarp."@en ;
  rdfs:comment "dct:source--  Neuendorf, K.K.E, Mehl, J.P. & Jackson, J.A. (eds), 2005. Glossary of geology, 5th Edition. American Geological Institute, Alexandria, 779 p."@en ;
  rdfs:label "buttress unconformity"@en ;
  rdfs:subClassOf gscn:Unconformable_Contact ;
.
gscn:Chronostratigraphic_Zone_Contact
  rdf:type owl:Class ;
  rdfs:comment "A contact between bodies of material having different ages of origin."@en ;
  rdfs:comment "dct:source--  FGDC"@en ;
  rdfs:label "chronostratigraphic-zone contact"@en ;
  rdfs:subClassOf gscn:Contact ;
.
gscn:Conductivity_Contact
  rdf:type owl:Class ;
  rdfs:comment "A geophysical contact between bodies of material distinguished based on electrical conductivity characteristics"@en ;
  rdfs:comment "dct:source--  CGI contacttype SKOS vocabulary 2012-11-24"@en ;
  rdfs:label "conductivity contact"@en ;
  rdfs:subClassOf gscn:Geophysical_Contact ;
.
gscn:Conformable_Contact
  rdf:type owl:Class ;
  rdfs:comment "A contact separating two geological units in which the layers are formed one above the other in order by regular, uninterrupted deposition under the same general conditions."@en ;
  rdfs:comment "dct:source--  Neuendorf, K.K.E, Mehl, J.P. & Jackson, J.A. (eds), 2005. Glossary of geology, 5th Edition. American Geological Institute, Alexandria, 779 p."@en ;
  rdfs:label "conformable contact"@en ;
  rdfs:subClassOf gscn:Depositional_Contact ;
.
gscn:Contact
  rdf:type owl:Class ;
  rdfs:comment "A surface that separates geologic units. Very general concept representing any kind of surface separating two geologic units, including primary boundaries such as depositional contacts, all kinds of unconformities, intrusive contacts, and gradational contacts, as well as faults that separate geologic units. (CGI ContactType vocabulary, adapted from Jackson, 1997, page 137, NADM C1 2004)"@en ;
  rdfs:label "Contact"@en ;
  rdfs:subClassOf gsoc:Low_Dimension_Feature ;
  rdfs:subClassOf gsog:Geologic_Structure ;
  rdfs:subClassOf [
      rdf:type owl:Restriction ;
      owl:minQualifiedCardinality "2"^^xsd:nonNegativeInteger ;
      owl:onClass gsog:Rock_Body_Boundary ;
      owl:onProperty gsoc:hostedBy ;
    ] ;
.
gscn:Deformation_Zone_Contact
  rdf:type owl:Class ;
  rdfs:comment "A lithogenetic bundary separating rock masses that have different deformation structure, e.g. sheared rock against non sheared rock, brecciated rock against non-brecciated rock."@en ;
  rdfs:comment "dct:source--  CGI contacttype SKOS vocabulary 2012-11-24"@en ;
  rdfs:label "deformation zone contact"@en ;
  rdfs:subClassOf gscn:Lithogenetic_Contact ;
.
gscn:Density_Contact
  rdf:type owl:Class ;
  rdfs:comment "A geophysical contact separating bodies of material with different density characteristics, generally determined through measurement and modelling of gravity variations."@en ;
  rdfs:comment "dct:source--  CGI contacttype SKOS vocabulary 2012-11-24"@en ;
  rdfs:label "density contact"@en ;
  rdfs:subClassOf gscn:Geophysical_Contact ;
.
gscn:Depositional_Contact
  rdf:type owl:Class ;
  rdfs:comment "Lithogenetic contact at which a sedimentary or volcanic rock has been deposited on (or against) another rock body. The relationship between the older underlying rocks and younger overlying rocks is unknown or not specfied."@en ;
  rdfs:comment "dct:source--  CGI contacttype SKOS vocabulary 2012-11-24"@en ;
  rdfs:label "depositional contact"@en ;
  rdfs:subClassOf gscn:Lithogenetic_Contact ;
.
gscn:Disconformable_Contact
  rdf:type owl:Class ;
  rdfs:comment "An unconformable contact between two geological units in which the bedding of the older, underlying unit is parallel to the bedding of the younger, overlying unit, but in which the contact between the two units is marked by an irregular or uneven surface of appreciable relief."@en ;
  rdfs:comment "dct:source--  Neuendorf, K.K.E, Mehl, J.P. & Jackson, J.A. (eds), 2005. Glossary of geology, 5th Edition. American Geological Institute, Alexandria, 779 p."@en ;
  rdfs:label "disconformable contact"@en ;
  rdfs:subClassOf gscn:Unconformable_Contact ;
.
gscn:Faulted_Contact
  rdf:type owl:Class ;
  rdfs:comment "A contact separating two bodies of material across which one body has slid past the other."@en ;
  rdfs:comment "dct:source--  Neuendorf, K.K.E, Mehl, J.P. & Jackson, J.A. (eds), 2005. Glossary of geology, 5th Edition. American Geological Institute, Alexandria, 779 p."@en ;
  rdfs:label "faulted contact"@en ;
  rdfs:subClassOf gscn:Contact ;
.
gscn:Geologic_Province_Contact
  rdf:type owl:Class ;
  rdfs:comment "A contact between regions characterised by their geological history or by similar structural, petrographic or stratigraphic features"@en ;
  rdfs:comment "dct:source--  Neuendorf, K.K.E, Mehl, J.P. & Jackson, J.A. (eds), 2005. Glossary of geology, 5th Edition. American Geological Institute, Alexandria, 779 p."@en ;
  rdfs:label "geologic province contact"@en ;
  rdfs:subClassOf gscn:Contact ;
.
gscn:Geophysical_Contact
  rdf:type owl:Class ;
  rdfs:comment "A contact separating bodies of material in the earth that have different geophysical properties. Use for boundaries that are detected by geophysical sensor techniques as opposed to direct lithologic observation."@en ;
  rdfs:comment "dct:source--  CGI contacttype SKOS vocabulary 2012-11-24"@en ;
  rdfs:label "geophysical contact"@en ;
  rdfs:subClassOf gscn:Contact ;
.
gscn:Glacial_Stationary_Line
  rdf:type owl:Class ;
  rdfs:comment "A boundary between a subglacial geomorphic unit and a periglacial geomorphic unit, marking the maximum extent of glacial cover. This can be thought of as the outcrop of the contact between a glacier and its substrate at some time at each point along the boundary. This contact type is included as an interim concept, assuming that in the future, there will be extensions to account better for geomorphic units and line types."@en ;
  rdfs:comment "dct:source--  CGI contacttype SKOS vocabulary 2012-11-24"@en ;
  rdfs:label "glacial stationary line"@en ;
  rdfs:subClassOf gscn:Contact ;
.
gscn:Gradational_Contact_Zone
  rdf:type owl:Class ;
  rdfs:label "Gradational Contact Zone"@en ;
  rdfs:subClassOf gsoc:Material_Feature ;
  rdfs:subClassOf [
      rdf:type owl:Restriction ;
      owl:minQualifiedCardinality "2"^^xsd:nonNegativeInteger ;
      owl:onClass gsog:Rock_Body ;
      owl:onProperty gsoc:hostedBy ;
    ] ;
  rdfs:subClassOf [
      rdf:type owl:Restriction ;
      owl:onProperty gsoc:contains ;
      owl:someValuesFrom gscn:Contact ;
    ] ;
  rdfs:subClassOf [
      rdf:type owl:Restriction ;
      owl:onProperty gsoc:hasEssentialPart ;
      owl:someValuesFrom gsog:Rock_Body ;
    ] ;
  rdfs:subClassOf [
      rdf:type owl:Restriction ;
      owl:onProperty gsoc:hasQuality ;
      owl:someValuesFrom gsoq:Thickness ;
    ] ;
.
gscn:Igneous_Intrusive_Contact
  rdf:type owl:Class ;
  rdfs:comment "An intrusive contact between a younger igneous rock and an older, pre-existing geological unit into which it has been intruded."@en ;
  rdfs:comment "dct:source--  Neuendorf, K.K.E, Mehl, J.P. & Jackson, J.A. (eds), 2005. Glossary of geology, 5th Edition. American Geological Institute, Alexandria, 779 p."@en ;
  rdfs:label "igneous intrusive contact"@en ;
  rdfs:subClassOf gscn:Lithogenetic_Contact ;
.
gscn:Igneous_Phase_Contact
  rdf:type owl:Class ;
  rdfs:comment "A lithogenetic contact separating lithologically distinct phases of a single intrusive body. Does not denote nature of contact (intrusive or gradation)."@en ;
  rdfs:comment "dct:source--  CGI contacttype SKOS vocabulary 2012-11-24"@en ;
  rdfs:label "igneous phase contact"@en ;
  rdfs:subClassOf gscn:Lithogenetic_Contact ;
.
gscn:Impact_Structure_Boundary
  rdf:type owl:Class ;
  rdfs:comment "dct:source--  CGI contacttype SKOS vocabulary 2012-11-24"@en ;
  rdfs:comment "surface that bounds a body of rock affected by an extraterrestrial impact event"@en ;
  rdfs:label "impact structure boundary"@en ;
  rdfs:subClassOf gscn:Lithogenetic_Contact ;
.
gscn:Lithogenetic_Contact
  rdf:type owl:Class ;
  rdfs:comment "A non-faulted contact separating bodies of material in the earth that have different lithologic character or geologic history."@en ;
  rdfs:comment "dct:source--  CGI contacttype SKOS vocabulary 2012-11-24"@en ;
  rdfs:label "lithogenetic contact"@en ;
  rdfs:subClassOf gscn:Contact ;
.
gscn:Magnetic_Contact
  rdf:type owl:Class ;
  rdfs:comment "A geophysical contact separating bodies of material distinguished based on properties related to magnetic fields."@en ;
  rdfs:comment "dct:source--  CGI contacttype SKOS vocabulary 2012-11-24"@en ;
  rdfs:label "magnetic contact"@en ;
  rdfs:subClassOf gscn:Geophysical_Contact ;
.
gscn:Magnetic_Polarity_Contact
  rdf:type owl:Class ;
  rdfs:comment "A magentic contact between bodies of material with different polarity of remnant magnetization, e.g. between sections of ocean floor with different polarity."@en ;
  rdfs:comment "dct:source--  CGI contacttype SKOS vocabulary 2012-11-24"@en ;
  rdfs:label "magnetic polarity contact"@en ;
  rdfs:subClassOf gscn:Magnetic_Contact ;
.
gscn:Magnetic_Susceptiblity_Contact
  rdf:type owl:Class ;
  rdfs:comment "A magnetic contact between bodies of material distinguished based on magnetic susceptibility characteristics."@en ;
  rdfs:comment "dct:source--  CGI contacttype SKOS vocabulary 2012-11-24"@en ;
  rdfs:label "magnetic susceptiblity contact"@en ;
  rdfs:subClassOf gscn:Magnetic_Contact ;
.
gscn:Magnetization_Contact
  rdf:type owl:Class ;
  rdfs:comment "A magnetic contact between bodies of material distinguished based on any aspect of magnetization of material in the units."@en ;
  rdfs:comment "dct:source--  CGI contacttype SKOS vocabulary 2012-11-24"@en ;
  rdfs:label "magnetization contact"@en ;
  rdfs:subClassOf gscn:Magnetic_Contact ;
.
gscn:Metamorphic_Contact
  rdf:type owl:Class ;
  rdfs:comment "Lithogenetic contact separating rocks that have different lithologic properties related to metamorphism, metasomatism, alteration, or mineralization. Generally separates metamorphic rock bodies, but may separate metamorphosed (broadly speaking) and non-metamorphosed rock."@en ;
  rdfs:comment "dct:source--  CGI contacttype SKOS vocabulary 2012-11-24"@en ;
  rdfs:label "metamorphic contact"@en ;
  rdfs:subClassOf gscn:Lithogenetic_Contact ;
.
gscn:Metamorphic_Facies_Contact
  rdf:type owl:Class ;
  rdfs:comment "A metamorphic contact separating rocks that have undergone metamorphism of a particular facies from those that have undergone metamorphism of another facies."@en ;
  rdfs:comment "dct:source--  CGI contacttype SKOS vocabulary 2012-11-24"@en ;
  rdfs:label "metamorphic facies contact"@en ;
  rdfs:subClassOf gscn:Metamorphic_Contact ;
.
gscn:Metasomatic_Facies_Contact
  rdf:type owl:Class ;
  rdfs:comment "A metamorphic contact separating rocks that have undergone metasomatism of a particular facies from those that have undergone metasomatism of another facies. Metasomatism is distinguished from metamorphism by significant changes in bulk chemistry of the affected rock."@en ;
  rdfs:comment "dct:source--  CGI contacttype SKOS vocabulary 2012-11-24"@en ;
  rdfs:label "metasomatic facies contact"@en ;
  rdfs:subClassOf gscn:Metamorphic_Contact ;
.
gscn:Mineralisation_Assemblage_Contact
  rdf:type owl:Class ;
  rdfs:comment "A metasomatic facies contact separating rocks which have been mineralised and contain a particular mineral assemblage from those which contain a different assemblage. Mineralization is a kind of metasomatism that introduces ecomomically important minerals."@en ;
  rdfs:comment "dct:source--  CGI contacttype SKOS vocabulary 2012-11-24"@en ;
  rdfs:label "mineralisation assemblage contact"@en ;
  rdfs:subClassOf gscn:Metamorphic_Contact ;
.
gscn:Nonconformable_Contact
  rdf:type owl:Class ;
  rdfs:comment "An unconformable contact between an underlying, older nonstratified geological unit (usually intrusive igneous rocks or metamorphics) and an overlying, younger stratified geological unit."@en ;
  rdfs:comment "dct:source--  Neuendorf, K.K.E, Mehl, J.P. & Jackson, J.A. (eds), 2005. Glossary of geology, 5th Edition. American Geological Institute, Alexandria, 779 p."@en ;
  rdfs:label "nonconformable contact"@en ;
  rdfs:subClassOf gscn:Unconformable_Contact ;
.
gscn:Paraconformable_Contact
  rdf:type owl:Class ;
  rdfs:comment "An unconformable contact between two geological units in which the bedding of the older, underlying unit is parallel to the bedding of the younger, overlying unit, in which the contact between the two units is planar, and may be coincident with a bedding plane."@en ;
  rdfs:comment "dct:source--  Neuendorf, K.K.E, Mehl, J.P. & Jackson, J.A. (eds), 2005. Glossary of geology, 5th Edition. American Geological Institute, Alexandria, 779 p."@en ;
  rdfs:label "paraconformable contact"@en ;
  rdfs:subClassOf gscn:Unconformable_Contact ;
.
gscn:Radiometric_Contact
  rdf:type owl:Class ;
  rdfs:comment "A geophysical contact separating bodies of material distinguished based on the characteristics of emitted of radiant energy related to radioactivity (e.g. gamma rays)."@en ;
  rdfs:comment "dct:source--  CGI contacttype SKOS vocabulary 2012-11-24"@en ;
  rdfs:label "radiometric contact"@en ;
  rdfs:subClassOf gscn:Geophysical_Contact ;
.
gscn:Sedimentary_Facies_Contact
  rdf:type owl:Class ;
  rdfs:comment "A lithogenetic contact separating essentially coeval sedimentary material bodies distinguished by characteristics reflecting different physical or chemical processes active at the time of deposition of the sediment."@en ;
  rdfs:comment "dct:source--  base on Nichols, Gary, 1999, Sedimentology and stratigraphy, Blackwell, p. 62-63."@en ;
  rdfs:label "sedimentary facies contact"@en ;
  rdfs:subClassOf gscn:Lithogenetic_Contact ;
.
gscn:Sedimentary_Intrusive_Contact
  rdf:type owl:Class ;
  rdfs:comment "An intrusive contact between a sedimentary rock unit and plastic sediment (e.g., clay, chalk, salt, gypsum, etc.), forced upward into it from underlying sediment"@en ;
  rdfs:comment "dct:source--  Neuendorf, K.K.E, Mehl, J.P. & Jackson, J.A. (eds), 2005. Glossary of geology, 5th Edition. American Geological Institute, Alexandria, 779 p."@en ;
  rdfs:label "sedimentary intrusive contact"@en ;
  rdfs:subClassOf gscn:Lithogenetic_Contact ;
.
gscn:Seismic_Contact
  rdf:type owl:Class ;
  rdfs:comment "A geophysical contact separating bodies of material defined based on their seismic character. Seismic character is based on transmission of vibrations (seismic waves) through a rock body, and relates to the velocity of transmission, and the nature of reflection, refraction, or transformation of seismic waves by inhomogeneities in the rock body."@en ;
  rdfs:comment "dct:source--  CGI contacttype SKOS vocabulary 2012-11-24"@en ;
  rdfs:label "seismic contact"@en ;
  rdfs:subClassOf gscn:Geophysical_Contact ;
.
gscn:Stratigraphic_Point
  rdf:type owl:Class ;
  rdfs:comment "A spatially restricted part of a Contact feature, typically located by a point location. "@en ;
  rdfs:label "Stratigraphic Point"@en ;
  rdfs:subClassOf gscn:Contact ;
  rdfs:subClassOf [
      rdf:type owl:Restriction ;
      owl:allValuesFrom gsoc:Spatial_Region_0D ;
      owl:onProperty gsoc:hasEssentialPart ;
    ] ;
  rdfs:subClassOf [
      rdf:type owl:Restriction ;
      owl:onClass gsoc:Spatial_Region_0D ;
      owl:onProperty gsoc:hasEssentialPart ;
      owl:qualifiedCardinality "1"^^xsd:nonNegativeInteger ;
    ] ;
  rdfs:subClassOf [
      rdf:type owl:Restriction ;
      owl:onProperty gsoc:isPartOf ;
      owl:someValuesFrom gscn:Contact ;
    ] ;
  rdfs:subClassOf [
      rdf:type owl:Restriction ;
      owl:onProperty gsoc:staticHostedBy ;
      owl:someValuesFrom gsgf:Stratigraphic_Section ;
    ] ;
.
gsog:GSSP
  rdfs:subClassOf [
      rdf:type owl:Restriction ;
      owl:onProperty gsoc:staticHostedBy ;
      owl:someValuesFrom gsgf:Stratigraphic_Point ;
    ] ;
  rdfs:subClassOf [
      rdf:type owl:Restriction ;
      owl:onProperty gsoc:staticHostedBy ;
      owl:someValuesFrom gsgf:Stratigraphic_Section ;
    ] ;
  rdfs:subClassOf [
      rdf:type owl:Restriction ;
      owl:onProperty gsoc:determinedBy ;
      owl:someValuesFrom gsgf:Stratigraphic_Point ;
    ] ;
.
gscn:Unconformable_Contact
  rdf:type owl:Class ;
  rdfs:comment "A contact separating two geological units in which the younger unit succeeds the older after a substantial hiatus in deposition."@en ;
  rdfs:comment "dct:source--  Neuendorf, K.K.E, Mehl, J.P. & Jackson, J.A. (eds), 2005. Glossary of geology, 5th Edition. American Geological Institute, Alexandria, 779 p."@en ;
  rdfs:label "unconformable contact"@en ;
  rdfs:subClassOf gscn:Depositional_Contact ;
.
gscn:Volcanic_Subsidence_Zone_Boundary
  rdf:type owl:Class ;
  rdfs:comment "boundary around a body of rock that is within a zone of subsidence or cratering produced by volcanic activity."@en ;
  rdfs:comment "dct:source--  this vocabulary, concept to encompass boundary of caldron, caldera, or crater."@en ;
  rdfs:label "volcanic subsidence zone boundary"@en ;
  rdfs:subClassOf gscn:Lithogenetic_Contact ;
.
gscn:Weathering_Contact
  rdf:type owl:Class ;
  rdfs:comment "A lithogenetic contact separating bodies of material differentiated based on lithologic properties related to weathering."@en ;
  rdfs:comment "dct:source--  CGI contacttype SKOS vocabulary 2012-11-24"@en ;
  rdfs:label "weathering contact"@en ;
  rdfs:subClassOf gscn:Lithogenetic_Contact ;
.
gscn:ontology
  rdf:type owl:Ontology ;
  rdfs:comment "This file contains the 2016 SKOS-RDF version of the CGI Contact Type vocabulary. Compilation and review in MS Excel spreadsheet, converted to MS Excel for SKOS generation using GSML_SKOS_fromXLS_2016.01.xslt."@en ;
  rdfs:comment "This vocabulary specifies Contact Type concepts, as defined by the IUGS Commission for Geoscience Information (CGI) Geoscience Terminology Working Group. Originally designed for use in the contactType property in GeoSciML Contact elements, adopt here as subClasses of gscn:Contact."@en ;
  rdfs:comment "dct:creator--  CGI Concept Definition Task Group, Stephen Richard Owl adoption for Loop3D project"@en ;
  rdfs:comment "dct:date--  2012-11-24"@en ;
  rdfs:comment "dct:modified-- 2020-01-29"@en ;
  rdfs:label "Contact"@en ;
  owl:imports gsoc:ontology ;
  owl:imports gsgf:ontology ;
  owl:imports gsog:ontology ;
  owl:imports gsoq:ontology ;
.
gsgf:Boundary_Stratotype
  rdf:type owl:Class ;
  rdfs:subClassOf [
      rdf:type owl:Restriction ;
      owl:onProperty gsoc:isExampleOf ;
      owl:someValuesFrom gscn:Contact ;
    ] ;
.
