# baseURI: https://w3id.org/gso/gso-gts/ontology
# imports: http://resource.geosciml.org/ontology/timescale/gts
# imports: http://resource.geosciml.org/ontology/timescale/thors
# imports: http://www.w3.org/2006/time
# imports: http://www.w3.org/ns/sosa/
# imports: https://w3id.org/gso/geologictime/ontology
# imports: https://w3id.org/gso/ischart/ontology

@prefix : <https://w3id.org/gso/gso-gts/> .
@prefix dbp: <http://dbpedia.org/resource/> .
@prefix dct: <http://purl.org/dc/terms/> .
@prefix gscn: <https://w3id.org/gso/geologiccontact/> .
@prefix gsgu: <https://w3id.org/gso/geologicunit/> .
@prefix gsoc: <https://w3id.org/gso/common/> .
@prefix gsog: <https://w3id.org/gso/geology/> .
@prefix gst: <https://w3id.org/gso/geologictime/> .
@prefix gts: <http://resource.geosciml.org/ontology/timescale/gts#> .
@prefix ischart: <https://w3id.org/gso/ischart/> .
@prefix owl: <http://www.w3.org/2002/07/owl#> .
@prefix rdf: <http://www.w3.org/1999/02/22-rdf-syntax-ns#> .
@prefix rdfs: <http://www.w3.org/2000/01/rdf-schema#> .
@prefix schema: <https://schema.org/> .
@prefix skos: <http://www.w3.org/2004/02/skos/core#> .
@prefix thors: <http://resource.geosciml.org/ontology/timescale/thors#> .
@prefix time: <http://www.w3.org/2006/time#> .
@prefix unit: <http://qudt.org/vocab/unit/> .
@prefix xml: <http://www.w3.org/XML/1998/namespace> .
@prefix xsd: <http://www.w3.org/2001/XMLSchema#> .

gts:GeochronologicBoundary
  rdfs:comment "#subclass of thors:EraBoundary, stratotype only stratigraphicPoint." ;
  owl:equivalentClass gsog:Geologic_Time_Boundary ;
.
gts:GeochronologicEra
  rdfs:comment "#gts era has gts:rank, gts:stratotype (optional), and skos:notation, subclass from thors:Era" ;
  owl:equivalentClass gsog:Geologic_Time_Interval ;
.
gts:GeologicTimescale
  owl:equivalentClass gsog:Geologic_Time_Scale ;
.
gts:NumericEraBoundary
  rdfs:comment "in practice the classes have the same extension" ;
  owl:equivalentClass gsog:GSSA ;
.
thors:Era
  rdfs:comment "gsoc:timeHasBeginning | gsoc:timeHasEnd some  gsoc:Temporal_Boundary.  thors:Era has thors:begin and :end properties with range thors:EraBoundary, but both properties are listed as deprecated. use gsoc:Temporal_Boundary because the time instants are coupled to the Era they bound, making them features." ;
  owl:subClassOf gsoc:Time_Interval_Feature ;
.
thors:EraBoundary
  rdfs:subClassOf gsoc:Temporal_Boundary ;
.
thors:component
  rdfs:comment "range of thors:component is thors:Era, domain is referenceSystem. Use to indentify intervals that are included in a a thors:ReferenceSystem." ;
  rdfs:subPropertyOf gsoc:timeIncludes ;
.
thors:referencePoint
  rdfs:comment "gsoc:timeHasBeginning | gsoc:timeHasEnd some  gsoc:Temporal_Boundary. thors referencePOint are thors:EraBoundary objects. domain is referenc system." ;
  rdfs:comment "owl:equivalentProperty gsoc:timeHasBeginning ";
  rdfs:subPropertyOf gsoc:timeHasBeginning ;
.
time:Instant
  rdfs:comment "owlsameAs gsoc:Time_Instant";
    rdfs:subClassOf gsoc:Time_Instant ;
.
time:ProperInterval
  rdfs:comment "owl:sameAs gsoc:Time_Interval" ;
  rdfs:subClassOf gsoc:Time_Interval
.
time:TRS
  rdfs:subClassOf gsoc:Temporal_Reference_System ;
.
time:TemporalEntity
  rdf:type owl:thing ;
  rdfs:comment "all time:TemporalEntity are gsoc:Time_Region, but not vice versa" ;
  rdfs:subClassOf gsoc:Time_Region ;
.
time:inside
  rdfs:comment " time:inside is narrower; doesn't allow timeStartedBy and timeFinishedBy where the object is an instant, or timeEquivalentTo." ;
  owl:subPropertyOf gsoc:timeContains ;
  owl:subPropertyOf gsoc:timeIncludes ;
.
time:intervalAfter
  rdfs:subPropertyOf gsoc:timeYoungerThan ;
.
time:intervalBefore
  rdfs:subPropertyOf gsoc:timeOlderThan ;
.
time:intervalContains
  owl:subPropertyOf gsoc:timeContains ;
.
time:intervalDisjoint
  rdfs:subPropertyOf gsoc:timeDisjoint ;
.
time:intervalDuring
  rdfs:comment "OWL Time time:intervalDuring is narrower, only relates ProperIntervals."@en ;
  owl:subPropertyOf gsoc:timeDuring ;
.
time:intervalEquals
  rdfs:comment "OWL Time time:intervalEquals is narrower-only relates intervals. GSO allow interval or instant, direct or indirect." ;
  owl:subPropertyOf gsoc:timeEquivalentTo ;
.
time:intervalFinishedBy
  rdfs:comment "OWL time time:intervalFinsishedBy is narrower, only finishing time entity can only be interval time_region. GSO allow interval or instant, direct or indirect." ;
  owl:subPropertyOf gsoc:timeFinishedBy ;
.
time:intervalFinishes
  rdfs:comment "OWL time time:Finishes is narrower, only finishing time entity can only be interval time_region. GSO allow interval or instant, direct or indirect." ;
  owl:subPropertyOf gsoc:timeFinishes ;
.
time:intervalIn
  rdfs:comment ".  OWL Time time:intervalIn is subproperty, restricted to relating intervals, and not including timeEquivalentTo" ;
  owl:subPropertyOf gsoc:timeIncludedBy ;
.
time:intervalStartedBy
  owl:subPropertyOf gsoc:timeStartedBy ;
.
time:intervalStarts
  rdfs:comment "OWL time time:intervalStarts is narrower; only relates ProperInterval" ;
  owl:subPropertyOf gsoc:timeStarts ;
.
gsoc:Temporal_Value
  rdfs:subClassOf time:TemporalPosition ;
.
gsoc:Time_Interval_Reference_System
  rdfs:subClassOf thors:ReferenceSystem ;
.
gsoc:Time_Numeric_Value
  rdfs:comment "rdfs:subClassOf (time:TimePosition and (time:numericPosition exactly 1)) ;.  range of timePosition allows nominal position with a string value. In GSO this would need to be a timeInterval that is included in a Time_Interval_Reference_System" ;
  rdfs:subClassOf time:TimePosition ;
.
gsoc:hostedBy
  rdf:type owl:ObjectProperty ;
  rdfs:comment "this doesn't have any direct mapping into the owl:time, gts:, thors: view of things. It emerges from Boyan's modeling of 'features', which is different from the OGC concept. In practical terms, for the one direct mapping I've tried, it maps to gts:stratotype in the context of a geologic time boundary.";
.
time:intervalMeets 
	rdfs:subPropertyOf gsoc:nextTimeInterval;
	rdfs:comment "gsoc:nextTimeInterval  owl:equivalentProperty time:intervalMeets ;";
.
gsoc:timeContains
  rdf:type owl:ObjectProperty ;
  rdfs:comment "Equivalent to union of OWL Time time:intervalContains and time:inside" ;
.
gst:Age
  owl:equivalentClass gts:Age ;
.
gst:Eon
  owl:equivalentClass gts:Eon ;
.
gst:Epoch
  owl:equivalentClass gts:Epoch ;
.
gst:Era
  owl:equivalentClass gts:Era ;
.
gst:Period
  owl:equivalentClass gts:Period ;
.
gst:Supereon
  owl:equivalentClass gts:Supereon ;
.
gsgu:Chronostratigraphic_Unit
  rdf:type owl:Thing ;
  rdfs:comment "no gts: equivalent?" ;
.
gsog:Generic_Geologic_Time_Unit
  rdf:type owl:Thing ;
    rdfs:comment "no gts: equivalent, but broadly corresponds to gts:GeochronologicEra" ;
.
:ontology
  rdf:type owl:Ontology ;
  dct:created "2021-12-18"^^xsd:date ;
  dct:modified "2023-05-04 SMR change owl:sameAs to rdfs:subClassOf "@en 
  rdfs:comment "construct to map gso time classes and properties to owl:time, gts, and thors" ;
  skos:historyNote "change owl:sameAs to rdfs:subClassOf "@en ;
  owl:imports <http://resource.geosciml.org/ontology/timescale/gts> ;
  owl:imports <http://resource.geosciml.org/ontology/timescale/thors> ;
  owl:imports <http://www.w3.org/2006/time> ;
  owl:imports <http://www.w3.org/ns/sosa/> ;
  owl:imports gst:ontology ;
  owl:imports ischart:ontology ;
.
