# baseURI: http://loop3d.org/GSO/ontology/2020/1/lithology/materialcategory/ontology
# imports: http://loop3d.org/GSO/ontology/2020/1/geologicfeature/ontology
# imports: http://loop3d.org/GSO/ontology/2020/1/geologicquality/ontology

@prefix gslth: <http://loop3d.org/GSO/ontology/2020/1/lithology/> .
@prefix gsmc: <http://loop3d.org/GSO/ontology/2020/1/lithology/materialcategory/> .
@prefix gsog: <http://loop3d.org/GSO/ontology/2020/1/geologicfeature/> .
@prefix owl: <http://www.w3.org/2002/07/owl#> .
@prefix rdf: <http://www.w3.org/1999/02/22-rdf-syntax-ns#> .
@prefix rdfs: <http://www.w3.org/2000/01/rdf-schema#> .
@prefix xml: <http://www.w3.org/XML/1998/namespace> .
@prefix xsd: <http://www.w3.org/2001/XMLSchema#> .

gsmc:Mono-mineralic_crystal_particle_material
  rdfs:subClassOf gsmc:Mono_mineralic_granular_material ;
.


gsmc:fluidal_pyroclastic_granular_material
  rdfs:subClassOf gsog:pyroclastic_granular_material ;
.
gsmc:glass_shard_granular_material
  rdfs:subClassOf gsog:pyroclastic_granular_material ;
.
gsmc:hydroclastic_granular_material
  rdfs:subClassOf gsog:pyroclastic_granular_material ;
.



gsmc:Axiolitic_granular_material
  a owl:Class ;
  rdfs:comment "Material that is a collection of elongate to irregular lenticular particles with radial aggregates of acicular and fibrous mineral coalescing along a central axis."@en ;
  rdfs:comment "dct:source--  Williams, Turner, Gilbert 1954"@en ;
  rdfs:label "Axiolitic granular material"@en ;
  rdfs:subClassOf gsog:Aggregate_non-clastic_particle_material ;
.
gsmc:Bleb_granular_material
  a owl:Class ;
  rdfs:comment "Granular material composed of small rounded particle of uncertain origin"@en ;
  rdfs:comment "dct:source--  this vocabulary"@en ;
  rdfs:label "bleb"@en ;
  rdfs:subClassOf gsog:Granular_Material ;
.
gsmc:Concretionary_particle_material
  a owl:Class ;
  rdfs:comment "Granular material composed of particles that are hard, compact masses or aggregates of mineral matter, normally subsperical but commonly oblate, disc-shaped or irregular. Formed by precipitation of mineral from solution in the pores of a granular rock, localized around a nucleus or center, to define a discrete, sharply separated object. Size ranges from cm to meters. Particle geometry description for concretion describes the concretion size and shape, not the size and shape of particles forming the concretion."@en ;
  rdfs:comment "dct:source--  Neuendorf et al, 2005"@en ;
  rdfs:label "concretionary particle material"@en ;
  rdfs:subClassOf gsog:Aggregate_non-clastic_particle_material ;
.
gsmc:Crystallite
  a owl:Class ;
  rdfs:comment "Granular material consisting of minute, spherical, rod, or hair-like particles, mineralogy not discernible with hand lense. Typically appear isotropic in thin section."@en ;
  rdfs:comment "dct:source--  Williams, Turner, Gilbert 1954"@en ;
  rdfs:label "crystallite"@en ;
  rdfs:subClassOf gsog:Crystallized_Particle_Material ;
.
gsmc:Glomerocryst_granular_material
  a owl:Class ;
  rdfs:comment "Granular material consisting of particles that are aggregates of crystals of the same mineral"@en ;
  rdfs:comment "Typically will not play a framework role in a Rock Material.  Expect these to be conceptually like a sub class of phenocryst, but avoid that commitment for now."@en ;
  rdfs:comment "dct:source--  definition of glomerocryst from Neuendorf et al., 2005"@en ;
  rdfs:label "glomerocryst granular material"@en ;
  rdfs:subClassOf gsog:Aggregate_non-clastic_particle_material ;
.
gsmc:Lithic_rich_epiclastic_material
  a owl:Class ;
  rdfs:comment "Epiclastic material consisting largely of lithic rock fragment particles. Qualitative term, in absence of actual detrital mode data."@en ;
  rdfs:label "Lithic-rich epiclastic material "@en ;
  rdfs:subClassOf gsmc:epiclastic_granular_material ;
.
gsmc:Microlite
  a owl:Class ;
  rdfs:comment "Granular material consisting of minute incipient crystals that display some birefringence in thin section; mineralogy not discernible with hand lense. Coarser grained than crystallite."@en ;
  rdfs:comment "dct:source--  Williams, Turner, Gilbert 1954"@en ;
  rdfs:label "microlite"@en ;
  rdfs:subClassOf gsog:Crystallized_Particle_Material ;
.
gsmc:Mono_mineralic_granular_material
  a owl:Class ;
  rdfs:comment "Granular material composed of greater than 75 percent of particles consisting of a single mineral species."@en ;
  rdfs:comment "dct:source--  NADM SLTTm 2004"@en ;
  rdfs:label "mono mineralic granular material"@en ;
  rdfs:subClassOf gsog:Granular_Material ;
.
gsmc:Monomictic_granular_material
  a owl:Class ;
  rdfs:comment "Granular material consisting of grains or clasts composed of a single rock or mineral type (Jackson, 1997)"@en ;
  rdfs:comment "dct:source--  Jackson 1997"@en ;
  rdfs:label "monomictic granular material"@en ;
  rdfs:subClassOf gsog:Granular_Particle_Material ;
.
gsmc:Polymictic_granular_material
  a owl:Class ;
  rdfs:comment "Granular material consisting of grains or clasts composed of multiple mineral or rock types"@en ;
  rdfs:comment "dct:source--  Jackson, 1997, p. 501"@en ;
  rdfs:label "polymictic"@en ;
  rdfs:subClassOf gsog:Granular_Particle_Material ;
.
gsmc:Quartz_rich_epiclastic_material
  a owl:Class ;
  rdfs:comment "Epiclastic material consisting largely of quartz mineral particles. Qualitative term, in absence of actual detrital mode data."@en ;
  rdfs:label "Quartz-rich epiclastic material "@en ;
  rdfs:subClassOf gsmc:epiclastic_granular_material ;
.
gsmc:Sparite
  a owl:Class ;
  rdfs:comment "Crystalline granular material composed of carbonate minerals, usually calcite or dolomite, interpreted to be precipitated in situ, with grain size greater than about 10 microns."@en ;
  rdfs:label "Sparite "@en ;
  rdfs:subClassOf gsog:Crystallized_Particle_Material ;
.
gsmc:Spherulitic_granular_material
  a owl:Class ;
  rdfs:comment "Granular material consisting of rounded or spherical masses of acicular or fibrous mineral, typically in glassy siliceous lava."@en ;
  rdfs:comment "dct:source--  definition of spherule from Williams, Turner, Gilbert 1954"@en ;
  rdfs:label "Spherulitic granular material"@en ;
  rdfs:subClassOf gsog:Aggregate_non-clastic_particle_material ;
.
gsmc:Syngenetic_granular_material
  a owl:Class ;
  rdfs:comment "Granular material consisting of nonbiogenic particles formed by in situ or intrabasinal physical-chemical-mechanical processes without the direct biochemical activity of organisms, penecontemporaneously with sediment accumulation or during diagenetic modification."@en ;
  rdfs:comment "dct:source--  NADM SLTTs 2004"@en ;
  rdfs:label "syngenetic granular material"@en ;
  rdfs:subClassOf gsog:Granular_Particle_Material ;
.
gsmc:Variolitic_granular_material
  a owl:Class ;
  rdfs:comment "Granular material consisting of spherulitic clusters of crystals in a mafic rock, usually consisting of divergent plagioclase fibers, with or without interstitial glass, or intergrown with granules of pyroxene, olivine or iron ore. (equivalent to Spherule, but in mafic rock)"@en ;
  rdfs:comment "dct:source-- definition of variole from Williams, Turner, Gilbert 1954"@en ;
  rdfs:label "Variolitic granular material"@en ;
  rdfs:subClassOf gsmc:Spherulitic_granular_material ;
.
gsmc:accidental_pyroclastic_fragment
  a owl:Class ;
  rdfs:comment "Granular material consisting of fragments of rock generated by disruption as a direct result of volcanic action but not formed by previous activity of the magmatic system, generally derived from subvolcanic basement."@en ;
  rdfs:comment "dct:source--  Gillespie and Styles 1999"@en ;
  rdfs:label "accidental pyroclastic granular material"@en ;
  rdfs:subClassOf gsog:pyroclastic_granular_material ;
.
gsmc:arkosic_epiclastic_material
  a owl:Class ;
  rdfs:comment "Sandstone petrographic composition term indicating that detrital mode for clastic rock (Q-F-L) includes less than 75 percent quartz and the feldspar to lithic ratio is greater than 3 to 1. This corresponds to the arkose field of Folk (1968). For clastic rocks with little or no matrix and cement, rocks in this detrital mode composition category will also have quartz-feldspathic mineralogical composition."@en ;
  rdfs:comment "dct:source--  Folk1968"@en ;
  rdfs:label "arkosic epiclastic material"@en ;
  rdfs:subClassOf gsmc:feldspathic_epiclastic_material ;
.
gsmc:asphaltic_bearing_material
  a owl:Class ;
  rdfs:comment "Material contains greater than 5 percent (by volume) of asphalt, which is a 'dark brown to black viscous liquid or low-melting solid bitumen that consists almost entirely of carbon and hydrogen...[and] formed in oil-bearing rocks by the evaporation of volatiles...' (Jackson, 1997, p. 39)."@en ;
  rdfs:comment "dct:source--  Jackson 1997"@en ;
  rdfs:label "asphaltic"@en ;
  rdfs:subClassOf gsmc:carbonaceous_bearing_material ;
.
gsmc:autoclastic_granular_material
  a owl:Class ;
  rdfs:comment "Granular material consisting of fragments of extrusive igneous rock formed by mechanical friction of moving lava flow, breakage of chilled lava flow rinds, or gravity crumbling of active spines and domes. Gillespie and Styles (1999) include as type of juvenile pyroclastic fragment, inconsistent with definition of pyroclastic by IUGS and BGS."@en ;
  rdfs:comment "dct:source--  Gillespie and Styles, 1999"@en ;
  rdfs:label "autoclastic granular material"@en ;
  rdfs:subClassOf gsog:Clastic_Granular_Material ;
.
gsmc:barium_bearing_carbonate_material
  a owl:Class ;
  rdfs:comment "CO3 is the predominant anion, and greater than 5 mole percent of cations are Ba."@en ;
  rdfs:comment "dct:source--  This vocabulary"@en ;
  rdfs:label "barium bearing carbonate chemistry"@en ;
  rdfs:subClassOf gsmc:carbonate_composition_material ;
.
gsmc:bioclastic_granular_material
  a owl:Class ;
  rdfs:comment "Granular material consisting of particles that are shell, bone, or other hard skeletal structure of an animal, plant, or protozoan. May be fossilized or non-fossilized. Use in situations where fossil organism can not be identified, thus 'material fossil' is too specific."@en ;
  rdfs:comment "dct:source--  This vocabulary"@en ;
  rdfs:label "bioclastic granular material"@en ;
  rdfs:subClassOf gsog:Biogenic_Granular_Material ;
.
gsmc:calcareous_carbonate_bearing_material
  a owl:Class ;
  rdfs:comment "Material in which greater than 5 percent , but less than 50 percent of rock (by volume) consists of calcium carbonate minerals;  material contains sufficient CaCO3 to react forming bubbles when hydrochloric acid is applied."@en ;
  rdfs:comment "dct:source--  NADM SLTTm 2004"@en ;
  rdfs:label "calcareous"@en ;
  rdfs:subClassOf gsmc:carbonate_mineral_bearing_material ;
.
gsmc:calcareous_carbonate_monomeralic_material
  a owl:Class ;
  rdfs:comment "Carbonate minerals form greater than 75 percent of rock, and calcium carbonate minerals (calcite, aragonite) form greater than 75 percent of carbonate mineral fraction."@en ;
  rdfs:comment "dct:source--  NADM SLTTm 2004"@en ;
  rdfs:label "calcareous monomeralic carbonate"@en ;
  rdfs:subClassOf gsmc:calcium_rich_carbonate_chemistry ;
  rdfs:subClassOf gsmc:carbonate_monomeralic_material ;
.
gsmc:calcium_rich_carbonate_material
  a owl:Class ;
  rdfs:comment "CO3 is the predominante anion, and the Ca is the most abundant (mole percent) cation."@en ;
  rdfs:comment "dct:source--  Struik etal 2002, This vocabulary"@en ;
  rdfs:label "calcium rich carbonate chemistry"@en ;
  rdfs:subClassOf gsmc:carbonate_composition_material ;
.
gsmc:calcsilicate_mineral_bearing_material
  a owl:Class ;
  rdfs:comment "Material in which greater than 5 percent , but less than 50 percent of rock (by volume) consists of calcsilicate minerals of any sort. Calcsilicate minerals include andradite, calcic plagioclase, clinozoisite, diopside, epidote, grossular, grossular-hibschite Series, hedenbergite, johannsenite, meionite, prehnite, pumpellyite, titanite, uvarovite, vesuvianite, wollastonite, zoisite (https://www.mindat.org/min-51217.html)"@en ;
  rdfs:comment "dct:source--  This vocabulary"@en ;
  rdfs:label "calcsilicate bearing"@en ;
  rdfs:subClassOf gslth:Material ;
.
gsmc:calcsilicate_mineral_rich_material
  a owl:Class ;
  rdfs:comment "Material consists of greater than or equal to 50 percent calcsilicate or carbonate minerals and carbonate minerals less than or equal to calcsilicate minerals in mineral mode."@en ;
  rdfs:comment "dct:source--  NADM SLTTm 2004"@en ;
  rdfs:label "calcsilicate"@en ;
  rdfs:subClassOf gslth:Material ;
.
gsmc:calcsilicate_or_carbonate_mineral_material
  a owl:Class ;
  rdfs:comment "Material consists of greater than 50 percent calcsilicate or carbonate minerals and relative proportion of calcsilicate and carbonate minerals is unknown or not specified."@en ;
  rdfs:comment "dct:source--  NADM SLTTm 2004"@en ;
  rdfs:label "impure calcsilicate or carbonate"@en ;
  rdfs:subClassOf gslth:Material ;
.
gsmc:carbonaceous_bearing_material
  a owl:Class ;
  rdfs:comment "Containing greater than 5 percent reduced carbon in compounds that are typically the diagenetic products of dead organisms (e.g. coal, oil, gas, lignite, peat). 5 percent value is chosen for consistency with SLTTs usage of term carbonaceous."@en ;
  rdfs:comment "dct:source--  Struik2002, SLTTs2004, This vocabulary"@en ;
  rdfs:label "carbonaceous compound bearing material"@en ;
  rdfs:subClassOf gslth:Material ;
.
gsmc:carbonaceous_material
  a owl:Class ;
  rdfs:comment "Material containing greater that 50 percent (by volume) carbon or hydrocarbon mineral phases, including coal, oil, gas, lignite, peat."@en ;
  rdfs:comment "dct:source--  This vocabulary"@en ;
  rdfs:label "carbonaceous"@en ;
  rdfs:subClassOf gsmc:carbonaceous_bearing_material ;
.
gsmc:carbonate_composition_material
  a owl:Class ;
  rdfs:comment "Material in which carbonate (CO3) anion is the predominant anion (by mole percent) in chemical analysis. Sub-categories may be defined by dominant cation. Material in this chemical class overlaps with the monomineralic carbonate class, and probably overlaps with the Carbonate class in the mineralogical composition classification."@en ;
  rdfs:comment "dct:source--  Struik etal 2002, This vocabulary"@en ;
  rdfs:label "carbonate composition material"@en ;
  rdfs:subClassOf gslth:Material ;
.
gsmc:carbonate_lithic_epiclastic_material
  a owl:Class ;
  rdfs:comment "Granular material consisting of mechanically formed and deposited fragments of carbonate rock...derived from an older, lithified limestone or dolomite within, adjacent to, or outside the depositional site"@en ;
  rdfs:comment "dct:source--  Neuendorf et al., 2005, p. 375"@en ;
  rdfs:label "carbonate lithic epiclastic material"@en ;
  rdfs:subClassOf gsmc:lithic_epiclastic_material ;
.
gsmc:carbonate_mineral_bearing_material
  a owl:Class ;
  rdfs:comment "Material in which greater than 5 percent , but less than 50 percent of rock (by volume) consists of carbonate minerals of any sort ."@en ;
  rdfs:comment "dct:source--  This vocabulary"@en ;
  rdfs:label "carbonate bearing"@en ;
  rdfs:subClassOf gslth:Material ;
.
gsmc:carbonate_mineral_dominant_material
  a owl:Class ;
  rdfs:comment "Material consists of greater than 50 percent calcsilicate or carbonate minerals and carbonate minerals greater than calcsilicate minerals in mineral mode. Metacarbonate of NADMSC SLTTm (2004) terminology, adopted here for non-genetic use."@en ;
  rdfs:comment "dct:source--  NADM SLTTm 2004"@en ;
  rdfs:label "carbonate mineral dominant material"@en ;
  rdfs:subClassOf gslth:Material ;
.
gsmc:carbonate_monomeralic_material
  a owl:Class ;
  rdfs:comment "Rock in which carbonate minerals form greater than 75 percent of rock."@en ;
  rdfs:comment "dct:source--  NADM SLTTm 2004"@en ;
  rdfs:label "monomineralic carbonate"@en ;
  rdfs:subClassOf gsmc:carbonate_mineral_dominant_material ;
.
gsmc:chloride_composition_material
  a owl:Class ;
  rdfs:comment "Chloride is the most abundant (mole percent) anion"@en ;
  rdfs:comment "dct:source--  Struik etal 2002, This vocabulary"@en ;
  rdfs:label "chloride composition material"@en ;
  rdfs:subClassOf gslth:Material ;
.
gsmc:chlorite_mineral_bearing_material
  a owl:Class ;
  rdfs:comment "Greater than accessory amount (greater than 5 percent by volume) of chlorite group minerals are present"@en ;
  rdfs:comment "dct:source--  This vocabulary"@en ;
  rdfs:label "chloritic"@en ;
  rdfs:subClassOf gslth:Material ;
.
gsmc:clay_bearing_material
  a owl:Class ;
  rdfs:comment "Greater than accessory amount (greater than 5 percent by volume) of clay is present"@en ;
  rdfs:comment "dct:source--  This vocabulary"@en ;
  rdfs:label "argillic material"@en ;
  rdfs:subClassOf gslth:Material ;
.
gsmc:coated_particle_granular_material
  a owl:Class ;
  rdfs:comment "Granular material consisting of particles that have coats or layers of foreign material, usually fine mud-sized and occasionally recrystallized, that form concentric or overlapping shells around a core of rock, shell, peloidal, or intraclastic material. (eg: oolith, pisolith)"@en ;
  rdfs:comment "dct:source--  NADM SLTTs 2004"@en ;
  rdfs:label "coated particle granular material"@en ;
  rdfs:subClassOf gsog:Clastic_Granular_Material ;
.
gsmc:cognate_volcanic_granular_material
  a owl:Class ;
  rdfs:comment "Granular material consisting of fragments of rock formed during earlier (related) volcanic activity that have been ejected with other pyroclastic debris during a later eruption."@en ;
  rdfs:comment "dct:source--  Base on Gillespie and Styles, 1999"@en ;
  rdfs:label "cognate volcanic granular material"@en ;
  rdfs:subClassOf gsog:pyroclastic_granular_material ;
.
gsmc:coprolite_granular_material
  a owl:Class ;
  rdfs:comment "Granular material consisting of the fossilised excrement of vertebrate animals"@en ;
  rdfs:comment "dct:source--  Neuendorf et al., 2005"@en ;
  rdfs:label "coprolite"@en ;
  rdfs:subClassOf gsog:Biogenic_Granular_Material ;
.
gsmc:crystal_fragment_granular_material
  a owl:Class ;
  rdfs:comment "Granular material consisting of fragments crystals interpreted to have been broken by pyroclastic processes."@en ;
  rdfs:comment "dct:source--  this vocabulary"@en ;
  rdfs:label "crystal fragment granular material"@en ;
  rdfs:subClassOf gsog:pyroclastic_granular_material ;
.
gsmc:dolomite_bearing_material
  a owl:Class ;
  rdfs:comment "Material in which greater than 5 percent , but less than 50 percent of rock (by volume) consists of dolomite; carbonate minerals form less than 50 percent of rock."@en ;
  rdfs:comment "dct:source--  This vocabulary"@en ;
  rdfs:label "dolomite-bearing material"@en ;
  rdfs:subClassOf gsmc:carbonate_mineral_bearing_material ;
.
gsmc:dolomite_rich_material
  a owl:Class ;
  rdfs:comment "Carbonate minerals form greater than 75 percent of rock, and dolomite forms greater than 75 percent of carbonate minerals."@en ;
  rdfs:comment "dct:source--  NADM SLTTm 2004"@en ;
  rdfs:label "dolomite monomineralic carbonate"@en ;
  rdfs:subClassOf gsmc:carbonate_monomeralic_material ;
.
gsmc:epiclastic_granular_material
  a owl:Class ;
  rdfs:comment "Granular material consisting of grains or fragments produced by weathering and erosion of a pre-existing rock mass. Consists of particles whose origin as a fragment is a result of surface (sedimentary, weathering...) processes. 'Crystals, crystal fragments, glass and rock fragments that have been liberated from any type of pre-existing consolidated rock (volcanic or non-volcanic) by weathering or erosion and transported from the site of origin by gravity, air, water, or ice' [Schmid, 1981]. Distinguished from intraclast in that epiclast is derived from a pre-existing rock from outside the basin of deposition (NADM SLTTs 2004) before introduction into a clastic rock material."@en ;
  rdfs:comment "dct:source--  Schmid 1981, NADM SLTTs 2004"@en ;
  rdfs:label "epiclastic granular material"@en ;
  rdfs:subClassOf gsog:Clastic_Granular_Material ;
.
gsmc:fecal_pellet_granular_material
  a owl:Class ;
  rdfs:comment "Granular material consisting of organic excrement, mainly of invertebrates, occuring especially in modern marine sediments but also fossilised in some sedimentary rocks, usually with simple ovoid form, less commonly rod-shaped."@en ;
  rdfs:comment "dct:source--  Neuendorf et al., 2005"@en ;
  rdfs:label "fecal pellet granular material"@en ;
  rdfs:subClassOf gsog:Biogenic_Granular_Material ;
.
gsmc:feldspar_rich_epiclastic_material
  a owl:Class ;
  rdfs:comment "Epiclastic material consisting largely of feldspar mineral particles. Qualitative term, in absence of actual detrital mode data."@en ;
  rdfs:comment "dct:source--  This vocabulary"@en ;
  rdfs:label "feldspar rich epclastic material"@en ;
  rdfs:subClassOf gsmc:epiclastic_granular_material ;
.
gsmc:feldspathic_epiclastic_material
  a owl:Class ;
  rdfs:comment "Epiclastic material in which the ratio of feldspar to lithic fragments is greater than 1:1 and less than 75 percent quartz is present in the detrital mode.   General sandstone petrography term used to describe sand or sandstone.  Subsumes lithic arkosic and arkosic sandstone petrographic composition classes. Usage of modifier feldspathic is consistent with petrographic subdivisions of Dott (1964) and Williams, Turner and Gilbert (1982)"@en ;
  rdfs:comment "dct:source--  Dott1964, Folk1968"@en ;
  rdfs:label "feldspathic epiclastic material"@en ;
  rdfs:subClassOf gsmc:epiclastic_granular_material ;
.
gsmc:feldspathic_lithic_epiclastic_material
  a owl:Class ;
  rdfs:comment "Epiclastic material in which less than 75 percent of particles are quartz, and the ratio of feldspar to lithic fragments is between 1 to 1 and 1 to 3 in the detrital mode. This corresponds to the feldspathic litharenite field of Folk (1968). Rocks in this class are likely to be quartzo-feldspathic in terms of mineralogical composition, but because the mineralogical composition of the lithic fraction is not constrained, this correlation is not necessary."@en ;
  rdfs:comment "dct:source--  Folk1968"@en ;
  rdfs:label "feldspathic lithic epiclastic material"@en ;
  rdfs:subClassOf gsmc:lithic_epiclastic_material ;
.
gsmc:ferromagnesian_mineral_rich_material
  a owl:Class ;
  rdfs:comment "Material consists of greater than 40 percent dark ferromagnesian silicate minerals. Standard term defined by Bates and Jackson (1987) to mean 'containing iron and magnesium'. Subsumes mafic and ultramafic."@en ;
  rdfs:comment "dct:source--  NADM SLTTm 2004"@en ;
  rdfs:label "ferromagnesian"@en ;
  rdfs:subClassOf gslth:Material ;
.
gsmc:ferruginous_mineral_bearing_material
  a owl:Class ;
  rdfs:comment "Greater than accessory amount (greater than 5 percent by volume) of non-silicate iron minerals (hematite, magnetite, siderite...) are present. Rocks containing abundant iron-rich silicate minerals would use the 'Ferromagnesian' terms."@en ;
  rdfs:comment "dct:source--  This vocabulary"@en ;
  rdfs:label "ferruginous mineral-bearing material"@en ;
  rdfs:subClassOf gslth:Material ;
.
gsmc:fiamme_granular_material
  a owl:Class ;
  rdfs:comment "Granular material consisting of lens-shaped bodies, usually mm to cm thick, and centimeters to 1-2 decimeters long, typically seen on surfaces of some pyroclastic rocks. The name fiamme comes from the Italian word for flames, describing their shape. The term is descriptive and non-genetic. Generally interpreted to form by the collapse of pumice fragments during welding in a hot pyroclastic deposit."@en ;
  rdfs:comment "dct:source--  Neuendorf et al 2005, http://en.wikipedia.org/wiki/Fiamme"@en ;
  rdfs:label "fiamme granular material"@en ;
  rdfs:subClassOf gsog:pyroclastic_granular_material ;
.
gsmc:fluidal_pyroclastic_granular_material
  a owl:Class ;
  rdfs:comment "Granular material consisting of particles that have a rounded, fluidal shape indicating that they were in a wholly or partly molten state during formation and subsequent transport. Concept corresponds to bomb, but with no size denotation."@en ;
  rdfs:comment "dct:source--  Base on Gillespie and Styles, 1999"@en ;
  rdfs:label "fluidal pyroclastic granular material"@en ;
.
gsmc:fluoride_rich_composition_material
  a owl:Class ;
  rdfs:comment "Fluorine is the most abundant (mole percent) anion"@en ;
  rdfs:comment "dct:source--  Struik etal 2002, This vocabulary"@en ;
  rdfs:label "fluoride composition material"@en ;
  rdfs:subClassOf gslth:Material ;
.
gsmc:glass_shard_granular_material
  a owl:Class ;
  rdfs:comment "Granular material consisting of vitric fragments formed by pyroclastic processes, often with a characteristically curved surface of fracture. Shards generally consist of bubble-wall fragments produced by disintegration of pumice during or after an eruption"@en ;
  rdfs:comment "dct:source--  GGIPAC"@en ;
  rdfs:label "glass shard granular material"@en ;
.
gsmc:halide_rich_composition_material
  a owl:Class ;
  rdfs:comment "One or more of halide group elements (F, Cl, Br, I) are most abundant (mole percent) anion"@en ;
  rdfs:comment "dct:source--  Struik etal 2002, This vocabulary"@en ;
  rdfs:label "halide composition material"@en ;
  rdfs:subClassOf gslth:Material ;
.
gsmc:high_silica_material
  a owl:Class ;
  rdfs:comment "Containing 65 percent or more SiO2 by weight. Syn acid."@en ;
  rdfs:comment "dct:source--  Struik2002, SLTTs2004, This vocabulary"@en ;
  rdfs:label "high silica chemistry"@en ;
  rdfs:subClassOf gsmc:silicate_mineral_material ;
.
gsmc:hydroclastic_granular_material
  a owl:Class ;
  rdfs:comment "Granular material consisting of juvenile pyroclastic fragments formed by magma-water interaction during subaqueous or subglacial extrusion, typically consist of chilled glass."@en ;
  rdfs:comment "dct:source--  Gillespie and Styles 1999"@en ;
  rdfs:label "hydroclastic granular material"@en ;
.
gsmc:intermediate_silica_content_material
  a owl:Class ;
  rdfs:comment "Containing SiO2 in the range 52-65 percent, sometimes described as \\intermediate\\ rocks."@en ;
  rdfs:comment "dct:source--  Struik2002, SLTTs2004, This vocabulary"@en ;
  rdfs:label "intermediate silica chemistry"@en ;
  rdfs:subClassOf gsmc:silicate_mineral_material ;
.
gsmc:intraclastic_granular_material
  a owl:Class ;
  rdfs:comment "Granular material consisting of torn-up and re-worked fragments of penecontemporaneous sediment (usually weakly consolidated) that has been eroded within the basin of deposition...and re-deposited there...The fragment may range in size from fine sand to gravel...  A term introduced by Folk (1959, p. 4) for a component of limestone. "@en ;
  rdfs:comment "dct:source--  NADM SLTTs 2004, Neuendorf et al., 2005, Folk, 1959"@en ;
  rdfs:label "intraclastic granular material"@en ;
  rdfs:subClassOf gsog:Clastic_Granular_Material ;
.
gsmc:iron_bearing_carbonate_composition_material
  a owl:Class ;
  rdfs:comment "CO3 is the predominant anion, and iron is greater than 5 mole percent of the cations (includes Fe, Mg, Mn, Ba, Sr, Ca...)."@en ;
  rdfs:comment "dct:source--  This vocabulary"@en ;
  rdfs:label "iron bearing carbonate chemistry"@en ;
  rdfs:subClassOf gsmc:carbonate_composition_material ;
.
gsmc:iron_rich_carbonate_composition_material
  a owl:Class ;
  rdfs:comment "CO3 is the predominant anion, and iron is the most abundant (mole percent) cation"@en ;
  rdfs:comment "dct:source--  This vocabulary"@en ;
  rdfs:label "iron rich carbonate composition material"@en ;
  rdfs:subClassOf gsmc:iron_bearing_carbonate_composition_material ;
.
gsmc:juvenile_pyroclastic_granular_material
  a owl:Class ;
  rdfs:comment "Granular material consisting of fragments formed directly from cooling magma during transport prior to primary deposition."@en ;
  rdfs:comment "dct:source--  Gillespie and Styles 1999"@en ;
  rdfs:label "juvenile pyroclastic granular material"@en ;
  rdfs:subClassOf gsog:pyroclastic_granular_material ;
.
gsmc:lithic_arkosic_epiclastic_material
  a owl:Class ;
  rdfs:comment "Epiclastic material consisting of less than 75 percent quartz particles and the ratio of lithic fragments to feldspar particles is between 1:1 and 1:3 in the detrital mode. This corresponds to the lithic arkose field of Folk (1968), the 75 percent quartz boundary is chosen to be consistent with quartzsose composition as defined in the mineralogic compostion terms vocabulary. Because of the abundance of lithic fragments for which the mineralogic composition is not specified, and the presence of undiscernible matrix and cement that are not incuded in the detrital mode, corresondence with a mineralogical composition is very approximate."@en ;
  rdfs:comment "dct:source--  Folk1968"@en ;
  rdfs:label "lithic arkosic epiclastic material"@en ;
  rdfs:subClassOf gsmc:feldspathic_epiclastic_material ;
.
gsmc:lithic_epiclastic_material
  a owl:Class ;
  rdfs:comment "Epiclastic material consisting of less than 75 percent quartz paraticles, and the lithic to feldspar ratio is greater than 3 to 1 in the detrital mode. This corresponds to the litharenite field of Folk (1968). Because the mineralogy of the lithic fragments is not constrained, the mineralogical composition is largely independent of the detrital mode composition for this class."@en ;
  rdfs:comment "Epiclastic material consisting of less than 75 percent quartz particles, and the ratio of lithic fragments to feldspar is greater than 1:1 in the detrital mode. Because the mineralogy of the lithic fragments is not constrained, the mineralogical composition is largely independent of the detrital mode composition for this class."@en ;
  rdfs:comment "Granular material consisting of particles of rock derived by erosion from older, pre-existing rock materials of any kind, usually beyond the basin of accumulation but occasionally from within the basin of deposition (as from a submarine or subaqueous exposure adjacent to a depositional site). Particles can be identified as a piece of rock."@en ;
  rdfs:comment "dct:source--  Dott1964, Folk1968"@en ;
  rdfs:comment "dct:source--  Folk1968"@en ;
  rdfs:comment "dct:source--  this vocabulary"@en ;
  rdfs:label "lithic epiclastic material"@en ;
  rdfs:label "lithic rich detrital mode"@en ;
  rdfs:label "lithic rich epiclastic material"@en ;
  rdfs:subClassOf gsmc:epiclastic_granular_material ;
  rdfs:subClassOf gsmc:lithic_epiclastic_material ;
.
gsmc:low_silica_material
  a owl:Class ;
  rdfs:comment "Containing SiO2 in the range 44-52 percent. Syn basic."@en ;
  rdfs:comment "dct:source--  Struik2002, SLTTs2004, This vocabulary"@en ;
  rdfs:label "low silica chemistry"@en ;
  rdfs:subClassOf gsmc:silicate_mineral_material ;
.
gsmc:mafic_mineral_rich_material
  a owl:Class ;
  rdfs:comment "Material consists of greater than or equal to 40 percent and less than 90 percent ferromagnesian silicate minerals."@en ;
  rdfs:comment "dct:source--  NADM SLTTm 2004"@en ;
  rdfs:label "mafic"@en ;
  rdfs:subClassOf gsmc:ferromagnesian_mineral_rich_material ;
.
gsmc:magnesium_rich_carbonate_material
  a owl:Class ;
  rdfs:comment "CO3 is the predominant anion, and Mg is the most abundant (mole percent) cation."@en ;
  rdfs:comment "dct:source--  Struik etal 2002, This vocabulary"@en ;
  rdfs:label "magnesium rich carbonate chemistry"@en ;
  rdfs:subClassOf gsmc:carbonate_composition_material ;
.
gsmc:material_fossil_granular_material
  a owl:Class ;
  rdfs:comment "Granular material consisting of preserved or replaced remains (casts) of plants or animals. An additional type property element can provide a reference to a paleontologic description of the fossil or fossils present."@en ;
  rdfs:comment "dct:source--  GeoSciML v2 RC1 model element scope note"@en ;
  rdfs:label "material fossil material"@en ;
  rdfs:subClassOf gsmc:bioclastic_granular_material ;
.
gsmc:metallic_oxide_mineral_bearing
  a owl:Class ;
  rdfs:comment "Greater than accessory amounts (greater than 5 percent by volume) of base metal oxide minerals such as magnetite (Fe3O4) or pyrolusite (MnO2) are present."@en ;
  rdfs:comment "dct:source--  Struik2002, SLTTs2004, This vocabulary"@en ;
  rdfs:label "metallic oxide bearing"@en ;
  rdfs:subClassOf gslth:Material ;
.
gsmc:metaluminous_composition_material
  a owl:Class ;
  rdfs:comment "Chemical composition term used for igneous rocks, denoting that content of aluminum oxide is greater than sodium oxide plus potassium oxide, but aluminum oxide less than sum of Na, K and Ca oxide."@en ;
  rdfs:comment "dct:source--  Shand 1947"@en ;
  rdfs:label "metaluminous"@en ;
  rdfs:subClassOf gslth:Material ;
.
gsmc:mica_bearing_material
  a owl:Class ;
  rdfs:comment "Greater than accessory amount (greater than 5 percent by volume) of mica group mineral are present"@en ;
  rdfs:comment "dct:source--  This vocabulary"@en ;
  rdfs:label "micaceous"@en ;
  rdfs:subClassOf gslth:Material ;
.
gsmc:micrite
  a owl:Class ;
  rdfs:comment "Granular material consisting of carbonate mud with individual particles mostly less than 4 microns maximum diameter; might be of biogenic, biochemical or physiochemical origin. Constituent of a carbonate rock.  (Folk, 1959; Chilingar et al 1967 (https://doi.org/10.1016/S0070-4571(08)70844-6); Bissell and Chilingar, 1967; Neuendor et al., 2005)"@en ;
  rdfs:label "Micrite material"@en ;
  rdfs:subClassOf gsog:Clastic_Granular_Material ;
.
gsmc:nitrate_anion_rich_material
  a owl:Class ;
  rdfs:comment "Nitrate (NO3) is most abundant (mole percent) anion."@en ;
  rdfs:comment "dct:source--  Struik etal 2002, This vocabulary"@en ;
  rdfs:label "nitrate anion rich material"@en ;
  rdfs:subClassOf gslth:Material ;
.
gsmc:oncoid_granular_material
  a owl:Class ;
  rdfs:comment "Granular material consisting of  '...coated grains with a cortex of irregular, partially overlapping laminae. They are typically irregular in shape and may exhibit biogenic structures. Some forms lack a distinct nucleus. Oncoids are generally larger than 2 mm.' (Hallsworth and Knox, 1999, p. 27). Synonymous with oncolite: A small, variously shaped, concentrically laminated, calcareous sedimentary structure, resembling an oolith, and formed by the accretion of successive layer[s]... It...generally does not exceed 10 cm in dimension. (Jackson, 1997, p. 446)."@en ;
  rdfs:comment "dct:source--  Jackson 1997, Hallsworth and Knox 1999"@en ;
  rdfs:label "oncoid granular material"@en ;
  rdfs:subClassOf gsmc:coated_particle_granular_material ;
.
gsmc:ontology
  a owl:Ontology ;
  rdfs:comment "This file contains the 2016 SKOS-RDF version of the CGI Composition Category vocabulary. Compilation and review in MS Excel spreadsheet, converted to MS Excel for SKOS generation using GSML_SKOS_fromXLS_2016.01.xslt."@en ;
  rdfs:comment "This file contains the CGI Particle type vocabulary, as defined by the IUGS Commission for Geoscience Information (CGI) Geoscience Terminology Working Group. Used to specify particleType in particleTypeDescription associated with a compoundMaterial. Terms to specify the nature of individual particles of each constituent in an aggregation, based mostly on their genesis. Because the constituents are identifiable parts, the part units must have some definition. Examples include clasts, crystals, pore space, material fossil. Constituent type is determined based on the nature of the particles, and ideally is independent of the relationship between particles in a compound material aggregation. By extension, this vocabulary includes all concepts in this conceptScheme, as well as concepts in any previous versions of the scheme."@en ;
  rdfs:comment "This file is derived from the 2016 SKOS-RDF version of the CGI Particle Type vocabulary. Compilation and review in MS Excel spreadsheet, converted to MS Excel for SKOS generation using SKOS_for_GA_from_XLS_2016.03.xslt. Owl conversion by Stephen M. Richard for Loop3D project. Particle/consituent roles have been separated into a praticle role vocabulary."@en ;
  rdfs:comment "This scheme describes the concept space for Composition Category concepts, as defined by the IUGS Commission for Geoscience Information (CGI) Geoscience Terminology Working Group. Original purpose for populating the materialcategory property in GeoSciML CompoundMaterialDescription elements."@en ;
  rdfs:comment "dct:creator--  CGI Concept Definition Task Group, Stephen M. Richard OWL conversion for Loop3D project" ;
  rdfs:comment "dct:creator--  CGI Geoscience Terminology Working Group, Stephen M. Richard"@en ;
  rdfs:comment "dct:date--  2012-11" ;
  rdfs:comment "dct:date--  2016-11-25"@en ;
  rdfs:comment "dct:modified-- 2020-02-03"@en ;
  rdfs:comment "dct:modified-- 2020-02-06" ;
  rdfs:label "Composition Category"@en ;
  rdfs:label "Particle Type categories"@en ;
  owl:imports gsog:ontology ;
  owl:imports <http://loop3d.org/GSO/ontology/2020/1/geologicquality/ontology> ;
.
gsmc:oolitic_granular_material
  a owl:Class ;
  rdfs:comment "Granular material consisting of particles that resembles an oolith in outer appearance and size- (Jackson, 1997, p. 447). Hallsworth and Knox (1999, p. 27) describe ooids as coated grains that typically are spherical or ellipsoidal in shape, with the degree of roundness increasing outward. Concentric to semi-concentric coats are smoothly and evenly laminated. A nucleus usually is present, and may have a composition different from the coatings. Biogenic structures are not obvious. NADMSC SLTTs (2004) considers synomous with oolith."@en ;
  rdfs:comment "dct:source--  Jackson1997, Hallsworth and Knox 1999"@en ;
  rdfs:label "oolitic granular material"@en ;
  rdfs:subClassOf gsmc:coated_particle_granular_material ;
.
gsmc:other_composition_material
  a owl:Class ;
  rdfs:comment "Composition is known but doesnâ€™t' fit in any other category"@en ;
  rdfs:comment "dct:source--  This vocabulary"@en ;
  rdfs:label "other composition"@en ;
  rdfs:subClassOf gslth:Material ;
.
gsmc:oxide_mineral_rich_material
  a owl:Class ;
  rdfs:comment "Material predominantly composed of oxide minerals"@en ;
  rdfs:comment "dct:source--  This vocabulary"@en ;
  rdfs:label "oxide"@en ;
  rdfs:subClassOf gslth:Material ;
.
gsmc:pelitic_mineral_rich_material
  a owl:Class ;
  rdfs:comment "Material for which the sum of modal quartz+feldspar+ mica + aluminous mineral is greater than or equal to 70 percent, and aluminous mineral + mica content is greater than or equal to 40 percent."@en ;
  rdfs:comment "dct:source--  NADM SLTTm 2004"@en ;
  rdfs:label "pelitic mineral rich material"@en ;
  rdfs:subClassOf gsmc:quartz_feldspar_pelitic_mineral_material ;
.
gsmc:peloid_granular_material
  a owl:Class ;
  rdfs:comment "Granular material consisting of usually rounded aggregates of clay-sized calcareous (micritic) material, origin and size are not specified"@en ;
  rdfs:comment "dct:source--  Neuendorf et al., 2005"@en ;
  rdfs:label "peloid granular material"@en ;
  rdfs:subClassOf gsog:Clastic_Granular_Material ;
.
gsmc:peralkaline_composition_material
  a owl:Class ;
  rdfs:comment "Aluminum oxide (Al2O3) is less than sum of K and Na oxide."@en ;
  rdfs:comment "dct:source--  Shand 1947"@en ;
  rdfs:label "peralkaline"@en ;
  rdfs:subClassOf gslth:Material ;
.
gsmc:peraluminous_composition_material
  a owl:Class ;
  rdfs:comment "Aluminum oxide (Al2O3) greater than sum of Na, K and Ca oxide."@en ;
  rdfs:comment "dct:source--  Shand 1947"@en ;
  rdfs:label "peraluminous"@en ;
  rdfs:subClassOf gslth:Material ;
.
gsmc:petroliferous_material
  a owl:Class ;
  rdfs:comment "Crude oil or natural gas is present, generally in trace amounts, commonly detected by smell"@en ;
  rdfs:comment "dct:source--  This vocabulary"@en ;
  rdfs:label "petroliferous"@en ;
  rdfs:subClassOf gslth:Material ;
.
gsmc:phosphate_composition_material
  a owl:Class ;
  rdfs:comment "Phosphate (PO4) is the most abundant (mole percent) anion."@en ;
  rdfs:comment "dct:source--  Struik etal 2002, This vocabulary"@en ;
  rdfs:label "phosphate chemistry"@en ;
  rdfs:subClassOf gslth:Material ;
.
gsmc:phosphatic_mineral_bearing_material
  a owl:Class ;
  rdfs:comment "Greater than accessory amount (greater than 5 percent by volume) of phosphate minerals are present"@en ;
  rdfs:comment "dct:source--  This vocabulary"@en ;
  rdfs:label "phosphatic"@en ;
  rdfs:subClassOf gslth:Material ;
.
gsmc:pisolitic_granular_material
  a owl:Class ;
  rdfs:comment "Granular material consisting of round or ellipsoidal accretionary particles resembling a pea in size and shape.... A pisoid...is larger and less regular in form than an ooid, although it may have the same concentric and/or radial internal structure (Jackson, 1997, p. 489)."@en ;
  rdfs:comment "dct:source--  NADM SLTTs 2004, Jackson 1997"@en ;
  rdfs:label "pisolitic granular material"@en ;
  rdfs:subClassOf gsmc:coated_particle_granular_material ;
.
gsmc:quartz_feldspar_pelitic_mineral_material
  a owl:Class ;
  rdfs:comment "Material for which the sum of modal quartz+feldspar+ mica + aluminous mineral is greater than or equal to 70 percent."@en ;
  rdfs:comment "dct:source--  NADM SLTTm 2004"@en ;
  rdfs:label "quartz feldspar pelitic"@en ;
  rdfs:subClassOf gslth:Material ;
.
gsmc:quartzo_feldspathic_mineral_material
  a owl:Class ;
  rdfs:comment "Material for which the sum of modal quartz+feldspar+ mica + aluminous mineral is greater than or equal to 70 percent, and quartz + feldspar (sensu Robertson, 1999) greater than 60 percent."@en ;
  rdfs:comment "dct:source--  NADM SLTTm 2004"@en ;
  rdfs:label "quartzo feldspathic"@en ;
  rdfs:subClassOf gsmc:quartz_feldspar_pelitic_mineral_material ;
.
gsmc:quartzose_epiclastic_material
  a owl:Class ;
  rdfs:comment "Epiclastic material consisting of greater than 95 percent quartz particles. This petrographic criteria follows the most restrictive definition of the composition field at the quartz vertex of the sandstone QFL triangle (Folk, 1968). This use of term quartzose is more restrictive that that used in the mineralogical composition term vocabulary, reflecting the interpretive significance of pure quartz sandstones in sedimentary petrology."@en ;
  rdfs:comment "dct:source--  Folk1968, This vocabulary"@en ;
  rdfs:label "quartzose detrital mode"@en ;
  rdfs:subClassOf gsmc:epiclastic_granular_material ;
.
gsmc:quartzose_material
  a owl:Class ;
  rdfs:comment "Material consists of greater than or equal to 75 percent quartz."@en ;
  rdfs:comment "dct:source--  NADM SLTTm 2004"@en ;
  rdfs:label "quartzose"@en ;
  rdfs:subClassOf gsmc:quartzo_feldspathic_mineral_material ;
.
gsmc:reworked_pyroclastic_granular_material
  a owl:Class ;
  rdfs:comment "Granular material consisting of fragments formed as a direct result of volcanic activity and reworked by sedimentary processes."@en ;
  rdfs:comment "dct:source--  Gillespie and Styles 1999"@en ;
  rdfs:label "reworked pyroclastic granular material"@en ;
  rdfs:subClassOf gsog:Clastic_Granular_Material ;
.
gsmc:semi_pelitic_mineral_rich_material
  a owl:Class ;
  rdfs:comment "Material for which the sum of modal quartz+feldspar+ mica + aluminous mineral is greater than or equal to 70 percent, and quartz+ feldspar less than 60 percent"@en ;
  rdfs:comment "dct:source--  NADM SLTTm 2004"@en ;
  rdfs:label "semi pelitic"@en ;
  rdfs:subClassOf gsmc:quartz_feldspar_pelitic_mineral_material ;
.
gsmc:silicate_mineral_material
  a owl:Class ;
  rdfs:comment "Composed of minerals whose crystal structure contains SiO4 tetrahedra, either isolated or joined through one or more oxygen atoms to form groups, chains, sheets or three-dimensional structures with metallic cations. Composition ranges from 20-100 percent SiO2. Typically some Al substitutues for silica. A survey of chemical analyses in the Georock database (query FOR ALL GEOLOGICAL SETTINGS, MATERIAL: WHOLE ROCK (AND VOLCANIC GLASS), PUB. YEARS: 2005-1970), 10/10/2005, http://georoc.mpch-mainz.gwdg.de/georoc/Entry.html) discovered that the lowest silica (Si02) content for igneous rock is about 20 percent. This is consistent with the lowest silica content found for a silicate mineral is about 21 percent for a chlorite variety found by scanning the mineral analyses in Deer, Howie, and Zussman (1966)."@en ;
  rdfs:comment "dct:source--  Neuendorf et al 2005, Struik 2002, This vocabulary"@en ;
  rdfs:label "silicate chemistry"@en ;
  rdfs:subClassOf gslth:Material ;
.
gsmc:silicic_material
  a owl:Class ;
  rdfs:comment "Greater than accessory amount (greater than 5 percent by volume) of silica, amorphous, as quartz, or any of the silica polymorphs are present"@en ;
  rdfs:comment "dct:source--  This vocabulary"@en ;
  rdfs:label "silicic material"@en ;
  rdfs:subClassOf gslth:Material ;
.
gsmc:sub_feldspathic_epiclastic_material
  a owl:Class ;
  rdfs:comment "Epiclastic material consisting of less than 50 percent lithic fragments, and between 75 and 95 percent quartz (thus less than 25 percent feldspar) in the detrital mode. This corresponds to the subarkose field of Folk (1968)."@en ;
  rdfs:comment "dct:source--  Folk1968"@en ;
  rdfs:label "sub feldspathic epiclastic material"@en ;
  rdfs:subClassOf gsmc:epiclastic_granular_material ;
.
gsmc:sub_lithic_granular_material
  a owl:Class ;
  rdfs:comment "Epiclastic material consisting of between 75 and 95 percent quartz with ratio of feldspar to lithic fragments that is less than 1 in the detrital mode. This corresponds to the sublitharenite field of Folk (1968), the 75 percent quartz boundary is consistent with quartzsose composition as defined in the mineralogic compostion terms vocabulary."@en ;
  rdfs:comment "dct:source--  Folk1968"@en ;
  rdfs:label "sub lithic granular material"@en ;
  rdfs:subClassOf gsmc:epiclastic_granular_material ;
.
gsmc:subaluminous_composition_material
  a owl:Class ;
  rdfs:comment "Aluminum oxide within 10 percent of sum of Na and K oxide. Generally applied to igneous rocks"@en ;
  rdfs:comment "dct:source--  Shand 1947"@en ;
  rdfs:label "subaluminous"@en ;
  rdfs:subClassOf gslth:Material ;
.
gsmc:sulfate_composition_material
  a owl:Class ;
  rdfs:comment "Sulfate is the most abundant anion"@en ;
  rdfs:comment "dct:source--  Struik etal 2002, This vocabulary"@en ;
  rdfs:label "sulfate chemistry material"@en ;
  rdfs:subClassOf gslth:Material ;
.
gsmc:sulfate_mineral_rich_material
  a owl:Class ;
  rdfs:comment "Material predominantly composed of sulfate minerals"@en ;
  rdfs:comment "dct:source--  This vocabulary"@en ;
  rdfs:label "sulfate"@en ;
  rdfs:subClassOf gslth:Material ;
.
gsmc:sulfide_composition_material
  a owl:Class ;
  rdfs:comment "Sulfur is the most abundant anion, cations are metals or semimetals."@en ;
  rdfs:comment "dct:source--  Neuendorf et al 2005, Struik 2002, This vocabulary"@en ;
  rdfs:label "sulfide chemistry material"@en ;
  rdfs:subClassOf gslth:Material ;
.
gsmc:sulfide_mineral_bearing_material
  a owl:Class ;
  rdfs:comment "Greater than accessory amount (greater than 5 percent by volume) of sulfide mineral are present"@en ;
  rdfs:comment "dct:source--  This vocabulary"@en ;
  rdfs:label "sulfide mineral-bearing_material"@en ;
  rdfs:subClassOf gslth:Material ;
.
gsmc:sulfide_mineral_rich_material
  a owl:Class ;
  rdfs:comment "Material predominantly composed of sulfide minerals"@en ;
  rdfs:comment "dct:source--  This vocabulary"@en ;
  rdfs:label "sulfide"@en ;
  rdfs:subClassOf gslth:Material ;
.
gsmc:sulfosalt_composition_material
  a owl:Class ;
  rdfs:comment "Sulfide in which a semimetal (As, Sb, Bi) is present in a cation role"@en ;
  rdfs:comment "dct:source--  Neuendorf et al 2005, Struik 2002, This vocabulary"@en ;
  rdfs:label "sulfosalt chemistry_material"@en ;
  rdfs:subClassOf gsmc:sulfide_composition_material ;
.
gsmc:ultramafic_mineral_rich_material
  a owl:Class ;
  rdfs:comment "Material consists of greater than 90 percent ferromagnesian silicate minerals."@en ;
  rdfs:comment "dct:source--  NADM SLTTm 2004"@en ;
  rdfs:label "ultramafic mineral rich"@en ;
  rdfs:subClassOf gsmc:ferromagnesian_mineral_rich_material ;
.
gsmc:ventrifact_granular_material
  a owl:Class ;
  rdfs:comment "Granular material consisting of particles that has been shaped, worn, faceted, cut or polished by the abrasive action of windblown particles."@en ;
  rdfs:comment "dct:source-- base on Neuendorf et al., 2005"@en ;
  rdfs:label "ventrifact granular material"@en ;
  rdfs:subClassOf gsog:Clastic_Granular_Material ;
.
gsmc:very_low_silica_material
  a owl:Class ;
  rdfs:comment "Containing between about 20 and 44 percent SiO2. A survey of chemical analyses in the Georock database (query FOR ALL GEOLOGICAL SETTINGS, MATERIAL: WHOLE ROCK (AND VOLCANIC GLASS), PUB. YEARS: 2005-1970), 10/10/2005, http://georoc.mpch-mainz.gwdg. syn ultrabasic."@en ;
  rdfs:comment "dct:source--  Struik2002, SLTTs2004, This vocabulary"@en ;
  rdfs:label "very low silica chemistry_material"@en ;
  rdfs:subClassOf gsmc:silicate_mineral_material ;
.
gsmc:volcanic_lithic_epiclastic_material
  a owl:Class ;
  rdfs:comment "Sedimentary material contains significant broken volcanic rock fragments or vitric fragments, irrespective of their pyroclastic or epiclastic origin."@en ;
  rdfs:comment "dct:source--  This vocabulary"@en ;
  rdfs:label "volcanic lithic epiclastic material"@en ;
  rdfs:subClassOf gsmc:lithic_epiclastic_material ;
.
gsmc:xenocryst_granular_material
  a owl:Class ;
  rdfs:comment "A xenocryst in general can not play a framework role in a Rock Material"@en ;
  rdfs:comment "Granular material consisting of crystals that resemble phenocrysts in an igneous rock, but that are foreign to the rock in which they occur - not formed by crystallization of the magma that formed the igneous rock."@en ;
  rdfs:comment "dct:source--  Neuendorf et al., 2005"@en ;
  rdfs:label "xenocryst granular material"@en ;
  rdfs:subClassOf gsog:Crystal_Constituent ;
.
